<?xml version="1.0"?>
<rdf:RDF xmlns="http://web-development-ontology.netlify.app/wdo/"
     xml:base="http://web-development-ontology.netlify.app/wdo/"
     xmlns:dc="http://purl.org/dc/elements/1.1/"
     xmlns:owl="http://www.w3.org/2002/07/owl#"
     xmlns:rdf="http://www.w3.org/1999/02/22-rdf-syntax-ns#"
     xmlns:xml="http://www.w3.org/XML/1998/namespace"
     xmlns:xsd="http://www.w3.org/2001/XMLSchema#"
     xmlns:rdfs="http://www.w3.org/2000/01/rdf-schema#"
     xmlns:skos="http://www.w3.org/2004/02/skos/core#"
     xmlns:terms="http://purl.org/dc/terms/">
    <owl:Ontology rdf:about="http://web-development-ontology.netlify.app/wdo/">
        <owl:versionIRI rdf:resource="http://web-development-ontology.netlify.app/wdo/1.0.0"/>
        <owl:imports rdf:resource="http://purl.obolibrary.org/obo/bfo/2020/bfo-core.owl"/>
        <dc:creator xml:lang="en">Group One, CoSc 6232 (Spring 2025)</dc:creator>
        <dc:description xml:lang="en">An ontology designed to support semantic-based explicit knowledge management for web development projects. WDO provides a structured vocabulary for representing artifacts like codebase components (classes, functions, attributes), documentation, licensing information, READMEs, best practices, and various digital assets extracted from local repositories or github oranizations. Its goal is to simplify the management, retrieval, and understanding of explicit knowledge within web development projects.</dc:description>
        <dc:identifier>WDO</dc:identifier>
        <dc:publisher xml:lang="en">Department of Computer Science, Addis Ababa University</dc:publisher>
        <dc:rights xml:lang="en">MIT License</dc:rights>
        <dc:title xml:lang="en">Web Development Ontology</dc:title>
        <rdfs:comment xml:lang="en">Web Development Ontology (WDO) is aligned with Basic Formal Ontology (BFO) 2020 (http://purl.obolibrary.org/obo/bfo/2020/bfo-core.owl) as its top-level ontology and adapts concepts from DoCO and CodeOntology where relevant to the web development domain.</rdfs:comment>
        <rdfs:seeAlso rdf:resource="https://github.com/shama-llama/semantic-web-kms"/>
        <owl:versionInfo xml:lang="en">1.0.0</owl:versionInfo>
    </owl:Ontology>
    


    <!-- 
    ///////////////////////////////////////////////////////////////////////////////////////
    //
    // Annotation properties
    //
    ///////////////////////////////////////////////////////////////////////////////////////
     -->


    


    <!-- http://purl.org/dc/elements/1.1/contributor -->


    <owl:AnnotationProperty rdf:about="http://purl.org/dc/elements/1.1/contributor"/>
    


    <!-- http://purl.org/dc/elements/1.1/creator -->


    <owl:AnnotationProperty rdf:about="http://purl.org/dc/elements/1.1/creator"/>
    


    <!-- http://purl.org/dc/elements/1.1/date -->


    <owl:AnnotationProperty rdf:about="http://purl.org/dc/elements/1.1/date"/>
    


    <!-- http://purl.org/dc/elements/1.1/description -->


    <owl:AnnotationProperty rdf:about="http://purl.org/dc/elements/1.1/description"/>
    


    <!-- http://purl.org/dc/elements/1.1/identifier -->


    <owl:AnnotationProperty rdf:about="http://purl.org/dc/elements/1.1/identifier"/>
    


    <!-- http://purl.org/dc/elements/1.1/license -->


    <owl:AnnotationProperty rdf:about="http://purl.org/dc/elements/1.1/license"/>
    


    <!-- http://purl.org/dc/elements/1.1/publisher -->


    <owl:AnnotationProperty rdf:about="http://purl.org/dc/elements/1.1/publisher"/>
    


    <!-- http://purl.org/dc/elements/1.1/rights -->


    <owl:AnnotationProperty rdf:about="http://purl.org/dc/elements/1.1/rights"/>
    


    <!-- http://purl.org/dc/elements/1.1/title -->


    <owl:AnnotationProperty rdf:about="http://purl.org/dc/elements/1.1/title"/>
    


    <!-- http://purl.org/dc/terms/description -->


    <owl:AnnotationProperty rdf:about="http://purl.org/dc/terms/description"/>
    


    <!-- http://purl.org/dc/terms/license -->


    <owl:AnnotationProperty rdf:about="http://purl.org/dc/terms/license"/>
    


    <!-- http://purl.org/dc/terms/title -->


    <owl:AnnotationProperty rdf:about="http://purl.org/dc/terms/title"/>
    


    <!-- http://www.w3.org/2000/01/rdf-schema#comment -->


    <owl:AnnotationProperty rdf:about="http://www.w3.org/2000/01/rdf-schema#comment"/>
    


    <!-- http://www.w3.org/2000/01/rdf-schema#label -->


    <owl:AnnotationProperty rdf:about="http://www.w3.org/2000/01/rdf-schema#label"/>
    


    <!-- http://www.w3.org/2000/01/rdf-schema#seeAlso -->


    <owl:AnnotationProperty rdf:about="http://www.w3.org/2000/01/rdf-schema#seeAlso"/>
    


    <!-- http://www.w3.org/2002/07/owl#imports -->


    <owl:AnnotationProperty rdf:about="http://www.w3.org/2002/07/owl#imports"/>
    


    <!-- http://www.w3.org/2002/07/owl#versionInfo -->


    <owl:AnnotationProperty rdf:about="http://www.w3.org/2002/07/owl#versionInfo"/>
    


    <!-- http://www.w3.org/2004/02/skos/core#altLabel -->


    <owl:AnnotationProperty rdf:about="http://www.w3.org/2004/02/skos/core#altLabel"/>
    


    <!-- http://www.w3.org/2004/02/skos/core#definition -->


    <owl:AnnotationProperty rdf:about="http://www.w3.org/2004/02/skos/core#definition"/>
    


    <!-- http://www.w3.org/2004/02/skos/core#example -->


    <owl:AnnotationProperty rdf:about="http://www.w3.org/2004/02/skos/core#example"/>
    


    <!-- http://www.w3.org/2004/02/skos/core#prefLabel -->


    <owl:AnnotationProperty rdf:about="http://www.w3.org/2004/02/skos/core#prefLabel"/>
    


    <!-- http://www.w3.org/2004/02/skos/core#scopeNote -->


    <owl:AnnotationProperty rdf:about="http://www.w3.org/2004/02/skos/core#scopeNote"/>
    


    <!-- 
    ///////////////////////////////////////////////////////////////////////////////////////
    //
    // Object Properties
    //
    ///////////////////////////////////////////////////////////////////////////////////////
     -->


    


    <!-- http://purl.obolibrary.org/obo/BFO_0000054 -->


    <owl:ObjectProperty rdf:about="http://purl.obolibrary.org/obo/BFO_0000054">
        <owl:inverseOf rdf:resource="http://purl.obolibrary.org/obo/BFO_0000055"/>
        <rdfs:domain rdf:resource="http://purl.obolibrary.org/obo/BFO_0000017"/>
        <rdfs:range rdf:resource="http://purl.obolibrary.org/obo/BFO_0000015"/>
        <dc:identifier>206-BFO</dc:identifier>
        <rdfs:label xml:lang="en">has realization</rdfs:label>
        <skos:altLabel xml:lang="en">realized in</skos:altLabel>
        <skos:definition xml:lang="en">b has realization c =Def c realizes b</skos:definition>
        <skos:example xml:lang="en">As for realizes</skos:example>
    </owl:ObjectProperty>
    


    <!-- http://purl.obolibrary.org/obo/BFO_0000055 -->


    <owl:ObjectProperty rdf:about="http://purl.obolibrary.org/obo/BFO_0000055">
        <rdfs:domain rdf:resource="http://purl.obolibrary.org/obo/BFO_0000015"/>
        <rdfs:range rdf:resource="http://purl.obolibrary.org/obo/BFO_0000017"/>
        <dc:identifier>059-BFO</dc:identifier>
        <rdfs:label xml:lang="en">realizes</rdfs:label>
        <skos:definition xml:lang="en">(Elucidation) realizes is a relation between a process b and realizable entity c such that c inheres in some d &amp; for all t, if b has participant d then c exists &amp; the type instantiated by b is correlated with the type instantiated by c</skos:definition>
        <skos:example xml:lang="en">A balding process realizes a disposition to go bald; a studying process realizes a student role; a process of pumping blood realizes the pumping function of a heart</skos:example>
        <skos:scopeNote xml:lang="en">Users that require more sophisticated representations of time are encouraged to import a temporal extension of BFO-Core provided by the BFO development team. See documentation for guidance: &lt;Link&gt;</skos:scopeNote>
    </owl:ObjectProperty>
    


    <!-- http://purl.obolibrary.org/obo/BFO_0000056 -->


    <owl:ObjectProperty rdf:about="http://purl.obolibrary.org/obo/BFO_0000056">
        <owl:inverseOf rdf:resource="http://purl.obolibrary.org/obo/BFO_0000057"/>
        <rdfs:domain>
            <owl:Class>
                <owl:unionOf rdf:parseType="Collection">
                    <rdf:Description rdf:about="http://purl.obolibrary.org/obo/BFO_0000020"/>
                    <rdf:Description rdf:about="http://purl.obolibrary.org/obo/BFO_0000031"/>
                    <owl:Class>
                        <owl:intersectionOf rdf:parseType="Collection">
                            <rdf:Description rdf:about="http://purl.obolibrary.org/obo/BFO_0000004"/>
                            <owl:Class>
                                <owl:complementOf rdf:resource="http://purl.obolibrary.org/obo/BFO_0000006"/>
                            </owl:Class>
                        </owl:intersectionOf>
                    </owl:Class>
                </owl:unionOf>
            </owl:Class>
        </rdfs:domain>
        <rdfs:range rdf:resource="http://purl.obolibrary.org/obo/BFO_0000015"/>
        <dc:identifier>250-BFO</dc:identifier>
        <rdfs:label xml:lang="en">participates in</rdfs:label>
        <skos:definition xml:lang="en">(Elucidation) participates in holds between some b that is either a specifically dependent continuant or generically dependent continuant or independent continuant that is not a spatial region &amp; some process p such that b participates in p some way</skos:definition>
        <skos:scopeNote xml:lang="en">Users that require more sophisticated representations of time are encouraged to import a temporal extension of BFO-Core provided by the BFO development team. See documentation for guidance: &lt;Link&gt;</skos:scopeNote>
    </owl:ObjectProperty>
    


    <!-- http://purl.obolibrary.org/obo/BFO_0000057 -->


    <owl:ObjectProperty rdf:about="http://purl.obolibrary.org/obo/BFO_0000057">
        <rdfs:domain rdf:resource="http://purl.obolibrary.org/obo/BFO_0000015"/>
        <rdfs:range>
            <owl:Class>
                <owl:unionOf rdf:parseType="Collection">
                    <rdf:Description rdf:about="http://purl.obolibrary.org/obo/BFO_0000020"/>
                    <rdf:Description rdf:about="http://purl.obolibrary.org/obo/BFO_0000031"/>
                    <owl:Class>
                        <owl:intersectionOf rdf:parseType="Collection">
                            <rdf:Description rdf:about="http://purl.obolibrary.org/obo/BFO_0000004"/>
                            <owl:Class>
                                <owl:complementOf rdf:resource="http://purl.obolibrary.org/obo/BFO_0000006"/>
                            </owl:Class>
                        </owl:intersectionOf>
                    </owl:Class>
                </owl:unionOf>
            </owl:Class>
        </rdfs:range>
        <dc:identifier>248-BFO</dc:identifier>
        <rdfs:label xml:lang="en">has participant</rdfs:label>
        <skos:definition xml:lang="en">p has participant c =Def c participates in p</skos:definition>
        <skos:scopeNote xml:lang="en">Users that require more sophisticated representations of time are encouraged to import a temporal extension of BFO-Core provided by the BFO development team. See documentation for guidance: &lt;Link&gt;</skos:scopeNote>
    </owl:ObjectProperty>
    


    <!-- http://purl.obolibrary.org/obo/BFO_0000058 -->


    <owl:ObjectProperty rdf:about="http://purl.obolibrary.org/obo/BFO_0000058">
        <owl:inverseOf rdf:resource="http://purl.obolibrary.org/obo/BFO_0000059"/>
        <rdfs:domain rdf:resource="http://purl.obolibrary.org/obo/BFO_0000031"/>
        <rdfs:range>
            <owl:Class>
                <owl:unionOf rdf:parseType="Collection">
                    <rdf:Description rdf:about="http://purl.obolibrary.org/obo/BFO_0000015"/>
                    <rdf:Description rdf:about="http://purl.obolibrary.org/obo/BFO_0000020"/>
                </owl:unionOf>
            </owl:Class>
        </rdfs:range>
        <dc:identifier>258-BFO</dc:identifier>
        <rdfs:label xml:lang="en">is concretized by</rdfs:label>
        <skos:definition xml:lang="en">c is concretized by b =Def b concretizes c</skos:definition>
        <skos:scopeNote xml:lang="en">Users that require more sophisticated representations of time are encouraged to import a temporal extension of BFO-Core provided by the BFO development team. See documentation for guidance: &lt;Link&gt;</skos:scopeNote>
    </owl:ObjectProperty>
    


    <!-- http://purl.obolibrary.org/obo/BFO_0000059 -->


    <owl:ObjectProperty rdf:about="http://purl.obolibrary.org/obo/BFO_0000059">
        <rdfs:domain>
            <owl:Class>
                <owl:unionOf rdf:parseType="Collection">
                    <rdf:Description rdf:about="http://purl.obolibrary.org/obo/BFO_0000015"/>
                    <rdf:Description rdf:about="http://purl.obolibrary.org/obo/BFO_0000020"/>
                </owl:unionOf>
            </owl:Class>
        </rdfs:domain>
        <rdfs:range rdf:resource="http://purl.obolibrary.org/obo/BFO_0000031"/>
        <dc:identifier>256-BFO</dc:identifier>
        <rdfs:label xml:lang="en">concretizes</rdfs:label>
        <skos:definition xml:lang="en">b concretizes c =Def b is a process or a specifically dependent continuant &amp; c is a generically dependent continuant &amp; there is some time t such that c is the pattern or content which b shares at t with actual or potential copies</skos:definition>
        <skos:scopeNote xml:lang="en">Users that require more sophisticated representations of time are encouraged to import a temporal extension of BFO-Core provided by the BFO development team. See documentation for guidance: &lt;Link&gt;</skos:scopeNote>
    </owl:ObjectProperty>
    


    <!-- http://purl.obolibrary.org/obo/BFO_0000062 -->


    <owl:ObjectProperty rdf:about="http://purl.obolibrary.org/obo/BFO_0000062">
        <owl:inverseOf rdf:resource="http://purl.obolibrary.org/obo/BFO_0000063"/>
        <rdf:type rdf:resource="http://www.w3.org/2002/07/owl#TransitiveProperty"/>
        <rdfs:domain rdf:resource="http://purl.obolibrary.org/obo/BFO_0000003"/>
        <rdfs:range rdf:resource="http://purl.obolibrary.org/obo/BFO_0000003"/>
        <dc:identifier>213-BFO</dc:identifier>
        <rdfs:label xml:lang="en">preceded by</rdfs:label>
        <skos:definition xml:lang="en">b preceded by c =Def b precedes c</skos:definition>
        <skos:example xml:lang="en">The temporal region occupied by the second half of the match is preceded by the temporal region occupied by the first half of the match</skos:example>
    </owl:ObjectProperty>
    


    <!-- http://purl.obolibrary.org/obo/BFO_0000063 -->


    <owl:ObjectProperty rdf:about="http://purl.obolibrary.org/obo/BFO_0000063">
        <rdf:type rdf:resource="http://www.w3.org/2002/07/owl#TransitiveProperty"/>
        <rdfs:domain rdf:resource="http://purl.obolibrary.org/obo/BFO_0000003"/>
        <rdfs:range rdf:resource="http://purl.obolibrary.org/obo/BFO_0000003"/>
        <dc:identifier>270-BFO</dc:identifier>
        <rdfs:label xml:lang="en">precedes</rdfs:label>
        <skos:definition xml:lang="en">(Elucidation) precedes is a relation between occurrents o, o&apos; such that if t is the temporal extent of o &amp; t&apos; is the temporal extent of o&apos; then either the last instant of o is before the first instant of o&apos; or the last instant of o is the first instant of o&apos; &amp; neither o nor o&apos; are temporal instants</skos:definition>
        <skos:example xml:lang="en">The temporal region occupied by Mary&apos;s birth precedes the temporal region occupied by Mary&apos;s death.</skos:example>
        <skos:scopeNote>Each temporal region is its own temporal extent. The temporal extent of a spatiotemporal region is the temporal region it temporally projects onto. The temporal extent of a process or process boundary that occupies temporal region t is t.</skos:scopeNote>
        <skos:scopeNote>Precedes defines a strict partial order on occurrents.</skos:scopeNote>
    </owl:ObjectProperty>
    


    <!-- http://purl.obolibrary.org/obo/BFO_0000066 -->


    <owl:ObjectProperty rdf:about="http://purl.obolibrary.org/obo/BFO_0000066">
        <owl:inverseOf rdf:resource="http://purl.obolibrary.org/obo/BFO_0000183"/>
        <rdfs:domain>
            <owl:Class>
                <owl:unionOf rdf:parseType="Collection">
                    <rdf:Description rdf:about="http://purl.obolibrary.org/obo/BFO_0000015"/>
                    <rdf:Description rdf:about="http://purl.obolibrary.org/obo/BFO_0000035"/>
                </owl:unionOf>
            </owl:Class>
        </rdfs:domain>
        <rdfs:range>
            <owl:Class>
                <owl:unionOf rdf:parseType="Collection">
                    <rdf:Description rdf:about="http://purl.obolibrary.org/obo/BFO_0000029"/>
                    <rdf:Description rdf:about="http://purl.obolibrary.org/obo/BFO_0000040"/>
                </owl:unionOf>
            </owl:Class>
        </rdfs:range>
        <dc:identifier>143-BFO</dc:identifier>
        <rdfs:label xml:lang="en">occurs in</rdfs:label>
        <skos:definition xml:lang="en">b occurs in c =Def b is a process or a process boundary &amp; c is a material entity or site &amp; there exists a spatiotemporal region r &amp; b occupies spatiotemporal region r &amp; for all time t, if b exists at t then c exists at t &amp; there exist spatial regions s and s&apos; where b spatially projects onto s at t &amp; c occupies spatial region s&apos; at t &amp; s is a continuant part of s&apos; at t</skos:definition>
        <skos:example xml:lang="en">A process of digestion occurs in the interior of an organism; a process of loading artillery rounds into a tank cannon occurs in the interior of the tank</skos:example>
    </owl:ObjectProperty>
    


    <!-- http://purl.obolibrary.org/obo/BFO_0000084 -->


    <owl:ObjectProperty rdf:about="http://purl.obolibrary.org/obo/BFO_0000084">
        <owl:inverseOf rdf:resource="http://purl.obolibrary.org/obo/BFO_0000101"/>
        <rdfs:domain rdf:resource="http://purl.obolibrary.org/obo/BFO_0000031"/>
        <rdfs:range>
            <owl:Class>
                <owl:intersectionOf rdf:parseType="Collection">
                    <rdf:Description rdf:about="http://purl.obolibrary.org/obo/BFO_0000004"/>
                    <owl:Class>
                        <owl:complementOf rdf:resource="http://purl.obolibrary.org/obo/BFO_0000006"/>
                    </owl:Class>
                </owl:intersectionOf>
            </owl:Class>
        </rdfs:range>
        <dc:identifier>252-BFO</dc:identifier>
        <rdfs:label xml:lang="en">generically depends on</rdfs:label>
        <skos:altLabel xml:lang="en">g-depends on</skos:altLabel>
        <skos:definition xml:lang="en">b generically depends on c =Def b is a generically dependent continuant &amp; c is an independent continuant that is not a spatial region &amp; at some time t there inheres in c a specifically dependent continuant which concretizes b at t</skos:definition>
        <skos:scopeNote xml:lang="en">Users that require more sophisticated representations of time are encouraged to import a temporal extension of BFO-Core provided by the BFO development team. See documentation for guidance: &lt;Link&gt;</skos:scopeNote>
    </owl:ObjectProperty>
    


    <!-- http://purl.obolibrary.org/obo/BFO_0000101 -->


    <owl:ObjectProperty rdf:about="http://purl.obolibrary.org/obo/BFO_0000101">
        <rdfs:domain>
            <owl:Class>
                <owl:intersectionOf rdf:parseType="Collection">
                    <rdf:Description rdf:about="http://purl.obolibrary.org/obo/BFO_0000004"/>
                    <owl:Class>
                        <owl:complementOf rdf:resource="http://purl.obolibrary.org/obo/BFO_0000006"/>
                    </owl:Class>
                </owl:intersectionOf>
            </owl:Class>
        </rdfs:domain>
        <rdfs:range rdf:resource="http://purl.obolibrary.org/obo/BFO_0000031"/>
        <dc:identifier>254-BFO</dc:identifier>
        <rdfs:label xml:lang="en">is carrier of</rdfs:label>
        <skos:definition xml:lang="en">b is carrier of c =Def there is some time t such that c generically depends on b at t</skos:definition>
        <skos:scopeNote xml:lang="en">Users that require more sophisticated representations of time are encouraged to import a temporal extension of BFO-Core provided by the BFO development team. See documentation for guidance: &lt;Link&gt;</skos:scopeNote>
    </owl:ObjectProperty>
    


    <!-- http://purl.obolibrary.org/obo/BFO_0000108 -->


    <owl:ObjectProperty rdf:about="http://purl.obolibrary.org/obo/BFO_0000108">
        <rdfs:domain rdf:resource="http://purl.obolibrary.org/obo/BFO_0000001"/>
        <rdfs:range rdf:resource="http://purl.obolibrary.org/obo/BFO_0000008"/>
        <dc:identifier>118-BFO</dc:identifier>
        <rdfs:label xml:lang="en">exists at</rdfs:label>
        <skos:definition xml:lang="en">(Elucidation) exists at is a relation between a particular and some temporal region at which the particular exists</skos:definition>
        <skos:example xml:lang="en">First World War exists at 1914-1916; Mexico exists at January 1, 2000</skos:example>
    </owl:ObjectProperty>
    


    <!-- http://purl.obolibrary.org/obo/BFO_0000115 -->


    <owl:ObjectProperty rdf:about="http://purl.obolibrary.org/obo/BFO_0000115">
        <rdfs:subPropertyOf rdf:resource="http://purl.obolibrary.org/obo/BFO_0000178"/>
        <owl:inverseOf rdf:resource="http://purl.obolibrary.org/obo/BFO_0000129"/>
        <rdfs:domain rdf:resource="http://purl.obolibrary.org/obo/BFO_0000040"/>
        <rdfs:range rdf:resource="http://purl.obolibrary.org/obo/BFO_0000040"/>
        <dc:identifier>230-BFO</dc:identifier>
        <rdfs:label xml:lang="en">has member part</rdfs:label>
        <skos:definition xml:lang="en">b has member part c =Def c member part of b</skos:definition>
        <skos:scopeNote xml:lang="en">Users that require more sophisticated representations of time are encouraged to import a temporal extension of BFO-Core provided by the BFO development team. See documentation for guidance: &lt;Link&gt;</skos:scopeNote>
    </owl:ObjectProperty>
    


    <!-- http://purl.obolibrary.org/obo/BFO_0000117 -->


    <owl:ObjectProperty rdf:about="http://purl.obolibrary.org/obo/BFO_0000117">
        <owl:inverseOf rdf:resource="http://purl.obolibrary.org/obo/BFO_0000132"/>
        <rdf:type rdf:resource="http://www.w3.org/2002/07/owl#TransitiveProperty"/>
        <rdfs:domain rdf:resource="http://purl.obolibrary.org/obo/BFO_0000003"/>
        <rdfs:range rdf:resource="http://purl.obolibrary.org/obo/BFO_0000003"/>
        <dc:identifier>202-BFO</dc:identifier>
        <rdfs:label xml:lang="en">has occurrent part</rdfs:label>
        <skos:definition xml:lang="en">b has occurrent part c =Def c occurrent part of b</skos:definition>
        <skos:example xml:lang="en">Mary&apos;s life has occurrent part Mary&apos;s 5th birthday</skos:example>
    </owl:ObjectProperty>
    


    <!-- http://purl.obolibrary.org/obo/BFO_0000121 -->


    <owl:ObjectProperty rdf:about="http://purl.obolibrary.org/obo/BFO_0000121">
        <rdfs:subPropertyOf rdf:resource="http://purl.obolibrary.org/obo/BFO_0000117"/>
        <owl:inverseOf rdf:resource="http://purl.obolibrary.org/obo/BFO_0000139"/>
        <rdf:type rdf:resource="http://www.w3.org/2002/07/owl#TransitiveProperty"/>
        <rdfs:domain rdf:resource="http://purl.obolibrary.org/obo/BFO_0000003"/>
        <rdfs:range rdf:resource="http://purl.obolibrary.org/obo/BFO_0000003"/>
        <dc:identifier>211-BFO</dc:identifier>
        <rdfs:label xml:lang="en">has temporal part</rdfs:label>
        <skos:definition xml:lang="en">b has temporal part c =Def c temporal part of b</skos:definition>
        <skos:example xml:lang="en">Your life has temporal part the first year of your life</skos:example>
    </owl:ObjectProperty>
    


    <!-- http://purl.obolibrary.org/obo/BFO_0000124 -->


    <owl:ObjectProperty rdf:about="http://purl.obolibrary.org/obo/BFO_0000124">
        <owl:inverseOf rdf:resource="http://purl.obolibrary.org/obo/BFO_0000171"/>
        <rdfs:domain>
            <owl:Class>
                <owl:intersectionOf rdf:parseType="Collection">
                    <rdf:Description rdf:about="http://purl.obolibrary.org/obo/BFO_0000004"/>
                    <owl:Class>
                        <owl:complementOf rdf:resource="http://purl.obolibrary.org/obo/BFO_0000006"/>
                    </owl:Class>
                </owl:intersectionOf>
            </owl:Class>
        </rdfs:domain>
        <rdfs:range>
            <owl:Class>
                <owl:intersectionOf rdf:parseType="Collection">
                    <rdf:Description rdf:about="http://purl.obolibrary.org/obo/BFO_0000004"/>
                    <owl:Class>
                        <owl:complementOf rdf:resource="http://purl.obolibrary.org/obo/BFO_0000006"/>
                    </owl:Class>
                </owl:intersectionOf>
            </owl:Class>
        </rdfs:range>
        <dc:identifier>236-BFO</dc:identifier>
        <rdfs:label xml:lang="en">location of</rdfs:label>
        <skos:definition xml:lang="en">b location of c =Def c located in b</skos:definition>
        <skos:scopeNote xml:lang="en">Users that require more sophisticated representations of time are encouraged to import a temporal extension of BFO-Core provided by the BFO development team. See documentation for guidance: &lt;Link&gt;</skos:scopeNote>
    </owl:ObjectProperty>
    


    <!-- http://purl.obolibrary.org/obo/BFO_0000127 -->


    <owl:ObjectProperty rdf:about="http://purl.obolibrary.org/obo/BFO_0000127">
        <owl:inverseOf rdf:resource="http://purl.obolibrary.org/obo/BFO_0000218"/>
        <rdfs:domain rdf:resource="http://purl.obolibrary.org/obo/BFO_0000040"/>
        <rdfs:range rdf:resource="http://purl.obolibrary.org/obo/BFO_0000016"/>
        <dc:identifier>244-BFO</dc:identifier>
        <rdfs:label xml:lang="en">material basis of</rdfs:label>
        <skos:definition xml:lang="en">b material basis of c =Def c has material basis b</skos:definition>
        <skos:scopeNote xml:lang="en">Users that require more sophisticated representations of time are encouraged to import a temporal extension of BFO-Core provided by the BFO development team. See documentation for guidance: &lt;Link&gt;</skos:scopeNote>
    </owl:ObjectProperty>
    


    <!-- http://purl.obolibrary.org/obo/BFO_0000129 -->


    <owl:ObjectProperty rdf:about="http://purl.obolibrary.org/obo/BFO_0000129">
        <rdfs:subPropertyOf rdf:resource="http://purl.obolibrary.org/obo/BFO_0000176"/>
        <rdfs:domain rdf:resource="http://purl.obolibrary.org/obo/BFO_0000040"/>
        <rdfs:range rdf:resource="http://purl.obolibrary.org/obo/BFO_0000040"/>
        <dc:identifier>228-BFO</dc:identifier>
        <rdfs:label xml:lang="en">member part of</rdfs:label>
        <skos:definition xml:lang="en">b member part of c =Def b is an object &amp; c is a material entity &amp; there is some time t such that b continuant part of c at t &amp; there is a mutually exhaustive and pairwise disjoint partition of c into objects x1, ..., xn (for some n ≠ 1) with b = xi (for some 1 &lt;= i &lt;= n)</skos:definition>
        <skos:scopeNote xml:lang="en">Users that require more sophisticated representations of time are encouraged to import a temporal extension of BFO-Core provided by the BFO development team. See documentation for guidance: &lt;Link&gt;</skos:scopeNote>
    </owl:ObjectProperty>
    


    <!-- http://purl.obolibrary.org/obo/BFO_0000132 -->


    <owl:ObjectProperty rdf:about="http://purl.obolibrary.org/obo/BFO_0000132">
        <rdf:type rdf:resource="http://www.w3.org/2002/07/owl#TransitiveProperty"/>
        <rdfs:domain rdf:resource="http://purl.obolibrary.org/obo/BFO_0000003"/>
        <rdfs:range rdf:resource="http://purl.obolibrary.org/obo/BFO_0000003"/>
        <dc:identifier>003-BFO</dc:identifier>
        <rdfs:label xml:lang="en">occurrent part of</rdfs:label>
        <skos:definition xml:lang="en">(Elucidation) occurrent part of is a relation between occurrents b and c when b is part of c</skos:definition>
        <skos:example xml:lang="en">Mary&apos;s 5th birthday is an occurrent part of Mary&apos;s life; the first set of the tennis match is an occurrent part of the tennis match</skos:example>
    </owl:ObjectProperty>
    


    <!-- http://purl.obolibrary.org/obo/BFO_0000139 -->


    <owl:ObjectProperty rdf:about="http://purl.obolibrary.org/obo/BFO_0000139">
        <rdfs:subPropertyOf rdf:resource="http://purl.obolibrary.org/obo/BFO_0000132"/>
        <rdf:type rdf:resource="http://www.w3.org/2002/07/owl#TransitiveProperty"/>
        <rdfs:domain rdf:resource="http://purl.obolibrary.org/obo/BFO_0000003"/>
        <rdfs:range rdf:resource="http://purl.obolibrary.org/obo/BFO_0000003"/>
        <dc:identifier>078-BFO</dc:identifier>
        <rdfs:label xml:lang="en">temporal part of</rdfs:label>
        <skos:definition xml:lang="en">b temporal part of c =Def b occurrent part of c &amp; (b and c are temporal regions) or (b and c are spatiotemporal regions &amp; b temporally projects onto an occurrent part of the temporal region that c temporally projects onto) or (b and c are processes or process boundaries &amp; b occupies a temporal region that is an occurrent part of the temporal region that c occupies)</skos:definition>
        <skos:example xml:lang="en">Your heart beating from 4pm to 5pm today is a temporal part of the process of your heart beating; the 4th year of your life is a temporal part of your life, as is the process boundary which separates the 3rd and 4th years of your life; the first quarter of a game of football is a temporal part of the whole game</skos:example>
    </owl:ObjectProperty>
    


    <!-- http://purl.obolibrary.org/obo/BFO_0000153 -->


    <owl:ObjectProperty rdf:about="http://purl.obolibrary.org/obo/BFO_0000153">
        <rdf:type rdf:resource="http://www.w3.org/2002/07/owl#FunctionalProperty"/>
        <rdfs:domain rdf:resource="http://purl.obolibrary.org/obo/BFO_0000011"/>
        <rdfs:range rdf:resource="http://purl.obolibrary.org/obo/BFO_0000008"/>
        <dc:identifier>080-BFO</dc:identifier>
        <rdfs:label xml:lang="en">temporally projects onto</rdfs:label>
        <skos:definition xml:lang="en">(Elucidation) temporally projects onto is a relation between a spatiotemporal region s and some temporal region which is the temporal extent of s</skos:definition>
        <skos:example xml:lang="en">The world line of a particle temporally projects onto the temporal region extending from the beginning to the end of the existence of the particle</skos:example>
    </owl:ObjectProperty>
    


    <!-- http://purl.obolibrary.org/obo/BFO_0000171 -->


    <owl:ObjectProperty rdf:about="http://purl.obolibrary.org/obo/BFO_0000171">
        <rdfs:domain>
            <owl:Class>
                <owl:intersectionOf rdf:parseType="Collection">
                    <rdf:Description rdf:about="http://purl.obolibrary.org/obo/BFO_0000004"/>
                    <owl:Class>
                        <owl:complementOf rdf:resource="http://purl.obolibrary.org/obo/BFO_0000006"/>
                    </owl:Class>
                </owl:intersectionOf>
            </owl:Class>
        </rdfs:domain>
        <rdfs:range>
            <owl:Class>
                <owl:intersectionOf rdf:parseType="Collection">
                    <rdf:Description rdf:about="http://purl.obolibrary.org/obo/BFO_0000004"/>
                    <owl:Class>
                        <owl:complementOf rdf:resource="http://purl.obolibrary.org/obo/BFO_0000006"/>
                    </owl:Class>
                </owl:intersectionOf>
            </owl:Class>
        </rdfs:range>
        <dc:identifier>234-BFO</dc:identifier>
        <rdfs:label xml:lang="en">located in</rdfs:label>
        <skos:definition xml:lang="en">b located in c =Def b is an independent continuant &amp; c is an independent &amp; neither is a spatial region &amp; there is some time t such that the spatial region which b occupies at t is continuant part of the spatial region which c occupies at t</skos:definition>
        <skos:scopeNote xml:lang="en">Users that require more sophisticated representations of time are encouraged to import a temporal extension of BFO-Core provided by the BFO development team. See documentation for guidance: &lt;Link&gt;</skos:scopeNote>
    </owl:ObjectProperty>
    


    <!-- http://purl.obolibrary.org/obo/BFO_0000176 -->


    <owl:ObjectProperty rdf:about="http://purl.obolibrary.org/obo/BFO_0000176">
        <owl:inverseOf rdf:resource="http://purl.obolibrary.org/obo/BFO_0000178"/>
        <rdfs:domain rdf:resource="http://purl.obolibrary.org/obo/BFO_0000002"/>
        <rdfs:range rdf:resource="http://purl.obolibrary.org/obo/BFO_0000002"/>
        <dc:identifier>221-BFO</dc:identifier>
        <rdfs:label xml:lang="en">continuant part of</rdfs:label>
        <skos:definition xml:lang="en">b continuant part of c =Def b and c are continuants &amp; there is some time t such that b and c exist at t &amp; b continuant part of c at t</skos:definition>
        <skos:example xml:lang="en">Milk teeth continuant part of human; surgically removed tumour continuant part of organism</skos:example>
        <skos:scopeNote xml:lang="en">Users that require more sophisticated representations of time are encouraged to import a temporal extension of BFO-Core provided by the BFO development team. See documentation for guidance: &lt;Link&gt;</skos:scopeNote>
    </owl:ObjectProperty>
    


    <!-- http://purl.obolibrary.org/obo/BFO_0000178 -->


    <owl:ObjectProperty rdf:about="http://purl.obolibrary.org/obo/BFO_0000178">
        <rdfs:domain rdf:resource="http://purl.obolibrary.org/obo/BFO_0000002"/>
        <rdfs:range rdf:resource="http://purl.obolibrary.org/obo/BFO_0000002"/>
        <dc:identifier>271-BFO</dc:identifier>
        <rdfs:label xml:lang="en">has continuant part</rdfs:label>
        <skos:definition xml:lang="en">b has continuant part c =Def c continuant part of b</skos:definition>
        <skos:scopeNote xml:lang="en">Users that require more sophisticated representations of time are encouraged to import a temporal extension of BFO-Core provided by the BFO development team. See documentation for guidance: &lt;Link&gt;</skos:scopeNote>
    </owl:ObjectProperty>
    


    <!-- http://purl.obolibrary.org/obo/BFO_0000183 -->


    <owl:ObjectProperty rdf:about="http://purl.obolibrary.org/obo/BFO_0000183">
        <rdfs:domain>
            <owl:Class>
                <owl:unionOf rdf:parseType="Collection">
                    <rdf:Description rdf:about="http://purl.obolibrary.org/obo/BFO_0000029"/>
                    <rdf:Description rdf:about="http://purl.obolibrary.org/obo/BFO_0000040"/>
                </owl:unionOf>
            </owl:Class>
        </rdfs:domain>
        <rdfs:range>
            <owl:Class>
                <owl:unionOf rdf:parseType="Collection">
                    <rdf:Description rdf:about="http://purl.obolibrary.org/obo/BFO_0000015"/>
                    <rdf:Description rdf:about="http://purl.obolibrary.org/obo/BFO_0000035"/>
                </owl:unionOf>
            </owl:Class>
        </rdfs:range>
        <dc:identifier>267-BFO</dc:identifier>
        <rdfs:label xml:lang="en">environs</rdfs:label>
        <skos:altLabel xml:lang="en">contains process</skos:altLabel>
        <skos:definition xml:lang="en">b environs c =Def c occurs in b</skos:definition>
        <skos:example xml:lang="en">Mouth environs process of mastication; city environs traffic</skos:example>
    </owl:ObjectProperty>
    


    <!-- http://purl.obolibrary.org/obo/BFO_0000184 -->


    <owl:ObjectProperty rdf:about="http://purl.obolibrary.org/obo/BFO_0000184">
        <owl:inverseOf rdf:resource="http://purl.obolibrary.org/obo/BFO_0000185"/>
        <rdf:type rdf:resource="http://www.w3.org/2002/07/owl#FunctionalProperty"/>
        <rdf:type rdf:resource="http://www.w3.org/2002/07/owl#InverseFunctionalProperty"/>
        <rdfs:domain rdf:resource="http://purl.obolibrary.org/obo/BFO_0000182"/>
        <rdfs:range rdf:resource="http://purl.obolibrary.org/obo/BFO_0000040"/>
        <dc:identifier>144-BFO</dc:identifier>
        <rdfs:label xml:lang="en">history of</rdfs:label>
        <skos:definition xml:lang="en">(Elucidation) history of is a relation between history b and material entity c such that b is the unique history of c</skos:definition>
        <skos:example xml:lang="en">This life is the history of this organism</skos:example>
    </owl:ObjectProperty>
    


    <!-- http://purl.obolibrary.org/obo/BFO_0000185 -->


    <owl:ObjectProperty rdf:about="http://purl.obolibrary.org/obo/BFO_0000185">
        <rdfs:domain rdf:resource="http://purl.obolibrary.org/obo/BFO_0000040"/>
        <rdfs:range rdf:resource="http://purl.obolibrary.org/obo/BFO_0000182"/>
        <dc:identifier>145-BFO</dc:identifier>
        <rdfs:label xml:lang="en">has history</rdfs:label>
        <skos:definition xml:lang="en">b has history c =Def c history of b</skos:definition>
        <skos:example xml:lang="en">This organism has history this life</skos:example>
    </owl:ObjectProperty>
    


    <!-- http://purl.obolibrary.org/obo/BFO_0000194 -->


    <owl:ObjectProperty rdf:about="http://purl.obolibrary.org/obo/BFO_0000194">
        <owl:inverseOf rdf:resource="http://purl.obolibrary.org/obo/BFO_0000195"/>
        <rdfs:domain>
            <owl:Class>
                <owl:unionOf rdf:parseType="Collection">
                    <rdf:Description rdf:about="http://purl.obolibrary.org/obo/BFO_0000020"/>
                    <owl:Class>
                        <owl:intersectionOf rdf:parseType="Collection">
                            <rdf:Description rdf:about="http://purl.obolibrary.org/obo/BFO_0000004"/>
                            <owl:Class>
                                <owl:complementOf rdf:resource="http://purl.obolibrary.org/obo/BFO_0000006"/>
                            </owl:Class>
                        </owl:intersectionOf>
                    </owl:Class>
                </owl:unionOf>
            </owl:Class>
        </rdfs:domain>
        <rdfs:range rdf:resource="http://purl.obolibrary.org/obo/BFO_0000020"/>
        <dc:identifier>260-BFO</dc:identifier>
        <rdfs:label xml:lang="en">specifically depended on by</rdfs:label>
        <skos:altLabel xml:lang="en">s-depended on by</skos:altLabel>
        <skos:definition xml:lang="en">b specifically depended on by c =Def c specifically depends on b</skos:definition>
        <skos:example xml:lang="en">Coloured object specifically depended on by colour</skos:example>
    </owl:ObjectProperty>
    


    <!-- http://purl.obolibrary.org/obo/BFO_0000195 -->


    <owl:ObjectProperty rdf:about="http://purl.obolibrary.org/obo/BFO_0000195">
        <rdfs:domain rdf:resource="http://purl.obolibrary.org/obo/BFO_0000020"/>
        <rdfs:range>
            <owl:Class>
                <owl:unionOf rdf:parseType="Collection">
                    <rdf:Description rdf:about="http://purl.obolibrary.org/obo/BFO_0000020"/>
                    <owl:Class>
                        <owl:intersectionOf rdf:parseType="Collection">
                            <rdf:Description rdf:about="http://purl.obolibrary.org/obo/BFO_0000004"/>
                            <owl:Class>
                                <owl:complementOf rdf:resource="http://purl.obolibrary.org/obo/BFO_0000006"/>
                            </owl:Class>
                        </owl:intersectionOf>
                    </owl:Class>
                </owl:unionOf>
            </owl:Class>
        </rdfs:range>
        <dc:identifier>012-BFO</dc:identifier>
        <rdfs:label xml:lang="en">specifically depends on</rdfs:label>
        <skos:altLabel xml:lang="en">s-depends on</skos:altLabel>
        <skos:definition xml:lang="en">(Elucidation) specifically depends on is a relation between a specifically dependent continuant b and specifically dependent continuant or independent continuant that is not a spatial region c such that b and c share no parts in common &amp; b is of a nature such that at all times t it cannot exist unless c exists &amp; b is not a boundary of c</skos:definition>
        <skos:example xml:lang="en">A shape specifically depends on the shaped object; hue, saturation and brightness of a colour sample specifically depends on each other</skos:example>
        <skos:scopeNote xml:lang="en">The analogue of specifically depends on for occurrents is has participant.</skos:scopeNote>
    </owl:ObjectProperty>
    


    <!-- http://purl.obolibrary.org/obo/BFO_0000196 -->


    <owl:ObjectProperty rdf:about="http://purl.obolibrary.org/obo/BFO_0000196">
        <rdfs:subPropertyOf rdf:resource="http://purl.obolibrary.org/obo/BFO_0000194"/>
        <owl:inverseOf rdf:resource="http://purl.obolibrary.org/obo/BFO_0000197"/>
        <rdfs:domain>
            <owl:Class>
                <owl:intersectionOf rdf:parseType="Collection">
                    <rdf:Description rdf:about="http://purl.obolibrary.org/obo/BFO_0000004"/>
                    <owl:Class>
                        <owl:complementOf rdf:resource="http://purl.obolibrary.org/obo/BFO_0000006"/>
                    </owl:Class>
                </owl:intersectionOf>
            </owl:Class>
        </rdfs:domain>
        <rdfs:range rdf:resource="http://purl.obolibrary.org/obo/BFO_0000020"/>
        <dc:identifier>053-BFO</dc:identifier>
        <rdfs:label xml:lang="en">bearer of</rdfs:label>
        <skos:definition xml:lang="en">b bearer of c =Def c inheres in b</skos:definition>
        <skos:example xml:lang="en">A patch of ink is the bearer of a colour quality; an organism is the bearer of a temperature quality</skos:example>
    </owl:ObjectProperty>
    


    <!-- http://purl.obolibrary.org/obo/BFO_0000197 -->


    <owl:ObjectProperty rdf:about="http://purl.obolibrary.org/obo/BFO_0000197">
        <rdfs:subPropertyOf rdf:resource="http://purl.obolibrary.org/obo/BFO_0000195"/>
        <rdfs:domain rdf:resource="http://purl.obolibrary.org/obo/BFO_0000020"/>
        <rdfs:range>
            <owl:Class>
                <owl:intersectionOf rdf:parseType="Collection">
                    <rdf:Description rdf:about="http://purl.obolibrary.org/obo/BFO_0000004"/>
                    <owl:Class>
                        <owl:complementOf rdf:resource="http://purl.obolibrary.org/obo/BFO_0000006"/>
                    </owl:Class>
                </owl:intersectionOf>
            </owl:Class>
        </rdfs:range>
        <dc:identifier>051-BFO</dc:identifier>
        <rdfs:label xml:lang="en">inheres in</rdfs:label>
        <skos:definition xml:lang="en">b inheres in c =Def b is a specifically dependent continuant &amp; c is an independent continuant that is not a spatial region &amp; b specifically depends on c</skos:definition>
        <skos:example xml:lang="en">A shape inheres in a shaped object; a mass inheres in a material entity</skos:example>
    </owl:ObjectProperty>
    


    <!-- http://purl.obolibrary.org/obo/BFO_0000199 -->


    <owl:ObjectProperty rdf:about="http://purl.obolibrary.org/obo/BFO_0000199">
        <rdf:type rdf:resource="http://www.w3.org/2002/07/owl#FunctionalProperty"/>
        <rdfs:domain>
            <owl:Class>
                <owl:unionOf rdf:parseType="Collection">
                    <rdf:Description rdf:about="http://purl.obolibrary.org/obo/BFO_0000015"/>
                    <rdf:Description rdf:about="http://purl.obolibrary.org/obo/BFO_0000035"/>
                </owl:unionOf>
            </owl:Class>
        </rdfs:domain>
        <rdfs:range rdf:resource="http://purl.obolibrary.org/obo/BFO_0000008"/>
        <dc:identifier>132-BFO</dc:identifier>
        <rdfs:label xml:lang="en">occupies temporal region</rdfs:label>
        <skos:definition xml:lang="en">p occupies temporal region t =Def p is a process or process boundary &amp; the spatiotemporal region occupied by p temporally projects onto t</skos:definition>
        <skos:example xml:lang="en">The Second World War occupies the temporal region September 1, 1939 - September 2, 1945</skos:example>
    </owl:ObjectProperty>
    


    <!-- http://purl.obolibrary.org/obo/BFO_0000200 -->


    <owl:ObjectProperty rdf:about="http://purl.obolibrary.org/obo/BFO_0000200">
        <rdf:type rdf:resource="http://www.w3.org/2002/07/owl#FunctionalProperty"/>
        <rdfs:domain>
            <owl:Class>
                <owl:unionOf rdf:parseType="Collection">
                    <rdf:Description rdf:about="http://purl.obolibrary.org/obo/BFO_0000015"/>
                    <rdf:Description rdf:about="http://purl.obolibrary.org/obo/BFO_0000035"/>
                </owl:unionOf>
            </owl:Class>
        </rdfs:domain>
        <rdfs:range rdf:resource="http://purl.obolibrary.org/obo/BFO_0000011"/>
        <dc:identifier>082-BFO</dc:identifier>
        <rdfs:label xml:lang="en">occupies spatiotemporal region</rdfs:label>
        <skos:definition xml:lang="en">(Elucidation) occupies spatiotemporal region is a relation between a process or process boundary p and the spatiotemporal region s which is its spatiotemporal extent</skos:definition>
        <skos:example xml:lang="en">A particle emitted by a nuclear reactor occupies the spatiotemporal region which is its trajectory</skos:example>
    </owl:ObjectProperty>
    


    <!-- http://purl.obolibrary.org/obo/BFO_0000210 -->


    <owl:ObjectProperty rdf:about="http://purl.obolibrary.org/obo/BFO_0000210">
        <rdfs:domain>
            <owl:Class>
                <owl:intersectionOf rdf:parseType="Collection">
                    <rdf:Description rdf:about="http://purl.obolibrary.org/obo/BFO_0000004"/>
                    <owl:Class>
                        <owl:complementOf rdf:resource="http://purl.obolibrary.org/obo/BFO_0000006"/>
                    </owl:Class>
                </owl:intersectionOf>
            </owl:Class>
        </rdfs:domain>
        <rdfs:range rdf:resource="http://purl.obolibrary.org/obo/BFO_0000006"/>
        <dc:identifier>232-BFO</dc:identifier>
        <rdfs:label xml:lang="en">occupies spatial region</rdfs:label>
        <skos:definition xml:lang="en">b occupies spatial region r =Def b is an independent continuant that is not a spatial region &amp; r is a spatial region &amp; there is some time t such that every continuant part of b occupies some continuant part of r at t and no continuant part of b occupies any spatial region that is not a continuant part of r at t</skos:definition>
        <skos:scopeNote xml:lang="en">Users that require more sophisticated representations of time are encouraged to import a temporal extension of BFO-Core provided by the BFO development team. See documentation for guidance: &lt;Link&gt;</skos:scopeNote>
    </owl:ObjectProperty>
    


    <!-- http://purl.obolibrary.org/obo/BFO_0000216 -->


    <owl:ObjectProperty rdf:about="http://purl.obolibrary.org/obo/BFO_0000216">
        <rdfs:domain rdf:resource="http://purl.obolibrary.org/obo/BFO_0000011"/>
        <rdfs:range rdf:resource="http://purl.obolibrary.org/obo/BFO_0000006"/>
        <dc:identifier>246-BFO</dc:identifier>
        <rdfs:label xml:lang="en">spatially projects onto</rdfs:label>
        <skos:definition xml:lang="en">(Elucidation) spatially projects onto is a relation between some spatiotemporal region b and spatial region c such that at some time t, c is the spatial extent of b at t</skos:definition>
        <skos:scopeNote xml:lang="en">Users that require more sophisticated representations of time are encouraged to import a temporal extension of BFO-Core provided by the BFO development team. See documentation for guidance: &lt;Link&gt;</skos:scopeNote>
    </owl:ObjectProperty>
    


    <!-- http://purl.obolibrary.org/obo/BFO_0000218 -->


    <owl:ObjectProperty rdf:about="http://purl.obolibrary.org/obo/BFO_0000218">
        <rdfs:domain rdf:resource="http://purl.obolibrary.org/obo/BFO_0000016"/>
        <rdfs:range rdf:resource="http://purl.obolibrary.org/obo/BFO_0000040"/>
        <dc:identifier>242-BFO</dc:identifier>
        <rdfs:label xml:lang="en">has material basis</rdfs:label>
        <skos:definition xml:lang="en">b has material basis c =Def b is a disposition &amp; c is a material entity &amp; there is some d bearer of b &amp; there is some time t such that c is a continuant part of d at t &amp; d has disposition b because c is a continuant part of d at t</skos:definition>
        <skos:scopeNote xml:lang="en">Users that require more sophisticated representations of time are encouraged to import a temporal extension of BFO-Core provided by the BFO development team. See documentation for guidance: &lt;Link&gt;</skos:scopeNote>
    </owl:ObjectProperty>
    


    <!-- http://purl.obolibrary.org/obo/BFO_0000221 -->


    <owl:ObjectProperty rdf:about="http://purl.obolibrary.org/obo/BFO_0000221">
        <owl:inverseOf rdf:resource="http://purl.obolibrary.org/obo/BFO_0000222"/>
        <rdfs:domain rdf:resource="http://purl.obolibrary.org/obo/BFO_0000203"/>
        <rdfs:range rdf:resource="http://purl.obolibrary.org/obo/BFO_0000008"/>
        <dc:identifier>268-BFO</dc:identifier>
        <rdfs:label xml:lang="en">first instant of</rdfs:label>
        <skos:definition xml:lang="en">t first instant of t&apos; =Def t is a temporal instant &amp; t&apos; is a temporal region t&apos; &amp; t precedes all temporal parts of t&apos; other than t</skos:definition>
        <skos:example xml:lang="en">An hour starting at midnight yesterday has first instant midnight yesterday</skos:example>
    </owl:ObjectProperty>
    


    <!-- http://purl.obolibrary.org/obo/BFO_0000222 -->


    <owl:ObjectProperty rdf:about="http://purl.obolibrary.org/obo/BFO_0000222">
        <rdf:type rdf:resource="http://www.w3.org/2002/07/owl#FunctionalProperty"/>
        <rdfs:domain rdf:resource="http://purl.obolibrary.org/obo/BFO_0000008"/>
        <rdfs:range rdf:resource="http://purl.obolibrary.org/obo/BFO_0000203"/>
        <dc:identifier>261-BFO</dc:identifier>
        <rdfs:label xml:lang="en">has first instant</rdfs:label>
        <skos:definition xml:lang="en">t has first instant t&apos; =Def t&apos; first instant of t</skos:definition>
        <skos:example xml:lang="en">The first hour of a year has first instant midnight on December 31</skos:example>
    </owl:ObjectProperty>
    


    <!-- http://purl.obolibrary.org/obo/BFO_0000223 -->


    <owl:ObjectProperty rdf:about="http://purl.obolibrary.org/obo/BFO_0000223">
        <owl:inverseOf rdf:resource="http://purl.obolibrary.org/obo/BFO_0000224"/>
        <rdfs:domain rdf:resource="http://purl.obolibrary.org/obo/BFO_0000203"/>
        <rdfs:range rdf:resource="http://purl.obolibrary.org/obo/BFO_0000008"/>
        <dc:identifier>269-BFO</dc:identifier>
        <rdfs:label xml:lang="en">last instant of</rdfs:label>
        <skos:definition xml:lang="en">t last instant of t&apos; =Def t is a temporal instant &amp; t&apos; is a temporal region &amp; all temporal parts of t&apos; other than t precede t</skos:definition>
        <skos:example xml:lang="en">Last midnight is the last instant of yesterday</skos:example>
    </owl:ObjectProperty>
    


    <!-- http://purl.obolibrary.org/obo/BFO_0000224 -->


    <owl:ObjectProperty rdf:about="http://purl.obolibrary.org/obo/BFO_0000224">
        <rdf:type rdf:resource="http://www.w3.org/2002/07/owl#FunctionalProperty"/>
        <rdfs:domain rdf:resource="http://purl.obolibrary.org/obo/BFO_0000008"/>
        <rdfs:range rdf:resource="http://purl.obolibrary.org/obo/BFO_0000203"/>
        <dc:identifier>215-BFO</dc:identifier>
        <rdfs:label xml:lang="en">has last instant</rdfs:label>
        <skos:definition xml:lang="en">t has last instant t&apos; =Def t&apos; last instant of t</skos:definition>
        <skos:example xml:lang="en">The last hour of a year has last instant midnight December 31</skos:example>
    </owl:ObjectProperty>
    


    <!-- http://web-development-ontology.netlify.app/wdo#accesses -->


    <owl:ObjectProperty rdf:about="http://web-development-ontology.netlify.app/wdo#accesses">
        <owl:inverseOf rdf:resource="http://web-development-ontology.netlify.app/wdo#isAccessedBy"/>
        <rdfs:domain rdf:resource="http://web-development-ontology.netlify.app/wdo#FunctionDefinition"/>
        <rdfs:range>
            <owl:Class>
                <owl:unionOf rdf:parseType="Collection">
                    <rdf:Description rdf:about="http://web-development-ontology.netlify.app/wdo#AttributeDeclaration"/>
                    <rdf:Description rdf:about="http://web-development-ontology.netlify.app/wdo#VariableDeclaration"/>
                </owl:unionOf>
            </owl:Class>
        </rdfs:range>
        <dc:identifier>WDO_OP:0000021</dc:identifier>
        <rdfs:label xml:lang="en">accesses</rdfs:label>
        <skos:definition xml:lang="en">A relation indicating that a function or method reads from or writes to a variable, attribute, or field.</skos:definition>
    </owl:ObjectProperty>
    


    <!-- http://web-development-ontology.netlify.app/wdo#addressesIssue -->


    <owl:ObjectProperty rdf:about="http://web-development-ontology.netlify.app/wdo#addressesIssue">
        <owl:inverseOf rdf:resource="http://web-development-ontology.netlify.app/wdo#isAddressedBy"/>
        <rdfs:domain rdf:resource="http://web-development-ontology.netlify.app/wdo#Commit"/>
        <rdfs:range rdf:resource="http://web-development-ontology.netlify.app/wdo#Issue"/>
        <dc:identifier>WDO_OP:0000042</dc:identifier>
        <rdfs:label xml:lang="en">addresses issue</rdfs:label>
        <skos:definition xml:lang="en">A relation that links a commit to an issue it makes progress on or is related to.</skos:definition>
    </owl:ObjectProperty>
    


    <!-- http://web-development-ontology.netlify.app/wdo#bearerOfInformation -->


    <owl:ObjectProperty rdf:about="http://web-development-ontology.netlify.app/wdo#bearerOfInformation">
        <owl:inverseOf rdf:resource="http://web-development-ontology.netlify.app/wdo#informationBorneBy"/>
        <rdfs:domain rdf:resource="http://web-development-ontology.netlify.app/wdo#DigitalInformationCarrier"/>
        <rdfs:range rdf:resource="http://web-development-ontology.netlify.app/wdo#InformationContentEntity"/>
        <dc:identifier>WDO_OP:0000001</dc:identifier>
        <rdfs:label xml:lang="en">bearer of information</rdfs:label>
        <skos:definition xml:lang="en">A relation between a digital information carrier (e.g., a file) and the information content entity it encodes or represents.</skos:definition>
    </owl:ObjectProperty>
    


    <!-- http://web-development-ontology.netlify.app/wdo#callsFunction -->


    <owl:ObjectProperty rdf:about="http://web-development-ontology.netlify.app/wdo#callsFunction">
        <rdfs:subPropertyOf rdf:resource="http://web-development-ontology.netlify.app/wdo#invokes"/>
        <owl:inverseOf rdf:resource="http://web-development-ontology.netlify.app/wdo#isCalledByFunctionAt"/>
        <rdfs:domain rdf:resource="http://web-development-ontology.netlify.app/wdo#FunctionCallSite"/>
        <rdfs:range rdf:resource="http://web-development-ontology.netlify.app/wdo#FunctionDefinition"/>
        <dc:identifier>WDO_OP:0000033</dc:identifier>
        <rdfs:label xml:lang="en">calls function</rdfs:label>
        <skos:definition xml:lang="en">A specific relation between a single FunctionCallSite and the FunctionDefinition it invokes.</skos:definition>
    </owl:ObjectProperty>
    


    <!-- http://web-development-ontology.netlify.app/wdo#committed -->


    <owl:ObjectProperty rdf:about="http://web-development-ontology.netlify.app/wdo#committed">
        <owl:inverseOf rdf:resource="http://web-development-ontology.netlify.app/wdo#committedBy"/>
        <rdfs:domain rdf:resource="http://xmlns.com/foaf/0.1/Person"/>
        <rdfs:range rdf:resource="http://web-development-ontology.netlify.app/wdo#Commit"/>
        <dc:identifier>WDO_OP:0000121</dc:identifier>
        <rdfs:label xml:lang="en">committed</rdfs:label>
        <skos:definition xml:lang="en">A relation linking a person to the commits they have performed as committer.</skos:definition>
    </owl:ObjectProperty>
    


    <!-- http://web-development-ontology.netlify.app/wdo#committedBy -->


    <owl:ObjectProperty rdf:about="http://web-development-ontology.netlify.app/wdo#committedBy">
        <rdfs:domain rdf:resource="http://web-development-ontology.netlify.app/wdo#Commit"/>
        <rdfs:range rdf:resource="http://xmlns.com/foaf/0.1/Person"/>
        <dc:identifier>WDO_OP:0000120</dc:identifier>
        <rdfs:label xml:lang="en">committed by</rdfs:label>
        <skos:definition xml:lang="en">A relation linking a commit to the person who performed the commit operation (committer in Git).</skos:definition>
    </owl:ObjectProperty>
    


    <!-- http://web-development-ontology.netlify.app/wdo#compiles -->


    <owl:ObjectProperty rdf:about="http://web-development-ontology.netlify.app/wdo#compiles">
        <owl:inverseOf rdf:resource="http://web-development-ontology.netlify.app/wdo#isCompiledBy"/>
        <rdfs:domain rdf:resource="http://web-development-ontology.netlify.app/wdo#BuildScript"/>
        <rdfs:range rdf:resource="http://web-development-ontology.netlify.app/wdo#SourceCodeFile"/>
        <dc:identifier>WDO_OP:0000045</dc:identifier>
        <rdfs:label xml:lang="en">compiles</rdfs:label>
        <skos:definition xml:lang="en">A relation from a build script to the source code files it processes during compilation.</skos:definition>
    </owl:ObjectProperty>
    


    <!-- http://web-development-ontology.netlify.app/wdo#conformsToGuideline -->


    <owl:ObjectProperty rdf:about="http://web-development-ontology.netlify.app/wdo#conformsToGuideline">
        <owl:inverseOf rdf:resource="http://web-development-ontology.netlify.app/wdo#isGuidelineFor"/>
        <rdfs:domain rdf:resource="http://purl.obolibrary.org/obo/BFO_0000001"/>
        <rdfs:range rdf:resource="http://web-development-ontology.netlify.app/wdo#BestPracticeGuideline"/>
        <dc:identifier>WDO_OP:0000006</dc:identifier>
        <rdfs:label xml:lang="en">conforms to guideline</rdfs:label>
        <skos:definition xml:lang="en">A relation indicating that an entity (e.g., SoftwareCode, a process) adheres to a BestPracticeGuideline.</skos:definition>
    </owl:ObjectProperty>
    


    <!-- http://web-development-ontology.netlify.app/wdo#contributesTo -->


    <owl:ObjectProperty rdf:about="http://web-development-ontology.netlify.app/wdo#contributesTo">
        <owl:inverseOf rdf:resource="http://web-development-ontology.netlify.app/wdo#hasContributor"/>
        <rdfs:domain rdf:resource="http://xmlns.com/foaf/0.1/Person"/>
        <rdfs:range rdf:resource="http://web-development-ontology.netlify.app/wdo#Repository"/>
        <dc:identifier>WDO_OP:0000124</dc:identifier>
        <rdfs:label xml:lang="en">contributes to</rdfs:label>
        <skos:definition xml:lang="en">A relation linking a person to a repository or project they have contributed to in any capacity.</skos:definition>
    </owl:ObjectProperty>
    


    <!-- http://web-development-ontology.netlify.app/wdo#declares -->


    <owl:ObjectProperty rdf:about="http://web-development-ontology.netlify.app/wdo#declares">
        <rdfs:subPropertyOf rdf:resource="http://purl.obolibrary.org/obo/BFO_0000178"/>
        <owl:inverseOf rdf:resource="http://web-development-ontology.netlify.app/wdo#isDeclaredBy"/>
        <rdfs:domain rdf:resource="http://web-development-ontology.netlify.app/wdo#SoftwareCode"/>
        <rdfs:range rdf:resource="http://web-development-ontology.netlify.app/wdo#CodeConstruct"/>
        <dc:identifier>WDO_OP:0000007</dc:identifier>
        <rdfs:label xml:lang="en">declares</rdfs:label>
        <skos:definition xml:lang="en">A general relation indicating that a code entity (like a class or module) declares a smaller code construct (like a method or attribute) as one of its parts.</skos:definition>
    </owl:ObjectProperty>
    


    <!-- http://web-development-ontology.netlify.app/wdo#documentsEntity -->


    <owl:ObjectProperty rdf:about="http://web-development-ontology.netlify.app/wdo#documentsEntity">
        <owl:inverseOf rdf:resource="http://web-development-ontology.netlify.app/wdo#isDocumentedBy"/>
        <rdfs:domain rdf:resource="http://web-development-ontology.netlify.app/wdo#Documentation"/>
        <rdfs:range rdf:resource="http://purl.obolibrary.org/obo/BFO_0000001"/>
        <dc:identifier>WDO_OP:0000004</dc:identifier>
        <rdfs:label xml:lang="en">documents entity</rdfs:label>
        <skos:definition xml:lang="en">A relation between a Documentation entity and the entity it describes or explains.</skos:definition>
    </owl:ObjectProperty>
    


    <!-- http://web-development-ontology.netlify.app/wdo#embedsCode -->


    <owl:ObjectProperty rdf:about="http://web-development-ontology.netlify.app/wdo#embedsCode">
        <owl:inverseOf rdf:resource="http://web-development-ontology.netlify.app/wdo#isEmbeddedIn"/>
        <rdfs:domain rdf:resource="http://web-development-ontology.netlify.app/wdo#Template"/>
        <rdfs:range rdf:resource="http://web-development-ontology.netlify.app/wdo#SoftwareCode"/>
        <dc:identifier>WDO_OP:0000024</dc:identifier>
        <rdfs:label xml:lang="en">embeds code</rdfs:label>
        <skos:definition xml:lang="en">A relation indicating that a template contains embedded software code that is processed at runtime.</skos:definition>
    </owl:ObjectProperty>
    


    <!-- http://web-development-ontology.netlify.app/wdo#extendsType -->


    <owl:ObjectProperty rdf:about="http://web-development-ontology.netlify.app/wdo#extendsType">
        <owl:inverseOf rdf:resource="http://web-development-ontology.netlify.app/wdo#isExtendedBy"/>
        <rdfs:domain rdf:resource="http://web-development-ontology.netlify.app/wdo#ComplexType"/>
        <rdfs:range rdf:resource="http://web-development-ontology.netlify.app/wdo#ComplexType"/>
        <dc:identifier>WDO_OP:0000010</dc:identifier>
        <rdfs:label xml:lang="en">extends type</rdfs:label>
        <skos:definition xml:lang="en">A relation indicating that a Complex Type inherits from or extends another Complex Type.</skos:definition>
    </owl:ObjectProperty>
    


    <!-- http://web-development-ontology.netlify.app/wdo#fixesIssue -->


    <owl:ObjectProperty rdf:about="http://web-development-ontology.netlify.app/wdo#fixesIssue">
        <rdfs:subPropertyOf rdf:resource="http://web-development-ontology.netlify.app/wdo#addressesIssue"/>
        <owl:inverseOf rdf:resource="http://web-development-ontology.netlify.app/wdo#isFixedBy"/>
        <rdfs:domain rdf:resource="http://web-development-ontology.netlify.app/wdo#Commit"/>
        <rdfs:range rdf:resource="http://web-development-ontology.netlify.app/wdo#Issue"/>
        <dc:identifier>WDO_OP:0000043</dc:identifier>
        <rdfs:label xml:lang="en">fixes issue</rdfs:label>
        <skos:definition xml:lang="en">A relation that is a sub-property of &apos;addressesIssue&apos;, specifically indicating that a commit resolves or closes an issue.</skos:definition>
    </owl:ObjectProperty>
    


    <!-- http://web-development-ontology.netlify.app/wdo#hasArgument -->


    <owl:ObjectProperty rdf:about="http://web-development-ontology.netlify.app/wdo#hasArgument">
        <owl:inverseOf rdf:resource="http://web-development-ontology.netlify.app/wdo#isArgumentIn"/>
        <rdfs:domain rdf:resource="http://web-development-ontology.netlify.app/wdo#FunctionCallSite"/>
        <rdfs:range rdf:resource="http://web-development-ontology.netlify.app/wdo#CodeConstruct"/>
        <dc:identifier>WDO_OP:0000034</dc:identifier>
        <rdfs:label xml:lang="en">has argument</rdfs:label>
        <skos:definition xml:lang="en">A relation between a FunctionCallSite and a CodeConstruct (such as a VariableDeclaration or a literal value) passed as an argument.</skos:definition>
    </owl:ObjectProperty>
    


    <!-- http://web-development-ontology.netlify.app/wdo#hasCodeDocumentation -->


    <owl:ObjectProperty rdf:about="http://web-development-ontology.netlify.app/wdo#hasCodeDocumentation">
        <rdfs:subPropertyOf rdf:resource="http://web-development-ontology.netlify.app/wdo#isDocumentedBy"/>
        <owl:inverseOf rdf:resource="http://web-development-ontology.netlify.app/wdo#isAboutCode"/>
        <rdfs:domain rdf:resource="http://web-development-ontology.netlify.app/wdo#SoftwareCode"/>
        <rdfs:range rdf:resource="http://web-development-ontology.netlify.app/wdo#Documentation"/>
        <dc:identifier>WDO_OP:0000076</dc:identifier>
        <rdfs:label xml:lang="en">has code documentation</rdfs:label>
        <skos:definition xml:lang="en">A specific relation from a code entity to the documentation that is about it.</skos:definition>
    </owl:ObjectProperty>
    


    <!-- http://web-development-ontology.netlify.app/wdo#hasCodePart -->


    <owl:ObjectProperty rdf:about="http://web-development-ontology.netlify.app/wdo#hasCodePart">
        <owl:inverseOf rdf:resource="http://web-development-ontology.netlify.app/wdo#isCodePartOf"/>
        <rdfs:domain rdf:resource="http://web-development-ontology.netlify.app/wdo#SoftwareCode"/>
        <rdfs:range rdf:resource="http://web-development-ontology.netlify.app/wdo#CodeConstruct"/>
        <dc:identifier>WDO_OP:0000130</dc:identifier>
        <rdfs:label xml:lang="en">has code part</rdfs:label>
        <skos:definition xml:lang="en">A relation indicating that a software code content entity contains a code construct as one of its parts.</skos:definition>
    </owl:ObjectProperty>
    


    <!-- http://web-development-ontology.netlify.app/wdo#hasCommit -->


    <owl:ObjectProperty rdf:about="http://web-development-ontology.netlify.app/wdo#hasCommit">
        <owl:inverseOf rdf:resource="http://web-development-ontology.netlify.app/wdo#isCommitIn"/>
        <rdfs:domain rdf:resource="http://web-development-ontology.netlify.app/wdo#Repository"/>
        <rdfs:range rdf:resource="http://web-development-ontology.netlify.app/wdo#Commit"/>
        <dc:identifier>WDO_OP:0000039</dc:identifier>
        <rdfs:label xml:lang="en">has commit</rdfs:label>
        <skos:definition xml:lang="en">A relation linking a repository to the commits in its history.</skos:definition>
    </owl:ObjectProperty>
    


    <!-- http://web-development-ontology.netlify.app/wdo#hasCommitMessage -->


    <owl:ObjectProperty rdf:about="http://web-development-ontology.netlify.app/wdo#hasCommitMessage">
        <owl:inverseOf rdf:resource="http://web-development-ontology.netlify.app/wdo#isMessageOfCommit"/>
        <rdfs:domain rdf:resource="http://web-development-ontology.netlify.app/wdo#Commit"/>
        <rdfs:range rdf:resource="http://web-development-ontology.netlify.app/wdo#CommitMessage"/>
        <dc:identifier>WDO_OP:0000041</dc:identifier>
        <rdfs:label xml:lang="en">has commit message</rdfs:label>
        <skos:definition xml:lang="en">A relation linking a Commit process to its descriptive CommitMessage entity.</skos:definition>
    </owl:ObjectProperty>
    


    <!-- http://web-development-ontology.netlify.app/wdo#hasContributor -->


    <owl:ObjectProperty rdf:about="http://web-development-ontology.netlify.app/wdo#hasContributor">
        <rdfs:domain rdf:resource="http://web-development-ontology.netlify.app/wdo#Repository"/>
        <rdfs:range rdf:resource="http://xmlns.com/foaf/0.1/Person"/>
        <dc:identifier>WDO_OP:0000125</dc:identifier>
        <rdfs:label xml:lang="en">has contributor</rdfs:label>
        <skos:definition xml:lang="en">A relation linking a repository or project to a person who has contributed to it in any capacity.</skos:definition>
    </owl:ObjectProperty>
    


    <!-- http://web-development-ontology.netlify.app/wdo#hasDocumentComponent -->


    <owl:ObjectProperty rdf:about="http://web-development-ontology.netlify.app/wdo#hasDocumentComponent">
        <rdfs:subPropertyOf rdf:resource="http://purl.obolibrary.org/obo/BFO_0000178"/>
        <owl:inverseOf rdf:resource="http://web-development-ontology.netlify.app/wdo#isDocumentComponentOf"/>
        <rdf:type rdf:resource="http://www.w3.org/2002/07/owl#TransitiveProperty"/>
        <rdfs:domain rdf:resource="http://web-development-ontology.netlify.app/wdo#InformationContentEntity"/>
        <rdfs:range rdf:resource="http://web-development-ontology.netlify.app/wdo#InformationContentEntity"/>
        <dc:identifier>WDO_OP:0000015</dc:identifier>
        <rdfs:label xml:lang="en">has document component</rdfs:label>
        <skos:definition xml:lang="en">A transitive part-whole relation between an InformationContentEntity (like a document) and a smaller InformationContentEntity that is one of its components (like a section or paragraph).</skos:definition>
    </owl:ObjectProperty>
    


    <!-- http://web-development-ontology.netlify.app/wdo#hasField -->


    <owl:ObjectProperty rdf:about="http://web-development-ontology.netlify.app/wdo#hasField">
        <rdfs:subPropertyOf rdf:resource="http://web-development-ontology.netlify.app/wdo#declares"/>
        <owl:inverseOf rdf:resource="http://web-development-ontology.netlify.app/wdo#isFieldOf"/>
        <rdfs:domain rdf:resource="http://web-development-ontology.netlify.app/wdo#ComplexType"/>
        <rdfs:range rdf:resource="http://web-development-ontology.netlify.app/wdo#AttributeDeclaration"/>
        <dc:identifier>WDO_OP:0000009</dc:identifier>
        <rdfs:label xml:lang="en">has field</rdfs:label>
        <skos:definition xml:lang="en">A relation between a Complex Type and an AttributeDeclaration that it declares as a field.</skos:definition>
    </owl:ObjectProperty>
    


    <!-- http://web-development-ontology.netlify.app/wdo#hasFile -->


    <owl:ObjectProperty rdf:about="http://web-development-ontology.netlify.app/wdo#hasFile">
        <owl:inverseOf rdf:resource="http://web-development-ontology.netlify.app/wdo#isFileOf"/>
        <rdfs:domain rdf:resource="http://web-development-ontology.netlify.app/wdo#Repository"/>
        <rdfs:range rdf:resource="http://web-development-ontology.netlify.app/wdo#DigitalInformationCarrier"/>
        <dc:identifier>WDO_OP:0000038</dc:identifier>
        <rdfs:label xml:lang="en">has file</rdfs:label>
        <skos:definition xml:lang="en">A relation linking a repository to the digital information carriers (files) it contains.</skos:definition>
    </owl:ObjectProperty>
    


    <!-- http://web-development-ontology.netlify.app/wdo#hasMethod -->


    <owl:ObjectProperty rdf:about="http://web-development-ontology.netlify.app/wdo#hasMethod">
        <rdfs:subPropertyOf rdf:resource="http://web-development-ontology.netlify.app/wdo#declares"/>
        <owl:inverseOf rdf:resource="http://web-development-ontology.netlify.app/wdo#isMethodOf"/>
        <rdfs:domain rdf:resource="http://web-development-ontology.netlify.app/wdo#ComplexType"/>
        <rdfs:range rdf:resource="http://web-development-ontology.netlify.app/wdo#FunctionDefinition"/>
        <dc:identifier>WDO_OP:0000008</dc:identifier>
        <rdfs:label xml:lang="en">has method</rdfs:label>
        <skos:definition xml:lang="en">A relation between a Complex Type (Class, Interface, Trait) and a FunctionDefinition that it declares as a method.</skos:definition>
    </owl:ObjectProperty>
    


    <!-- http://web-development-ontology.netlify.app/wdo#hasParameter -->


    <owl:ObjectProperty rdf:about="http://web-development-ontology.netlify.app/wdo#hasParameter">
        <rdfs:subPropertyOf rdf:resource="http://web-development-ontology.netlify.app/wdo#declares"/>
        <owl:inverseOf rdf:resource="http://web-development-ontology.netlify.app/wdo#isParameterOf"/>
        <rdfs:domain rdf:resource="http://web-development-ontology.netlify.app/wdo#FunctionDefinition"/>
        <rdfs:range rdf:resource="http://web-development-ontology.netlify.app/wdo#Parameter"/>
        <dc:identifier>WDO_OP:0000012</dc:identifier>
        <rdfs:label xml:lang="en">has parameter</rdfs:label>
        <skos:definition xml:lang="en">A relation between a FunctionDefinition and a Parameter that it declares.</skos:definition>
    </owl:ObjectProperty>
    


    <!-- http://web-development-ontology.netlify.app/wdo#hasProjectOutput -->


    <owl:ObjectProperty rdf:about="http://web-development-ontology.netlify.app/wdo#hasProjectOutput">
        <rdfs:subPropertyOf rdf:resource="http://purl.obolibrary.org/obo/BFO_0000057"/>
        <owl:inverseOf rdf:resource="http://web-development-ontology.netlify.app/wdo#isOutputOfProject"/>
        <rdfs:domain rdf:resource="http://web-development-ontology.netlify.app/wdo#WebDevelopmentProject"/>
        <rdfs:range rdf:resource="http://web-development-ontology.netlify.app/wdo#InformationContentEntity"/>
        <dc:identifier>WDO_OP:0000005</dc:identifier>
        <rdfs:label xml:lang="en">has project output</rdfs:label>
        <skos:definition xml:lang="en">A relation between a WebDevelopmentProject (a process) and an InformationContentEntity that is its output or deliverable.</skos:definition>
    </owl:ObjectProperty>
    


    <!-- http://web-development-ontology.netlify.app/wdo#hasRepository -->


    <owl:ObjectProperty rdf:about="http://web-development-ontology.netlify.app/wdo#hasRepository">
        <owl:inverseOf rdf:resource="http://web-development-ontology.netlify.app/wdo#isRepositoryOf"/>
        <rdfs:domain>
            <owl:Class>
                <owl:unionOf rdf:parseType="Collection">
                    <rdf:Description rdf:about="http://web-development-ontology.netlify.app/wdo#Organization"/>
                    <rdf:Description rdf:about="http://web-development-ontology.netlify.app/wdo#WebDevelopmentProject"/>
                </owl:unionOf>
            </owl:Class>
        </rdfs:domain>
        <rdfs:range rdf:resource="http://web-development-ontology.netlify.app/wdo#Repository"/>
        <dc:identifier>WDO_OP:0000037</dc:identifier>
        <rdfs:label xml:lang="en">has repository</rdfs:label>
        <skos:definition xml:lang="en">A relation that links a project or organization to its source code repository.</skos:definition>
    </owl:ObjectProperty>
    


    <!-- http://web-development-ontology.netlify.app/wdo#hasReturnType -->


    <owl:ObjectProperty rdf:about="http://web-development-ontology.netlify.app/wdo#hasReturnType">
        <owl:inverseOf rdf:resource="http://web-development-ontology.netlify.app/wdo#isReturnTypeOf"/>
        <rdfs:domain rdf:resource="http://web-development-ontology.netlify.app/wdo#FunctionDefinition"/>
        <rdfs:range rdf:resource="http://web-development-ontology.netlify.app/wdo#TypeDeclaration"/>
        <dc:identifier>WDO_OP:0000013</dc:identifier>
        <rdfs:label xml:lang="en">has return type</rdfs:label>
        <skos:definition xml:lang="en">A relation specifying the Type that a FunctionDefinition returns.</skos:definition>
    </owl:ObjectProperty>
    


    <!-- http://web-development-ontology.netlify.app/wdo#hasType -->


    <owl:ObjectProperty rdf:about="http://web-development-ontology.netlify.app/wdo#hasType">
        <owl:inverseOf rdf:resource="http://web-development-ontology.netlify.app/wdo#isTypeOf"/>
        <rdfs:domain rdf:resource="http://web-development-ontology.netlify.app/wdo#CodeConstruct"/>
        <rdfs:range rdf:resource="http://web-development-ontology.netlify.app/wdo#TypeDeclaration"/>
        <dc:identifier>WDO_OP:0000014</dc:identifier>
        <rdfs:label xml:lang="en">has type</rdfs:label>
        <skos:definition xml:lang="en">A relation specifying the Type of a typed code construct (e.g., an attribute, a parameter, a variable).</skos:definition>
    </owl:ObjectProperty>
    


    <!-- http://web-development-ontology.netlify.app/wdo#implementsInterface -->


    <owl:ObjectProperty rdf:about="http://web-development-ontology.netlify.app/wdo#implementsInterface">
        <owl:inverseOf rdf:resource="http://web-development-ontology.netlify.app/wdo#isImplementedBy"/>
        <rdfs:domain rdf:resource="http://web-development-ontology.netlify.app/wdo#ClassDefinition"/>
        <rdfs:range rdf:resource="http://web-development-ontology.netlify.app/wdo#InterfaceDefinition"/>
        <dc:identifier>WDO_OP:0000011</dc:identifier>
        <rdfs:label xml:lang="en">implements interface</rdfs:label>
        <skos:definition xml:lang="en">A relation indicating that a ClassDefinition implements an InterfaceDefinition.</skos:definition>
    </owl:ObjectProperty>
    


    <!-- http://web-development-ontology.netlify.app/wdo#imports -->


    <owl:ObjectProperty rdf:about="http://web-development-ontology.netlify.app/wdo#imports">
        <owl:inverseOf rdf:resource="http://web-development-ontology.netlify.app/wdo#isImportedBy"/>
        <rdfs:domain rdf:resource="http://web-development-ontology.netlify.app/wdo#Module"/>
        <rdfs:range rdf:resource="http://web-development-ontology.netlify.app/wdo#Module"/>
        <dc:identifier>WDO_OP:0000028</dc:identifier>
        <rdfs:label xml:lang="en">imports</rdfs:label>
        <skos:definition xml:lang="en">A relation indicating that a module uses or includes another module to access its functionality.</skos:definition>
    </owl:ObjectProperty>
    


    <!-- http://web-development-ontology.netlify.app/wdo#informationBorneBy -->


    <owl:ObjectProperty rdf:about="http://web-development-ontology.netlify.app/wdo#informationBorneBy">
        <rdfs:domain rdf:resource="http://web-development-ontology.netlify.app/wdo#InformationContentEntity"/>
        <rdfs:range rdf:resource="http://web-development-ontology.netlify.app/wdo#DigitalInformationCarrier"/>
        <dc:identifier>WDO_OP:0000002</dc:identifier>
        <rdfs:label xml:lang="en">information borne by</rdfs:label>
        <skos:definition xml:lang="en">A relation that is the inverse of &apos;bearerOfInformation&apos;, linking an information entity to the digital carrier that encodes it.</skos:definition>
    </owl:ObjectProperty>
    


    <!-- http://web-development-ontology.netlify.app/wdo#invokes -->


    <owl:ObjectProperty rdf:about="http://web-development-ontology.netlify.app/wdo#invokes">
        <owl:inverseOf rdf:resource="http://web-development-ontology.netlify.app/wdo#isInvokedBy"/>
        <rdfs:domain rdf:resource="http://web-development-ontology.netlify.app/wdo#FunctionDefinition"/>
        <rdfs:range rdf:resource="http://web-development-ontology.netlify.app/wdo#FunctionDefinition"/>
        <dc:identifier>WDO_OP:0000020</dc:identifier>
        <rdfs:label xml:lang="en">invokes</rdfs:label>
        <skos:definition xml:lang="en">An abstract relation indicating that one function&apos;s logic calls another function. This can be inferred from &apos;callsFunction&apos;.</skos:definition>
    </owl:ObjectProperty>
    


    <!-- http://web-development-ontology.netlify.app/wdo#isAboutCode -->


    <owl:ObjectProperty rdf:about="http://web-development-ontology.netlify.app/wdo#isAboutCode">
        <rdfs:subPropertyOf rdf:resource="http://web-development-ontology.netlify.app/wdo#documentsEntity"/>
        <rdfs:domain rdf:resource="http://web-development-ontology.netlify.app/wdo#Documentation"/>
        <rdfs:range rdf:resource="http://web-development-ontology.netlify.app/wdo#SoftwareCode"/>
        <dc:identifier>WDO_OP:0000100</dc:identifier>
        <rdfs:label xml:lang="en">is about code</rdfs:label>
        <skos:definition xml:lang="en">A specific relation indicating that a documentation element, such as a code comment, is about a code entity.</skos:definition>
    </owl:ObjectProperty>
    


    <!-- http://web-development-ontology.netlify.app/wdo#isAccessedBy -->


    <owl:ObjectProperty rdf:about="http://web-development-ontology.netlify.app/wdo#isAccessedBy">
        <rdfs:domain>
            <owl:Class>
                <owl:unionOf rdf:parseType="Collection">
                    <rdf:Description rdf:about="http://web-development-ontology.netlify.app/wdo#AttributeDeclaration"/>
                    <rdf:Description rdf:about="http://web-development-ontology.netlify.app/wdo#VariableDeclaration"/>
                </owl:unionOf>
            </owl:Class>
        </rdfs:domain>
        <rdfs:range rdf:resource="http://web-development-ontology.netlify.app/wdo#FunctionDefinition"/>
        <dc:identifier>WDO_OP:0000068</dc:identifier>
        <rdfs:label xml:lang="en">is accessed by</rdfs:label>
        <skos:definition xml:lang="en">A relation from an attribute or variable to the function that accesses it.</skos:definition>
    </owl:ObjectProperty>
    


    <!-- http://web-development-ontology.netlify.app/wdo#isAddressedBy -->


    <owl:ObjectProperty rdf:about="http://web-development-ontology.netlify.app/wdo#isAddressedBy">
        <rdfs:domain rdf:resource="http://web-development-ontology.netlify.app/wdo#Issue"/>
        <rdfs:range rdf:resource="http://web-development-ontology.netlify.app/wdo#Commit"/>
        <dc:identifier>WDO_OP:0000055</dc:identifier>
        <rdfs:label xml:lang="en">is addressed by</rdfs:label>
        <skos:definition xml:lang="en">A relation from an issue to a commit that makes progress on it.</skos:definition>
    </owl:ObjectProperty>
    


    <!-- http://web-development-ontology.netlify.app/wdo#isArgumentIn -->


    <owl:ObjectProperty rdf:about="http://web-development-ontology.netlify.app/wdo#isArgumentIn">
        <rdfs:domain rdf:resource="http://web-development-ontology.netlify.app/wdo#CodeConstruct"/>
        <rdfs:range rdf:resource="http://web-development-ontology.netlify.app/wdo#FunctionCallSite"/>
        <dc:identifier>WDO_OP:0000067</dc:identifier>
        <rdfs:label xml:lang="en">is argument in</rdfs:label>
        <skos:definition xml:lang="en">A relation from a code construct to the function call site where it is used as an argument.</skos:definition>
    </owl:ObjectProperty>
    


    <!-- http://web-development-ontology.netlify.app/wdo#isArtifactOfBuild -->


    <owl:ObjectProperty rdf:about="http://web-development-ontology.netlify.app/wdo#isArtifactOfBuild">
        <owl:inverseOf rdf:resource="http://web-development-ontology.netlify.app/wdo#packagesInto"/>
        <rdfs:domain rdf:resource="http://web-development-ontology.netlify.app/wdo#ArchiveFile"/>
        <rdfs:range rdf:resource="http://web-development-ontology.netlify.app/wdo#BuildScript"/>
        <dc:identifier>WDO_OP:0000073</dc:identifier>
        <rdfs:label xml:lang="en">is artifact of build</rdfs:label>
        <skos:definition xml:lang="en">A relation from a distributable archive file to the build script that created it.</skos:definition>
    </owl:ObjectProperty>
    


    <!-- http://web-development-ontology.netlify.app/wdo#isBaseFor -->


    <owl:ObjectProperty rdf:about="http://web-development-ontology.netlify.app/wdo#isBaseFor">
        <owl:inverseOf rdf:resource="http://web-development-ontology.netlify.app/wdo#isBasedOn"/>
        <rdfs:domain rdf:resource="http://web-development-ontology.netlify.app/wdo#ContainerImage"/>
        <rdfs:range rdf:resource="http://web-development-ontology.netlify.app/wdo#DockerfileSpecification"/>
        <dc:identifier>WDO_OP:0000074</dc:identifier>
        <rdfs:label xml:lang="en">is base for</rdfs:label>
        <skos:definition xml:lang="en">A relation from a container image to the Dockerfile specification that is based on it.</skos:definition>
    </owl:ObjectProperty>
    


    <!-- http://web-development-ontology.netlify.app/wdo#isBasedOn -->


    <owl:ObjectProperty rdf:about="http://web-development-ontology.netlify.app/wdo#isBasedOn">
        <rdfs:domain rdf:resource="http://web-development-ontology.netlify.app/wdo#DockerfileSpecification"/>
        <rdfs:range rdf:resource="http://web-development-ontology.netlify.app/wdo#ContainerImage"/>
        <dc:identifier>WDO_OP:0000047</dc:identifier>
        <rdfs:label xml:lang="en">is based on</rdfs:label>
        <skos:definition xml:lang="en">A relation from a Dockerfile specification to the base container image it extends.</skos:definition>
    </owl:ObjectProperty>
    


    <!-- http://web-development-ontology.netlify.app/wdo#isCalledByFunctionAt -->


    <owl:ObjectProperty rdf:about="http://web-development-ontology.netlify.app/wdo#isCalledByFunctionAt">
        <rdfs:subPropertyOf rdf:resource="http://web-development-ontology.netlify.app/wdo#isInvokedBy"/>
        <rdfs:domain rdf:resource="http://web-development-ontology.netlify.app/wdo#FunctionDefinition"/>
        <rdfs:range rdf:resource="http://web-development-ontology.netlify.app/wdo#FunctionCallSite"/>
        <dc:identifier>WDO_OP:0000066</dc:identifier>
        <rdfs:label xml:lang="en">is called by function at</rdfs:label>
        <skos:definition xml:lang="en">A specific relation from a function to the call site that invokes it.</skos:definition>
    </owl:ObjectProperty>
    


    <!-- http://web-development-ontology.netlify.app/wdo#isCodePartOf -->


    <owl:ObjectProperty rdf:about="http://web-development-ontology.netlify.app/wdo#isCodePartOf">
        <rdfs:domain rdf:resource="http://web-development-ontology.netlify.app/wdo#CodeConstruct"/>
        <rdfs:range rdf:resource="http://web-development-ontology.netlify.app/wdo#SoftwareCode"/>
        <dc:identifier>WDO_OP:0000131</dc:identifier>
        <rdfs:label xml:lang="en">is code part of</rdfs:label>
        <skos:definition xml:lang="en">A relation indicating that a code construct is part of a software code content entity.</skos:definition>
    </owl:ObjectProperty>
    


    <!-- http://web-development-ontology.netlify.app/wdo#isCommitIn -->


    <owl:ObjectProperty rdf:about="http://web-development-ontology.netlify.app/wdo#isCommitIn">
        <rdfs:domain rdf:resource="http://web-development-ontology.netlify.app/wdo#Commit"/>
        <rdfs:range rdf:resource="http://web-development-ontology.netlify.app/wdo#Repository"/>
        <dc:identifier>WDO_OP:0000052</dc:identifier>
        <rdfs:label xml:lang="en">is commit in</rdfs:label>
        <skos:definition xml:lang="en">A relation linking a commit to the repository it belongs to.</skos:definition>
    </owl:ObjectProperty>
    


    <!-- http://web-development-ontology.netlify.app/wdo#isCompiledBy -->


    <owl:ObjectProperty rdf:about="http://web-development-ontology.netlify.app/wdo#isCompiledBy">
        <rdfs:domain rdf:resource="http://web-development-ontology.netlify.app/wdo#SourceCodeFile"/>
        <rdfs:range rdf:resource="http://web-development-ontology.netlify.app/wdo#BuildScript"/>
        <dc:identifier>WDO_OP:0000072</dc:identifier>
        <rdfs:label xml:lang="en">is compiled by</rdfs:label>
        <skos:definition xml:lang="en">A relation from a source code file to the build script that compiles it.</skos:definition>
    </owl:ObjectProperty>
    


    <!-- http://web-development-ontology.netlify.app/wdo#isDeclarationUsedBy -->


    <owl:ObjectProperty rdf:about="http://web-development-ontology.netlify.app/wdo#isDeclarationUsedBy">
        <owl:inverseOf rdf:resource="http://web-development-ontology.netlify.app/wdo#usesDeclaration"/>
        <rdfs:domain rdf:resource="http://web-development-ontology.netlify.app/wdo#CodeConstruct"/>
        <rdfs:range rdf:resource="http://web-development-ontology.netlify.app/wdo#CodeConstruct"/>
        <dc:identifier>WDO_OP:0000069</dc:identifier>
        <rdfs:label xml:lang="en">is declaration used by</rdfs:label>
        <skos:definition xml:lang="en">A relation from a declaration to a code construct where that declaration is used.</skos:definition>
    </owl:ObjectProperty>
    


    <!-- http://web-development-ontology.netlify.app/wdo#isDeclaredBy -->


    <owl:ObjectProperty rdf:about="http://web-development-ontology.netlify.app/wdo#isDeclaredBy">
        <rdfs:domain rdf:resource="http://web-development-ontology.netlify.app/wdo#CodeConstruct"/>
        <rdfs:range rdf:resource="http://web-development-ontology.netlify.app/wdo#SoftwareCode"/>
        <dc:identifier>WDO_OP:0000057</dc:identifier>
        <rdfs:label xml:lang="en">is declared by</rdfs:label>
        <skos:definition xml:lang="en">A relation from a code construct to the larger code entity that declares it.</skos:definition>
    </owl:ObjectProperty>
    


    <!-- http://web-development-ontology.netlify.app/wdo#isDependencyOf -->


    <owl:ObjectProperty rdf:about="http://web-development-ontology.netlify.app/wdo#isDependencyOf">
        <owl:inverseOf rdf:resource="http://web-development-ontology.netlify.app/wdo#specifiesDependency"/>
        <rdfs:domain rdf:resource="http://web-development-ontology.netlify.app/wdo#SoftwarePackage"/>
        <rdfs:range>
            <owl:Class>
                <owl:unionOf rdf:parseType="Collection">
                    <rdf:Description rdf:about="http://web-development-ontology.netlify.app/wdo#BuildScript"/>
                    <rdf:Description rdf:about="http://web-development-ontology.netlify.app/wdo#SoftwarePackage"/>
                </owl:unionOf>
            </owl:Class>
        </rdfs:range>
        <dc:identifier>WDO_OP:0000070</dc:identifier>
        <rdfs:label xml:lang="en">is dependency of</rdfs:label>
        <skos:definition xml:lang="en">A relation from a package to the build script or other package that depends on it.</skos:definition>
    </owl:ObjectProperty>
    


    <!-- http://web-development-ontology.netlify.app/wdo#isDocumentComponentOf -->


    <owl:ObjectProperty rdf:about="http://web-development-ontology.netlify.app/wdo#isDocumentComponentOf">
        <rdfs:domain rdf:resource="http://web-development-ontology.netlify.app/wdo#InformationContentEntity"/>
        <rdfs:range rdf:resource="http://web-development-ontology.netlify.app/wdo#InformationContentEntity"/>
        <dc:identifier>WDO_OP:0000077</dc:identifier>
        <rdfs:label xml:lang="en">is document component of</rdfs:label>
        <skos:definition xml:lang="en">A relation from a smaller document part to the larger document that contains it.</skos:definition>
    </owl:ObjectProperty>
    


    <!-- http://web-development-ontology.netlify.app/wdo#isDocumentedBy -->


    <owl:ObjectProperty rdf:about="http://web-development-ontology.netlify.app/wdo#isDocumentedBy">
        <rdfs:domain rdf:resource="http://purl.obolibrary.org/obo/BFO_0000001"/>
        <rdfs:range rdf:resource="http://web-development-ontology.netlify.app/wdo#Documentation"/>
        <dc:identifier>WDO_OP:0000075</dc:identifier>
        <rdfs:label xml:lang="en">is documented by</rdfs:label>
        <skos:definition xml:lang="en">A relation from an entity to the documentation that describes it.</skos:definition>
    </owl:ObjectProperty>
    


    <!-- http://web-development-ontology.netlify.app/wdo#isEmbeddedIn -->


    <owl:ObjectProperty rdf:about="http://web-development-ontology.netlify.app/wdo#isEmbeddedIn">
        <rdfs:domain rdf:resource="http://web-development-ontology.netlify.app/wdo#SoftwareCode"/>
        <rdfs:range rdf:resource="http://web-development-ontology.netlify.app/wdo#Template"/>
        <dc:identifier>WDO_OP:0000082</dc:identifier>
        <rdfs:label xml:lang="en">is embedded in</rdfs:label>
        <skos:definition xml:lang="en">A relation from a piece of software code to the template it is embedded in.</skos:definition>
    </owl:ObjectProperty>
    


    <!-- http://web-development-ontology.netlify.app/wdo#isExtendedBy -->


    <owl:ObjectProperty rdf:about="http://web-development-ontology.netlify.app/wdo#isExtendedBy">
        <rdfs:domain rdf:resource="http://web-development-ontology.netlify.app/wdo#ComplexType"/>
        <rdfs:range rdf:resource="http://web-development-ontology.netlify.app/wdo#ComplexType"/>
        <dc:identifier>WDO_OP:0000063</dc:identifier>
        <rdfs:label xml:lang="en">is extended by</rdfs:label>
        <skos:definition xml:lang="en">A relation indicating that a Complex Type is a superclass or supertype for another Complex Type.</skos:definition>
    </owl:ObjectProperty>
    


    <!-- http://web-development-ontology.netlify.app/wdo#isFieldOf -->


    <owl:ObjectProperty rdf:about="http://web-development-ontology.netlify.app/wdo#isFieldOf">
        <rdfs:subPropertyOf rdf:resource="http://web-development-ontology.netlify.app/wdo#isDeclaredBy"/>
        <rdfs:domain rdf:resource="http://web-development-ontology.netlify.app/wdo#AttributeDeclaration"/>
        <rdfs:range rdf:resource="http://web-development-ontology.netlify.app/wdo#ComplexType"/>
        <dc:identifier>WDO_OP:0000059</dc:identifier>
        <rdfs:label xml:lang="en">is field of</rdfs:label>
        <skos:definition xml:lang="en">A relation from an attribute declaration to the complex type that declares it as a field.</skos:definition>
    </owl:ObjectProperty>
    


    <!-- http://web-development-ontology.netlify.app/wdo#isFileOf -->


    <owl:ObjectProperty rdf:about="http://web-development-ontology.netlify.app/wdo#isFileOf">
        <rdfs:domain rdf:resource="http://web-development-ontology.netlify.app/wdo#DigitalInformationCarrier"/>
        <rdfs:range rdf:resource="http://web-development-ontology.netlify.app/wdo#Repository"/>
        <dc:identifier>WDO_OP:0000051</dc:identifier>
        <rdfs:label xml:lang="en">is file of</rdfs:label>
        <skos:definition xml:lang="en">A relation linking a file to the repository that contains it.</skos:definition>
    </owl:ObjectProperty>
    


    <!-- http://web-development-ontology.netlify.app/wdo#isFixedBy -->


    <owl:ObjectProperty rdf:about="http://web-development-ontology.netlify.app/wdo#isFixedBy">
        <rdfs:subPropertyOf rdf:resource="http://web-development-ontology.netlify.app/wdo#isAddressedBy"/>
        <rdfs:domain rdf:resource="http://web-development-ontology.netlify.app/wdo#Issue"/>
        <rdfs:range rdf:resource="http://web-development-ontology.netlify.app/wdo#Commit"/>
        <dc:identifier>WDO_OP:0000056</dc:identifier>
        <rdfs:label xml:lang="en">is fixed by</rdfs:label>
        <skos:definition xml:lang="en">A relation from an issue to the commit that resolves it.</skos:definition>
    </owl:ObjectProperty>
    


    <!-- http://web-development-ontology.netlify.app/wdo#isFrameworkFor -->


    <owl:ObjectProperty rdf:about="http://web-development-ontology.netlify.app/wdo#isFrameworkFor">
        <owl:inverseOf rdf:resource="http://web-development-ontology.netlify.app/wdo#usesFramework"/>
        <rdfs:domain rdf:resource="http://web-development-ontology.netlify.app/wdo#SoftwareFramework"/>
        <rdfs:range rdf:resource="http://web-development-ontology.netlify.app/wdo#SoftwareCode"/>
        <dc:identifier>WDO_OP:0000071</dc:identifier>
        <rdfs:label xml:lang="en">is framework for</rdfs:label>
        <skos:definition xml:lang="en">A relation from a framework to the software code that is built upon it.</skos:definition>
    </owl:ObjectProperty>
    


    <!-- http://web-development-ontology.netlify.app/wdo#isGuidelineFor -->


    <owl:ObjectProperty rdf:about="http://web-development-ontology.netlify.app/wdo#isGuidelineFor">
        <rdfs:domain rdf:resource="http://web-development-ontology.netlify.app/wdo#BestPracticeGuideline"/>
        <rdfs:range rdf:resource="http://purl.obolibrary.org/obo/BFO_0000001"/>
        <dc:identifier>WDO_OP:0000079</dc:identifier>
        <rdfs:label xml:lang="en">is guideline for</rdfs:label>
        <skos:definition xml:lang="en">A relation from a guideline to an entity that conforms to it.</skos:definition>
    </owl:ObjectProperty>
    


    <!-- http://web-development-ontology.netlify.app/wdo#isImplementedBy -->


    <owl:ObjectProperty rdf:about="http://web-development-ontology.netlify.app/wdo#isImplementedBy">
        <rdfs:domain rdf:resource="http://web-development-ontology.netlify.app/wdo#InterfaceDefinition"/>
        <rdfs:range rdf:resource="http://web-development-ontology.netlify.app/wdo#ClassDefinition"/>
        <dc:identifier>WDO_OP:0000064</dc:identifier>
        <rdfs:label xml:lang="en">is implemented by</rdfs:label>
        <skos:definition xml:lang="en">A relation from an interface to a class that implements it.</skos:definition>
    </owl:ObjectProperty>
    


    <!-- http://web-development-ontology.netlify.app/wdo#isImportedBy -->


    <owl:ObjectProperty rdf:about="http://web-development-ontology.netlify.app/wdo#isImportedBy">
        <rdfs:domain rdf:resource="http://web-development-ontology.netlify.app/wdo#Module"/>
        <rdfs:range rdf:resource="http://web-development-ontology.netlify.app/wdo#Module"/>
        <dc:identifier>WDO_OP:0000029</dc:identifier>
        <rdfs:label xml:lang="en">is imported by</rdfs:label>
        <skos:definition xml:lang="en">A relation that is the inverse of &apos;imports&apos;, indicating that a module&apos;s functionality is used by another module.</skos:definition>
    </owl:ObjectProperty>
    


    <!-- http://web-development-ontology.netlify.app/wdo#isInvokedBy -->


    <owl:ObjectProperty rdf:about="http://web-development-ontology.netlify.app/wdo#isInvokedBy">
        <rdfs:domain rdf:resource="http://web-development-ontology.netlify.app/wdo#FunctionDefinition"/>
        <rdfs:range rdf:resource="http://web-development-ontology.netlify.app/wdo#FunctionDefinition"/>
        <dc:identifier>WDO_OP:0000065</dc:identifier>
        <rdfs:label xml:lang="en">is invoked by</rdfs:label>
        <skos:definition xml:lang="en">An abstract relation indicating that one function is called by another function&apos;s logic.</skos:definition>
    </owl:ObjectProperty>
    


    <!-- http://web-development-ontology.netlify.app/wdo#isJustifiedBy -->


    <owl:ObjectProperty rdf:about="http://web-development-ontology.netlify.app/wdo#isJustifiedBy">
        <owl:inverseOf rdf:resource="http://web-development-ontology.netlify.app/wdo#justifies"/>
        <rdfs:domain rdf:resource="http://purl.obolibrary.org/obo/BFO_0000001"/>
        <rdfs:range rdf:resource="http://web-development-ontology.netlify.app/wdo#ArchitecturalDecisionRecord"/>
        <dc:identifier>WDO_OP:0000078</dc:identifier>
        <rdfs:label xml:lang="en">is justified by</rdfs:label>
        <skos:definition xml:lang="en">A relation from an architectural choice to the decision record that justifies it.</skos:definition>
    </owl:ObjectProperty>
    


    <!-- http://web-development-ontology.netlify.app/wdo#isManipulatedBy -->


    <owl:ObjectProperty rdf:about="http://web-development-ontology.netlify.app/wdo#isManipulatedBy">
        <owl:inverseOf rdf:resource="http://web-development-ontology.netlify.app/wdo#manipulates"/>
        <rdfs:domain rdf:resource="http://web-development-ontology.netlify.app/wdo#HTMLCode"/>
        <rdfs:range rdf:resource="http://web-development-ontology.netlify.app/wdo#ProgrammingLanguageCode"/>
        <dc:identifier>WDO_OP:0000081</dc:identifier>
        <rdfs:label xml:lang="en">is manipulated by</rdfs:label>
        <skos:definition xml:lang="en">A relation from an HTML entity to the programming language code that manipulates it.</skos:definition>
    </owl:ObjectProperty>
    


    <!-- http://web-development-ontology.netlify.app/wdo#isMessageOfCommit -->


    <owl:ObjectProperty rdf:about="http://web-development-ontology.netlify.app/wdo#isMessageOfCommit">
        <rdfs:domain rdf:resource="http://web-development-ontology.netlify.app/wdo#CommitMessage"/>
        <rdfs:range rdf:resource="http://web-development-ontology.netlify.app/wdo#Commit"/>
        <dc:identifier>WDO_OP:0000054</dc:identifier>
        <rdfs:label xml:lang="en">is message of commit</rdfs:label>
        <skos:definition xml:lang="en">A relation linking a CommitMessage to the Commit process it describes.</skos:definition>
    </owl:ObjectProperty>
    


    <!-- http://web-development-ontology.netlify.app/wdo#isMethodOf -->


    <owl:ObjectProperty rdf:about="http://web-development-ontology.netlify.app/wdo#isMethodOf">
        <rdfs:subPropertyOf rdf:resource="http://web-development-ontology.netlify.app/wdo#isDeclaredBy"/>
        <rdfs:domain rdf:resource="http://web-development-ontology.netlify.app/wdo#FunctionDefinition"/>
        <rdfs:range rdf:resource="http://web-development-ontology.netlify.app/wdo#ComplexType"/>
        <dc:identifier>WDO_OP:0000058</dc:identifier>
        <rdfs:label xml:lang="en">is method of</rdfs:label>
        <skos:definition xml:lang="en">A relation from a function definition to the complex type that declares it as a method.</skos:definition>
    </owl:ObjectProperty>
    


    <!-- http://web-development-ontology.netlify.app/wdo#isModifiedBy -->


    <owl:ObjectProperty rdf:about="http://web-development-ontology.netlify.app/wdo#isModifiedBy">
        <owl:inverseOf rdf:resource="http://web-development-ontology.netlify.app/wdo#modifies"/>
        <rdfs:domain rdf:resource="http://web-development-ontology.netlify.app/wdo#DigitalInformationCarrier"/>
        <rdfs:range rdf:resource="http://web-development-ontology.netlify.app/wdo#Commit"/>
        <dc:identifier>WDO_OP:0000053</dc:identifier>
        <rdfs:label xml:lang="en">is modified by</rdfs:label>
        <skos:definition xml:lang="en">A relation between a file and the commit process that changed it.</skos:definition>
    </owl:ObjectProperty>
    


    <!-- http://web-development-ontology.netlify.app/wdo#isOutputOfProject -->


    <owl:ObjectProperty rdf:about="http://web-development-ontology.netlify.app/wdo#isOutputOfProject">
        <rdfs:domain rdf:resource="http://web-development-ontology.netlify.app/wdo#InformationContentEntity"/>
        <rdfs:range rdf:resource="http://web-development-ontology.netlify.app/wdo#WebDevelopmentProject"/>
        <dc:identifier>WDO_OP:0000049</dc:identifier>
        <rdfs:label xml:lang="en">is output of project</rdfs:label>
        <skos:definition xml:lang="en">A relation from an output or deliverable to the WebDevelopmentProject that produced it.</skos:definition>
    </owl:ObjectProperty>
    


    <!-- http://web-development-ontology.netlify.app/wdo#isParameterOf -->


    <owl:ObjectProperty rdf:about="http://web-development-ontology.netlify.app/wdo#isParameterOf">
        <rdfs:subPropertyOf rdf:resource="http://web-development-ontology.netlify.app/wdo#isDeclaredBy"/>
        <rdfs:domain rdf:resource="http://web-development-ontology.netlify.app/wdo#Parameter"/>
        <rdfs:range rdf:resource="http://web-development-ontology.netlify.app/wdo#FunctionDefinition"/>
        <dc:identifier>WDO_OP:0000060</dc:identifier>
        <rdfs:label xml:lang="en">is parameter of</rdfs:label>
        <skos:definition xml:lang="en">A relation from a parameter to the function definition that declares it.</skos:definition>
    </owl:ObjectProperty>
    


    <!-- http://web-development-ontology.netlify.app/wdo#isReferredToByArgument -->


    <owl:ObjectProperty rdf:about="http://web-development-ontology.netlify.app/wdo#isReferredToByArgument">
        <owl:inverseOf rdf:resource="http://web-development-ontology.netlify.app/wdo#refersToVariable"/>
        <rdfs:domain rdf:resource="http://web-development-ontology.netlify.app/wdo#VariableDeclaration"/>
        <rdfs:range rdf:resource="http://web-development-ontology.netlify.app/wdo#Argument"/>
        <dc:identifier>WDO_OP:0000102</dc:identifier>
        <rdfs:label xml:lang="en">is referred to by argument</rdfs:label>
        <skos:definition xml:lang="en">The inverse relation, linking a VariableDeclaration to Argument nodes that refer to it as an argument at a callsite.</skos:definition>
    </owl:ObjectProperty>
    


    <!-- http://web-development-ontology.netlify.app/wdo#isRepositoryOf -->


    <owl:ObjectProperty rdf:about="http://web-development-ontology.netlify.app/wdo#isRepositoryOf">
        <rdfs:domain rdf:resource="http://web-development-ontology.netlify.app/wdo#Repository"/>
        <rdfs:range>
            <owl:Class>
                <owl:unionOf rdf:parseType="Collection">
                    <rdf:Description rdf:about="http://web-development-ontology.netlify.app/wdo#Organization"/>
                    <rdf:Description rdf:about="http://web-development-ontology.netlify.app/wdo#WebDevelopmentProject"/>
                </owl:unionOf>
            </owl:Class>
        </rdfs:range>
        <dc:identifier>WDO_OP:0000050</dc:identifier>
        <rdfs:label xml:lang="en">is repository of</rdfs:label>
        <skos:definition xml:lang="en">A relation that links a repository to the project or organization it belongs to.</skos:definition>
    </owl:ObjectProperty>
    


    <!-- http://web-development-ontology.netlify.app/wdo#isReturnTypeOf -->


    <owl:ObjectProperty rdf:about="http://web-development-ontology.netlify.app/wdo#isReturnTypeOf">
        <rdfs:domain rdf:resource="http://web-development-ontology.netlify.app/wdo#TypeDeclaration"/>
        <rdfs:range rdf:resource="http://web-development-ontology.netlify.app/wdo#FunctionDefinition"/>
        <dc:identifier>WDO_OP:0000062</dc:identifier>
        <rdfs:label xml:lang="en">is return type of</rdfs:label>
        <skos:definition xml:lang="en">A relation from a type to the function definition that returns it.</skos:definition>
    </owl:ObjectProperty>
    


    <!-- http://web-development-ontology.netlify.app/wdo#isStyledBy -->


    <owl:ObjectProperty rdf:about="http://web-development-ontology.netlify.app/wdo#isStyledBy">
        <owl:inverseOf rdf:resource="http://web-development-ontology.netlify.app/wdo#styles"/>
        <rdfs:domain rdf:resource="http://web-development-ontology.netlify.app/wdo#HTMLCode"/>
        <rdfs:range rdf:resource="http://web-development-ontology.netlify.app/wdo#CSSCode"/>
        <dc:identifier>WDO_OP:0000080</dc:identifier>
        <rdfs:label xml:lang="en">is styled by</rdfs:label>
        <skos:definition xml:lang="en">A relation from an HTML entity to the CSS entity that styles it.</skos:definition>
    </owl:ObjectProperty>
    


    <!-- http://web-development-ontology.netlify.app/wdo#isTestedBy -->


    <owl:ObjectProperty rdf:about="http://web-development-ontology.netlify.app/wdo#isTestedBy">
        <owl:inverseOf rdf:resource="http://web-development-ontology.netlify.app/wdo#tests"/>
        <rdfs:domain rdf:resource="http://web-development-ontology.netlify.app/wdo#SoftwareCode"/>
        <rdfs:range rdf:resource="http://web-development-ontology.netlify.app/wdo#TestCode"/>
        <dc:identifier>WDO_OP:0000032</dc:identifier>
        <rdfs:label xml:lang="en">is tested by</rdfs:label>
        <skos:definition xml:lang="en">A relation that is the inverse of &apos;tests&apos;, indicating that a piece of software code is verified by a set of test code.</skos:definition>
    </owl:ObjectProperty>
    


    <!-- http://web-development-ontology.netlify.app/wdo#isTypeOf -->


    <owl:ObjectProperty rdf:about="http://web-development-ontology.netlify.app/wdo#isTypeOf">
        <rdfs:domain rdf:resource="http://web-development-ontology.netlify.app/wdo#TypeDeclaration"/>
        <rdfs:range rdf:resource="http://web-development-ontology.netlify.app/wdo#CodeConstruct"/>
        <dc:identifier>WDO_OP:0000061</dc:identifier>
        <rdfs:label xml:lang="en">is type of</rdfs:label>
        <skos:definition xml:lang="en">A relation from a type to the code construct that has that type.</skos:definition>
    </owl:ObjectProperty>
    


    <!-- http://web-development-ontology.netlify.app/wdo#justifies -->


    <owl:ObjectProperty rdf:about="http://web-development-ontology.netlify.app/wdo#justifies">
        <rdfs:domain rdf:resource="http://web-development-ontology.netlify.app/wdo#ArchitecturalDecisionRecord"/>
        <rdfs:range rdf:resource="http://purl.obolibrary.org/obo/BFO_0000001"/>
        <dc:identifier>WDO_OP:0000048</dc:identifier>
        <rdfs:label xml:lang="en">justifies</rdfs:label>
        <skos:definition xml:lang="en">A relation that links an Architectural Decision Record to the architectural component or design choice it justifies.</skos:definition>
    </owl:ObjectProperty>
    


    <!-- http://web-development-ontology.netlify.app/wdo#manipulates -->


    <owl:ObjectProperty rdf:about="http://web-development-ontology.netlify.app/wdo#manipulates">
        <rdfs:domain rdf:resource="http://web-development-ontology.netlify.app/wdo#ProgrammingLanguageCode"/>
        <rdfs:range rdf:resource="http://web-development-ontology.netlify.app/wdo#HTMLCode"/>
        <dc:identifier>WDO_OP:0000019</dc:identifier>
        <rdfs:label xml:lang="en">manipulates</rdfs:label>
        <skos:definition xml:lang="en">A relation indicating that programming language code acts on or modifies HTML code, such as through the Document Object Model (DOM).</skos:definition>
    </owl:ObjectProperty>
    


    <!-- http://web-development-ontology.netlify.app/wdo#modifies -->


    <owl:ObjectProperty rdf:about="http://web-development-ontology.netlify.app/wdo#modifies">
        <rdfs:domain rdf:resource="http://web-development-ontology.netlify.app/wdo#Commit"/>
        <rdfs:range rdf:resource="http://web-development-ontology.netlify.app/wdo#DigitalInformationCarrier"/>
        <dc:identifier>WDO_OP:0000040</dc:identifier>
        <rdfs:label xml:lang="en">modifies</rdfs:label>
        <skos:definition xml:lang="en">A relation between a commit process and the file(s) it changed.</skos:definition>
    </owl:ObjectProperty>
    


    <!-- http://web-development-ontology.netlify.app/wdo#packagesInto -->


    <owl:ObjectProperty rdf:about="http://web-development-ontology.netlify.app/wdo#packagesInto">
        <rdfs:domain rdf:resource="http://web-development-ontology.netlify.app/wdo#BuildScript"/>
        <rdfs:range rdf:resource="http://web-development-ontology.netlify.app/wdo#ArchiveFile"/>
        <dc:identifier>WDO_OP:0000046</dc:identifier>
        <rdfs:label xml:lang="en">packages into</rdfs:label>
        <skos:definition xml:lang="en">A relation from a build script to the final distributable archive artifact it creates (e.g., a JAR, ZIP, wheel).</skos:definition>
    </owl:ObjectProperty>
    


    <!-- http://web-development-ontology.netlify.app/wdo#refersToVariable -->


    <owl:ObjectProperty rdf:about="http://web-development-ontology.netlify.app/wdo#refersToVariable">
        <rdfs:domain rdf:resource="http://web-development-ontology.netlify.app/wdo#Argument"/>
        <rdfs:range rdf:resource="http://web-development-ontology.netlify.app/wdo#VariableDeclaration"/>
        <dc:identifier>WDO_OP:0000101</dc:identifier>
        <rdfs:label xml:lang="en">refers to variable</rdfs:label>
        <skos:definition xml:lang="en">A relation from an Argument node at a callsite to the VariableDeclaration it refers to as an argument value.</skos:definition>
    </owl:ObjectProperty>
    


    <!-- http://web-development-ontology.netlify.app/wdo#specifiesDependency -->


    <owl:ObjectProperty rdf:about="http://web-development-ontology.netlify.app/wdo#specifiesDependency">
        <rdfs:domain>
            <owl:Class>
                <owl:unionOf rdf:parseType="Collection">
                    <rdf:Description rdf:about="http://web-development-ontology.netlify.app/wdo#BuildScript"/>
                    <rdf:Description rdf:about="http://web-development-ontology.netlify.app/wdo#SoftwarePackage"/>
                </owl:unionOf>
            </owl:Class>
        </rdfs:domain>
        <rdfs:range rdf:resource="http://web-development-ontology.netlify.app/wdo#SoftwarePackage"/>
        <dc:identifier>WDO_OP:0000025</dc:identifier>
        <rdfs:label xml:lang="en">specifies dependency</rdfs:label>
        <skos:definition xml:lang="en">A relation indicating that a build script or software package specifies another package as a dependency.</skos:definition>
    </owl:ObjectProperty>
    


    <!-- http://web-development-ontology.netlify.app/wdo#styles -->


    <owl:ObjectProperty rdf:about="http://web-development-ontology.netlify.app/wdo#styles">
        <rdfs:domain rdf:resource="http://web-development-ontology.netlify.app/wdo#CSSCode"/>
        <rdfs:range rdf:resource="http://web-development-ontology.netlify.app/wdo#HTMLCode"/>
        <dc:identifier>WDO_OP:0000027</dc:identifier>
        <rdfs:label xml:lang="en">styles</rdfs:label>
        <skos:definition xml:lang="en">A relation indicating that a CSS entity provides presentation rules for an HTML entity.</skos:definition>
    </owl:ObjectProperty>
    


    <!-- http://web-development-ontology.netlify.app/wdo#tests -->


    <owl:ObjectProperty rdf:about="http://web-development-ontology.netlify.app/wdo#tests">
        <rdfs:domain rdf:resource="http://web-development-ontology.netlify.app/wdo#TestCode"/>
        <rdfs:range rdf:resource="http://web-development-ontology.netlify.app/wdo#SoftwareCode"/>
        <dc:identifier>WDO_OP:0000031</dc:identifier>
        <rdfs:label xml:lang="en">tests</rdfs:label>
        <skos:definition xml:lang="en">A relation between test code and the application code it is intended to verify.</skos:definition>
    </owl:ObjectProperty>
    


    <!-- http://web-development-ontology.netlify.app/wdo#usesDeclaration -->


    <owl:ObjectProperty rdf:about="http://web-development-ontology.netlify.app/wdo#usesDeclaration">
        <rdfs:domain rdf:resource="http://web-development-ontology.netlify.app/wdo#CodeConstruct"/>
        <rdfs:range rdf:resource="http://web-development-ontology.netlify.app/wdo#CodeConstruct"/>
        <dc:identifier>WDO_OP:0000044</dc:identifier>
        <rdfs:label xml:lang="en">uses declaration</rdfs:label>
        <skos:definition xml:lang="en">A relation linking the usage of a variable or type in an expression to its original declaration construct.</skos:definition>
    </owl:ObjectProperty>
    


    <!-- http://web-development-ontology.netlify.app/wdo#usesFramework -->


    <owl:ObjectProperty rdf:about="http://web-development-ontology.netlify.app/wdo#usesFramework">
        <rdfs:domain rdf:resource="http://web-development-ontology.netlify.app/wdo#SoftwareCode"/>
        <rdfs:range rdf:resource="http://web-development-ontology.netlify.app/wdo#SoftwareFramework"/>
        <dc:identifier>WDO_OP:0000023</dc:identifier>
        <rdfs:label xml:lang="en">uses framework</rdfs:label>
        <skos:definition xml:lang="en">A relation indicating that a piece of software code is built upon or makes use of a software framework.</skos:definition>
    </owl:ObjectProperty>
    


    <!-- 
    ///////////////////////////////////////////////////////////////////////////////////////
    //
    // Data properties
    //
    ///////////////////////////////////////////////////////////////////////////////////////
     -->


    


    <!-- http://web-development-ontology.netlify.app/wdo#endsAtLine -->


    <owl:DatatypeProperty rdf:about="http://web-development-ontology.netlify.app/wdo#endsAtLine">
        <rdfs:domain rdf:resource="http://web-development-ontology.netlify.app/wdo#InformationContentEntity"/>
        <rdfs:range rdf:resource="http://www.w3.org/2001/XMLSchema#nonNegativeInteger"/>
        <dc:identifier>WDO_DP:0000003</dc:identifier>
        <rdfs:label xml:lang="en">ends at line</rdfs:label>
        <skos:definition xml:lang="en">A data property that specifies the ending line number of an information entity within its source file.</skos:definition>
    </owl:DatatypeProperty>
    


    <!-- http://web-development-ontology.netlify.app/wdo#hasAccessModifier -->


    <owl:DatatypeProperty rdf:about="http://web-development-ontology.netlify.app/wdo#hasAccessModifier">
        <rdfs:domain>
            <owl:Class>
                <owl:unionOf rdf:parseType="Collection">
                    <rdf:Description rdf:about="http://web-development-ontology.netlify.app/wdo#AttributeDeclaration"/>
                    <rdf:Description rdf:about="http://web-development-ontology.netlify.app/wdo#FunctionDefinition"/>
                </owl:unionOf>
            </owl:Class>
        </rdfs:domain>
        <rdfs:range rdf:resource="http://www.w3.org/2001/XMLSchema#string"/>
        <dc:identifier>WDO_DP:0000033</dc:identifier>
        <rdfs:label xml:lang="en">has access modifier</rdfs:label>
        <skos:definition xml:lang="en">A data property that specifies the visibility of a field or method (e.g., &quot;public&quot;, &quot;private&quot;, &quot;protected&quot;).</skos:definition>
    </owl:DatatypeProperty>
    


    <!-- http://web-development-ontology.netlify.app/wdo#hasCanonicalName -->


    <owl:DatatypeProperty rdf:about="http://web-development-ontology.netlify.app/wdo#hasCanonicalName">
        <rdfs:domain rdf:resource="http://web-development-ontology.netlify.app/wdo#SoftwareCode"/>
        <rdfs:range rdf:resource="http://www.w3.org/2001/XMLSchema#string"/>
        <dc:identifier>WDO_DP:0000004</dc:identifier>
        <rdfs:label xml:lang="en">has canonical name</rdfs:label>
        <skos:definition xml:lang="en">A data property that specifies the fully qualified or canonical name of a code element (e.g., package.class.method).</skos:definition>
    </owl:DatatypeProperty>
    


    <!-- http://web-development-ontology.netlify.app/wdo#hasCommitHash -->


    <owl:DatatypeProperty rdf:about="http://web-development-ontology.netlify.app/wdo#hasCommitHash">
        <rdfs:domain rdf:resource="http://web-development-ontology.netlify.app/wdo#Commit"/>
        <rdfs:range rdf:resource="http://www.w3.org/2001/XMLSchema#string"/>
        <dc:identifier>WDO_DP:0000024</dc:identifier>
        <rdfs:label xml:lang="en">has commit hash</rdfs:label>
        <skos:definition xml:lang="en">A data property that specifies the unique SHA hash identifying a commit process.</skos:definition>
    </owl:DatatypeProperty>
    


    <!-- http://web-development-ontology.netlify.app/wdo#hasContent -->


    <owl:DatatypeProperty rdf:about="http://web-development-ontology.netlify.app/wdo#hasContent">
        <rdfs:domain>
            <owl:Class>
                <owl:unionOf rdf:parseType="Collection">
                    <rdf:Description rdf:about="http://web-development-ontology.netlify.app/wdo#CommitMessage"/>
                    <rdf:Description rdf:about="http://web-development-ontology.netlify.app/wdo#ConfigurationSetting"/>
                </owl:unionOf>
            </owl:Class>
        </rdfs:domain>
        <rdfs:range rdf:resource="http://www.w3.org/2001/XMLSchema#string"/>
        <dc:identifier>WDO_DP:0000020</dc:identifier>
        <rdfs:label xml:lang="en">has content</rdfs:label>
        <skos:definition xml:lang="en">A data property that holds the literal content of an information entity, such as a configuration setting or commit message.</skos:definition>
    </owl:DatatypeProperty>
    


    <!-- http://web-development-ontology.netlify.app/wdo#hasCreationTimestamp -->


    <owl:DatatypeProperty rdf:about="http://web-development-ontology.netlify.app/wdo#hasCreationTimestamp">
        <rdfs:domain rdf:resource="http://web-development-ontology.netlify.app/wdo#DigitalInformationCarrier"/>
        <rdfs:range rdf:resource="http://www.w3.org/2001/XMLSchema#dateTime"/>
        <dc:identifier>WDO_DP:0000026</dc:identifier>
        <rdfs:label xml:lang="en">has creation timestamp</rdfs:label>
        <skos:definition xml:lang="en">A data property that specifies the timestamp when a file was first created.</skos:definition>
    </owl:DatatypeProperty>
    


    <!-- http://web-development-ontology.netlify.app/wdo#hasCyclomaticComplexity -->


    <owl:DatatypeProperty rdf:about="http://web-development-ontology.netlify.app/wdo#hasCyclomaticComplexity">
        <rdfs:domain rdf:resource="http://web-development-ontology.netlify.app/wdo#FunctionDefinition"/>
        <rdfs:range rdf:resource="http://www.w3.org/2001/XMLSchema#positiveInteger"/>
        <dc:identifier>WDO_DP:0000031</dc:identifier>
        <rdfs:label xml:lang="en">has cyclomatic complexity</rdfs:label>
        <skos:definition xml:lang="en">A data property that specifies the quantitative measure of the number of linearly independent paths through a function&apos;s source code.</skos:definition>
    </owl:DatatypeProperty>
    


    <!-- http://web-development-ontology.netlify.app/wdo#hasEndpointPath -->


    <owl:DatatypeProperty rdf:about="http://web-development-ontology.netlify.app/wdo#hasEndpointPath">
        <rdfs:domain rdf:resource="http://web-development-ontology.netlify.app/wdo#APIDocumentation"/>
        <rdfs:range rdf:resource="http://www.w3.org/2001/XMLSchema#string"/>
        <dc:identifier>WDO_DP:0000037</dc:identifier>
        <rdfs:label xml:lang="en">has endpoint path</rdfs:label>
        <skos:definition xml:lang="en">A data property that specifies the URL path for an API endpoint (e.g., &quot;/api/users/{id}&quot;).</skos:definition>
    </owl:DatatypeProperty>
    


    <!-- http://web-development-ontology.netlify.app/wdo#hasExtension -->


    <owl:DatatypeProperty rdf:about="http://web-development-ontology.netlify.app/wdo#hasExtension">
        <rdfs:domain rdf:resource="http://web-development-ontology.netlify.app/wdo#DigitalInformationCarrier"/>
        <rdfs:range rdf:resource="http://www.w3.org/2001/XMLSchema#string"/>
        <dc:identifier>WDO_DP:0000022</dc:identifier>
        <rdfs:label xml:lang="en">has extension</rdfs:label>
        <skos:definition xml:lang="en">A data property that specifies the file extension of a digital information carrier (e.g., &apos;py&apos;, &apos;md&apos;, &apos;png&apos;).</skos:definition>
    </owl:DatatypeProperty>
    


    <!-- http://web-development-ontology.netlify.app/wdo#hasFontFamilyName -->


    <owl:DatatypeProperty rdf:about="http://web-development-ontology.netlify.app/wdo#hasFontFamilyName">
        <rdfs:domain rdf:resource="http://web-development-ontology.netlify.app/wdo#FontDescription"/>
        <rdfs:range rdf:resource="http://www.w3.org/2001/XMLSchema#string"/>
        <dc:identifier>WDO_DP:0000014</dc:identifier>
        <rdfs:label xml:lang="en">has font family name</rdfs:label>
        <skos:definition xml:lang="en">A data property that specifies the family name of a font (e.g., &quot;Arial&quot;, &quot;Times New Roman&quot;).</skos:definition>
    </owl:DatatypeProperty>
    


    <!-- http://web-development-ontology.netlify.app/wdo#hasFontStyle -->


    <owl:DatatypeProperty rdf:about="http://web-development-ontology.netlify.app/wdo#hasFontStyle">
        <rdfs:domain rdf:resource="http://web-development-ontology.netlify.app/wdo#FontDescription"/>
        <rdfs:range rdf:resource="http://www.w3.org/2001/XMLSchema#string"/>
        <dc:identifier>WDO_DP:0000015</dc:identifier>
        <rdfs:label xml:lang="en">has font style</rdfs:label>
        <skos:definition xml:lang="en">A data property that specifies the style of a font (e.g., &quot;Regular&quot;, &quot;Italic&quot;, &quot;Bold&quot;).</skos:definition>
    </owl:DatatypeProperty>
    


    <!-- http://web-development-ontology.netlify.app/wdo#hasFrameRate -->


    <owl:DatatypeProperty rdf:about="http://web-development-ontology.netlify.app/wdo#hasFrameRate">
        <rdfs:domain rdf:resource="http://web-development-ontology.netlify.app/wdo#VideoDescription"/>
        <rdfs:range rdf:resource="http://www.w3.org/2001/XMLSchema#decimal"/>
        <dc:identifier>WDO_DP:0000011</dc:identifier>
        <rdfs:label xml:lang="en">has frame rate</rdfs:label>
        <skos:definition xml:lang="en">A data property that specifies the frame rate of a video asset in frames per second.</skos:definition>
    </owl:DatatypeProperty>
    


    <!-- http://web-development-ontology.netlify.app/wdo#hasHeadingLevel -->


    <owl:DatatypeProperty rdf:about="http://web-development-ontology.netlify.app/wdo#hasHeadingLevel">
        <rdfs:domain rdf:resource="http://web-development-ontology.netlify.app/wdo#Heading"/>
        <rdfs:range rdf:resource="http://www.w3.org/2001/XMLSchema#positiveInteger"/>
        <dc:identifier>WDO_DP:0000016</dc:identifier>
        <rdfs:label xml:lang="en">has heading level</rdfs:label>
        <skos:definition xml:lang="en">A data property that specifies the hierarchical level of a heading in a document (e.g., 1 for h1, 2 for h2).</skos:definition>
    </owl:DatatypeProperty>
    


    <!-- http://web-development-ontology.netlify.app/wdo#hasHttpMethod -->


    <owl:DatatypeProperty rdf:about="http://web-development-ontology.netlify.app/wdo#hasHttpMethod">
        <rdfs:domain rdf:resource="http://web-development-ontology.netlify.app/wdo#APIDocumentation"/>
        <rdfs:range rdf:resource="http://www.w3.org/2001/XMLSchema#string"/>
        <dc:identifier>WDO_DP:0000038</dc:identifier>
        <rdfs:label xml:lang="en">has http method</rdfs:label>
        <skos:definition xml:lang="en">A data property that specifies the allowed HTTP method for an API endpoint (e.g., &quot;GET&quot;, &quot;POST&quot;).</skos:definition>
    </owl:DatatypeProperty>
    


    <!-- http://web-development-ontology.netlify.app/wdo#hasImageFormatName -->


    <owl:DatatypeProperty rdf:about="http://web-development-ontology.netlify.app/wdo#hasImageFormatName">
        <rdfs:domain rdf:resource="http://web-development-ontology.netlify.app/wdo#ImageDescription"/>
        <rdfs:range rdf:resource="http://www.w3.org/2001/XMLSchema#string"/>
        <dc:identifier>WDO_DP:0000009</dc:identifier>
        <rdfs:label xml:lang="en">has image format name</rdfs:label>
        <skos:definition xml:lang="en">A data property that specifies the common name of the image format (e.g., &quot;JPEG&quot;, &quot;PNG&quot;, &quot;SVG&quot;).</skos:definition>
    </owl:DatatypeProperty>
    


    <!-- http://web-development-ontology.netlify.app/wdo#hasImageHeight -->


    <owl:DatatypeProperty rdf:about="http://web-development-ontology.netlify.app/wdo#hasImageHeight">
        <rdfs:domain rdf:resource="http://web-development-ontology.netlify.app/wdo#ImageDescription"/>
        <rdfs:range rdf:resource="http://www.w3.org/2001/XMLSchema#nonNegativeInteger"/>
        <dc:identifier>WDO_DP:0000008</dc:identifier>
        <rdfs:label xml:lang="en">has image height</rdfs:label>
        <skos:definition xml:lang="en">A data property that specifies the height of the image in pixels.</skos:definition>
    </owl:DatatypeProperty>
    


    <!-- http://web-development-ontology.netlify.app/wdo#hasImageWidth -->


    <owl:DatatypeProperty rdf:about="http://web-development-ontology.netlify.app/wdo#hasImageWidth">
        <rdfs:domain rdf:resource="http://web-development-ontology.netlify.app/wdo#ImageDescription"/>
        <rdfs:range rdf:resource="http://www.w3.org/2001/XMLSchema#nonNegativeInteger"/>
        <dc:identifier>WDO_DP:0000007</dc:identifier>
        <rdfs:label xml:lang="en">has image width</rdfs:label>
        <skos:definition xml:lang="en">A data property that specifies the width of the image in pixels.</skos:definition>
    </owl:DatatypeProperty>
    


    <!-- http://web-development-ontology.netlify.app/wdo#hasIssueIdentifier -->


    <owl:DatatypeProperty rdf:about="http://web-development-ontology.netlify.app/wdo#hasIssueIdentifier">
        <rdfs:domain rdf:resource="http://web-development-ontology.netlify.app/wdo#Issue"/>
        <rdfs:range rdf:resource="http://www.w3.org/2001/XMLSchema#string"/>
        <dc:identifier>WDO_DP:0000023</dc:identifier>
        <rdfs:label xml:lang="en">has issue identifier</rdfs:label>
        <skos:definition xml:lang="en">A data property that specifies the unique identifier for an issue from its tracking system (e.g., &quot;PROJ-123&quot;).</skos:definition>
    </owl:DatatypeProperty>
    


    <!-- http://web-development-ontology.netlify.app/wdo#hasLicenseIdentifier -->


    <owl:DatatypeProperty rdf:about="http://web-development-ontology.netlify.app/wdo#hasLicenseIdentifier">
        <rdfs:domain rdf:resource="http://web-development-ontology.netlify.app/wdo#License"/>
        <rdfs:range rdf:resource="http://www.w3.org/2001/XMLSchema#string"/>
        <dc:identifier>WDO_DP:0000018</dc:identifier>
        <rdfs:label xml:lang="en">has license identifier</rdfs:label>
        <skos:definition xml:lang="en">A data property that specifies the standard identifier for a license, preferably its SPDX ID (e.g., &quot;MIT&quot;, &quot;Apache-2.0&quot;).</skos:definition>
    </owl:DatatypeProperty>
    


    <!-- http://web-development-ontology.netlify.app/wdo#hasLineCount -->


    <owl:DatatypeProperty rdf:about="http://web-development-ontology.netlify.app/wdo#hasLineCount">
        <rdfs:domain rdf:resource="http://web-development-ontology.netlify.app/wdo#SoftwareCode"/>
        <rdfs:range rdf:resource="http://www.w3.org/2001/XMLSchema#nonNegativeInteger"/>
        <dc:identifier>WDO_DP:0000029</dc:identifier>
        <rdfs:label xml:lang="en">has line count</rdfs:label>
        <skos:definition xml:lang="en">A data property that specifies the number of lines in a piece of code.</skos:definition>
    </owl:DatatypeProperty>
    


    <!-- http://web-development-ontology.netlify.app/wdo#hasMediaDuration -->


    <owl:DatatypeProperty rdf:about="http://web-development-ontology.netlify.app/wdo#hasMediaDuration">
        <rdfs:domain>
            <owl:Class>
                <owl:unionOf rdf:parseType="Collection">
                    <rdf:Description rdf:about="http://web-development-ontology.netlify.app/wdo#AudioDescription"/>
                    <rdf:Description rdf:about="http://web-development-ontology.netlify.app/wdo#VideoDescription"/>
                </owl:unionOf>
            </owl:Class>
        </rdfs:domain>
        <rdfs:range rdf:resource="http://www.w3.org/2001/XMLSchema#decimal"/>
        <dc:identifier>WDO_DP:0000010</dc:identifier>
        <rdfs:label xml:lang="en">has media duration in seconds</rdfs:label>
        <skos:definition xml:lang="en">A data property that specifies the duration of a time-based media asset, such as video or audio, represented as a decimal number of total seconds.</skos:definition>
    </owl:DatatypeProperty>
    


    <!-- http://web-development-ontology.netlify.app/wdo#hasMediaEncodingFormat -->


    <owl:DatatypeProperty rdf:about="http://web-development-ontology.netlify.app/wdo#hasMediaEncodingFormat">
        <rdfs:domain>
            <owl:Class>
                <owl:unionOf rdf:parseType="Collection">
                    <rdf:Description rdf:about="http://web-development-ontology.netlify.app/wdo#AudioDescription"/>
                    <rdf:Description rdf:about="http://web-development-ontology.netlify.app/wdo#VideoDescription"/>
                </owl:unionOf>
            </owl:Class>
        </rdfs:domain>
        <rdfs:range rdf:resource="http://www.w3.org/2001/XMLSchema#string"/>
        <dc:identifier>WDO_DP:0000012</dc:identifier>
        <rdfs:label xml:lang="en">has media encoding format</rdfs:label>
        <skos:definition xml:lang="en">A data property that specifies the encoding format of a media asset (e.g., &quot;H.264&quot; for video, &quot;AAC&quot; for audio).</skos:definition>
    </owl:DatatypeProperty>
    


    <!-- http://web-development-ontology.netlify.app/wdo#hasModificationTimestamp -->


    <owl:DatatypeProperty rdf:about="http://web-development-ontology.netlify.app/wdo#hasModificationTimestamp">
        <rdfs:domain rdf:resource="http://web-development-ontology.netlify.app/wdo#DigitalInformationCarrier"/>
        <rdfs:range rdf:resource="http://www.w3.org/2001/XMLSchema#dateTime"/>
        <dc:identifier>WDO_DP:0000027</dc:identifier>
        <rdfs:label xml:lang="en">has modification timestamp</rdfs:label>
        <skos:definition xml:lang="en">A data property that specifies the timestamp when a file was last modified.</skos:definition>
    </owl:DatatypeProperty>
    


    <!-- http://web-development-ontology.netlify.app/wdo#hasProgrammingLanguage -->


    <owl:DatatypeProperty rdf:about="http://web-development-ontology.netlify.app/wdo#hasProgrammingLanguage">
        <rdfs:domain rdf:resource="http://web-development-ontology.netlify.app/wdo#ProgrammingLanguageCode"/>
        <rdfs:range rdf:resource="http://www.w3.org/2001/XMLSchema#string"/>
        <dc:identifier>WDO_DP:0000036</dc:identifier>
        <rdfs:label xml:lang="en">has programming language</rdfs:label>
        <skos:definition xml:lang="en">A data property that specifies the name of the programming language (e.g., &quot;Java&quot;, &quot;Python&quot;).</skos:definition>
    </owl:DatatypeProperty>
    


    <!-- http://web-development-ontology.netlify.app/wdo#hasRelativePath -->


    <owl:DatatypeProperty rdf:about="http://web-development-ontology.netlify.app/wdo#hasRelativePath">
        <rdfs:domain rdf:resource="http://web-development-ontology.netlify.app/wdo#DigitalInformationCarrier"/>
        <rdfs:range rdf:resource="http://www.w3.org/2001/XMLSchema#string"/>
        <dc:identifier>WDO_DP:0000017</dc:identifier>
        <rdfs:label xml:lang="en">has relative path</rdfs:label>
        <skos:definition xml:lang="en">A data property that specifies the path of a file relative to the root of its source repository.</skos:definition>
    </owl:DatatypeProperty>
    


    <!-- http://web-development-ontology.netlify.app/wdo#hasSampleRate -->


    <owl:DatatypeProperty rdf:about="http://web-development-ontology.netlify.app/wdo#hasSampleRate">
        <rdfs:domain rdf:resource="http://web-development-ontology.netlify.app/wdo#AudioDescription"/>
        <rdfs:range rdf:resource="http://www.w3.org/2001/XMLSchema#decimal"/>
        <dc:identifier>WDO_DP:0000013</dc:identifier>
        <rdfs:label xml:lang="en">has sample rate</rdfs:label>
        <skos:definition xml:lang="en">A data property that specifies the sample rate of an audio asset in Hertz (Hz).</skos:definition>
    </owl:DatatypeProperty>
    


    <!-- http://web-development-ontology.netlify.app/wdo#hasSimpleName -->


    <owl:DatatypeProperty rdf:about="http://web-development-ontology.netlify.app/wdo#hasSimpleName">
        <rdfs:domain rdf:resource="http://web-development-ontology.netlify.app/wdo#InformationContentEntity"/>
        <rdfs:range rdf:resource="http://www.w3.org/2001/XMLSchema#string"/>
        <dc:identifier>WDO_DP:0000005</dc:identifier>
        <rdfs:label xml:lang="en">has simple name</rdfs:label>
        <skos:definition xml:lang="en">A data property that specifies the simple, unqualified name of an information content entity.</skos:definition>
    </owl:DatatypeProperty>
    


    <!-- http://web-development-ontology.netlify.app/wdo#hasSizeInBytes -->


    <owl:DatatypeProperty rdf:about="http://web-development-ontology.netlify.app/wdo#hasSizeInBytes">
        <rdfs:domain rdf:resource="http://web-development-ontology.netlify.app/wdo#DigitalInformationCarrier"/>
        <rdfs:range rdf:resource="http://www.w3.org/2001/XMLSchema#nonNegativeInteger"/>
        <dc:identifier>WDO_DP:0000019</dc:identifier>
        <rdfs:label xml:lang="en">has size in bytes</rdfs:label>
        <skos:definition xml:lang="en">A data property that specifies the size of a file in bytes.</skos:definition>
    </owl:DatatypeProperty>
    


    <!-- http://web-development-ontology.netlify.app/wdo#hasSourceCodeSnippet -->


    <owl:DatatypeProperty rdf:about="http://web-development-ontology.netlify.app/wdo#hasSourceCodeSnippet">
        <rdfs:domain rdf:resource="http://web-development-ontology.netlify.app/wdo#CodeConstruct"/>
        <rdfs:range rdf:resource="http://www.w3.org/2001/XMLSchema#string"/>
        <dc:identifier>WDO_DP:0000001</dc:identifier>
        <rdfs:label xml:lang="en">has source code snippet</rdfs:label>
        <skos:definition xml:lang="en">A data property that holds the literal source code string of a code construct.</skos:definition>
    </owl:DatatypeProperty>
    


    <!-- http://web-development-ontology.netlify.app/wdo#hasSourceRepositoryURL -->


    <owl:DatatypeProperty rdf:about="http://web-development-ontology.netlify.app/wdo#hasSourceRepositoryURL">
        <rdfs:domain rdf:resource="http://web-development-ontology.netlify.app/wdo#Repository"/>
        <rdfs:range rdf:resource="http://www.w3.org/2001/XMLSchema#anyURI"/>
        <dc:identifier>WDO_DP:0000028</dc:identifier>
        <rdfs:label xml:lang="en">has source repository URL</rdfs:label>
        <skos:definition xml:lang="en">A data property that specifies the URL of the remote repository.</skos:definition>
    </owl:DatatypeProperty>
    


    <!-- http://web-development-ontology.netlify.app/wdo#hasStatus -->


    <owl:DatatypeProperty rdf:about="http://web-development-ontology.netlify.app/wdo#hasStatus">
        <rdfs:domain rdf:resource="http://web-development-ontology.netlify.app/wdo#Issue"/>
        <rdfs:range rdf:resource="http://www.w3.org/2001/XMLSchema#string"/>
        <dc:identifier>WDO_DP:0000039</dc:identifier>
        <rdfs:label xml:lang="en">has status</rdfs:label>
        <skos:definition xml:lang="en">A data property that specifies the current state of an issue (e.g., &quot;Open&quot;, &quot;In Progress&quot;, &quot;Resolved&quot;).</skos:definition>
    </owl:DatatypeProperty>
    


    <!-- http://web-development-ontology.netlify.app/wdo#hasTextValue -->


    <owl:DatatypeProperty rdf:about="http://web-development-ontology.netlify.app/wdo#hasTextValue">
        <rdfs:domain rdf:resource="http://web-development-ontology.netlify.app/wdo#TextualElement"/>
        <rdfs:range rdf:resource="http://www.w3.org/2001/XMLSchema#string"/>
        <dc:identifier>WDO_DP:0000006</dc:identifier>
        <rdfs:label xml:lang="en">has text value</rdfs:label>
        <skos:definition xml:lang="en">A data property that holds the literal text value of a textual document component.</skos:definition>
    </owl:DatatypeProperty>
    


    <!-- http://web-development-ontology.netlify.app/wdo#hasTokenCount -->


    <owl:DatatypeProperty rdf:about="http://web-development-ontology.netlify.app/wdo#hasTokenCount">
        <rdfs:domain rdf:resource="http://web-development-ontology.netlify.app/wdo#SoftwareCode"/>
        <rdfs:range rdf:resource="http://www.w3.org/2001/XMLSchema#nonNegativeInteger"/>
        <dc:identifier>WDO_DP:0000030</dc:identifier>
        <rdfs:label xml:lang="en">has token count</rdfs:label>
        <skos:definition xml:lang="en">A data property that specifies the number of lexical tokens in a piece of code.</skos:definition>
    </owl:DatatypeProperty>
    


    <!-- http://web-development-ontology.netlify.app/wdo#hasVersion -->


    <owl:DatatypeProperty rdf:about="http://web-development-ontology.netlify.app/wdo#hasVersion">
        <rdfs:domain>
            <owl:Class>
                <owl:unionOf rdf:parseType="Collection">
                    <rdf:Description rdf:about="http://web-development-ontology.netlify.app/wdo#SoftwareFramework"/>
                    <rdf:Description rdf:about="http://web-development-ontology.netlify.app/wdo#SoftwarePackage"/>
                </owl:unionOf>
            </owl:Class>
        </rdfs:domain>
        <rdfs:range rdf:resource="http://www.w3.org/2001/XMLSchema#string"/>
        <dc:identifier>WDO_DP:0000025</dc:identifier>
        <rdfs:label xml:lang="en">has version</rdfs:label>
        <skos:definition xml:lang="en">A data property that specifies the version string of a software package or framework (e.g., &quot;16.8.0&quot;, &quot;5.2.3&quot;).</skos:definition>
    </owl:DatatypeProperty>
    


    <!-- http://web-development-ontology.netlify.app/wdo#isAsynchronous -->


    <owl:DatatypeProperty rdf:about="http://web-development-ontology.netlify.app/wdo#isAsynchronous">
        <rdfs:domain rdf:resource="http://web-development-ontology.netlify.app/wdo#FunctionDefinition"/>
        <rdfs:range rdf:resource="http://www.w3.org/2001/XMLSchema#boolean"/>
        <dc:identifier>WDO_DP:0000032</dc:identifier>
        <rdfs:label xml:lang="en">is asynchronous</rdfs:label>
        <skos:definition xml:lang="en">A data property that specifies whether a function is asynchronous, meaning it may not complete its execution immediately.</skos:definition>
    </owl:DatatypeProperty>
    


    <!-- http://web-development-ontology.netlify.app/wdo#isFinal -->


    <owl:DatatypeProperty rdf:about="http://web-development-ontology.netlify.app/wdo#isFinal">
        <rdfs:domain>
            <owl:Class>
                <owl:unionOf rdf:parseType="Collection">
                    <rdf:Description rdf:about="http://web-development-ontology.netlify.app/wdo#AttributeDeclaration"/>
                    <rdf:Description rdf:about="http://web-development-ontology.netlify.app/wdo#ClassDefinition"/>
                </owl:unionOf>
            </owl:Class>
        </rdfs:domain>
        <rdfs:range rdf:resource="http://www.w3.org/2001/XMLSchema#boolean"/>
        <dc:identifier>WDO_DP:0000035</dc:identifier>
        <rdfs:label xml:lang="en">is final</rdfs:label>
        <skos:definition xml:lang="en">A data property that specifies whether a class cannot be subclassed or a field cannot be reassigned.</skos:definition>
    </owl:DatatypeProperty>
    


    <!-- http://web-development-ontology.netlify.app/wdo#isStatic -->


    <owl:DatatypeProperty rdf:about="http://web-development-ontology.netlify.app/wdo#isStatic">
        <rdfs:domain>
            <owl:Class>
                <owl:unionOf rdf:parseType="Collection">
                    <rdf:Description rdf:about="http://web-development-ontology.netlify.app/wdo#AttributeDeclaration"/>
                    <rdf:Description rdf:about="http://web-development-ontology.netlify.app/wdo#FunctionDefinition"/>
                </owl:unionOf>
            </owl:Class>
        </rdfs:domain>
        <rdfs:range rdf:resource="http://www.w3.org/2001/XMLSchema#boolean"/>
        <dc:identifier>WDO_DP:0000034</dc:identifier>
        <rdfs:label xml:lang="en">is static</rdfs:label>
        <skos:definition xml:lang="en">A data property that specifies whether a member belongs to the type itself rather than to an instance of that type.</skos:definition>
    </owl:DatatypeProperty>
    


    <!-- http://web-development-ontology.netlify.app/wdo#startsAtLine -->


    <owl:DatatypeProperty rdf:about="http://web-development-ontology.netlify.app/wdo#startsAtLine">
        <rdfs:domain rdf:resource="http://web-development-ontology.netlify.app/wdo#InformationContentEntity"/>
        <rdfs:range rdf:resource="http://www.w3.org/2001/XMLSchema#nonNegativeInteger"/>
        <dc:identifier>WDO_DP:0000002</dc:identifier>
        <rdfs:label xml:lang="en">starts at line</rdfs:label>
        <skos:definition xml:lang="en">A data property that specifies the starting line number of an information entity within its source file.</skos:definition>
    </owl:DatatypeProperty>
    


    <!-- 
    ///////////////////////////////////////////////////////////////////////////////////////
    //
    // Classes
    //
    ///////////////////////////////////////////////////////////////////////////////////////
     -->


    


    <!-- http://purl.obolibrary.org/obo/BFO_0000001 -->


    <owl:Class rdf:about="http://purl.obolibrary.org/obo/BFO_0000001">
        <dc:identifier>001-BFO</dc:identifier>
        <rdfs:label xml:lang="en">entity</rdfs:label>
        <skos:definition xml:lang="en">(Elucidation) An entity is anything that exists or has existed or will exist</skos:definition>
        <skos:example xml:lang="en">Julius Caesar; the Second World War; your body mass index; Verdi&apos;s Requiem</skos:example>
    </owl:Class>
    


    <!-- http://purl.obolibrary.org/obo/BFO_0000002 -->


    <owl:Class rdf:about="http://purl.obolibrary.org/obo/BFO_0000002">
        <rdfs:subClassOf rdf:resource="http://purl.obolibrary.org/obo/BFO_0000001"/>
        <rdfs:subClassOf>
            <owl:Restriction>
                <owl:onProperty rdf:resource="http://purl.obolibrary.org/obo/BFO_0000176"/>
                <owl:allValuesFrom rdf:resource="http://purl.obolibrary.org/obo/BFO_0000002"/>
            </owl:Restriction>
        </rdfs:subClassOf>
        <owl:disjointWith rdf:resource="http://purl.obolibrary.org/obo/BFO_0000003"/>
        <dc:identifier>008-BFO</dc:identifier>
        <rdfs:label xml:lang="en">continuant</rdfs:label>
        <skos:definition xml:lang="en">(Elucidation) A continuant is an entity that persists, endures, or continues to exist through time while maintaining its identity</skos:definition>
        <skos:example xml:lang="en">A human being; a tennis ball; a cave; a region of space; someone&apos;s temperature</skos:example>
    </owl:Class>
    


    <!-- http://purl.obolibrary.org/obo/BFO_0000003 -->


    <owl:Class rdf:about="http://purl.obolibrary.org/obo/BFO_0000003">
        <rdfs:subClassOf rdf:resource="http://purl.obolibrary.org/obo/BFO_0000001"/>
        <dc:identifier>077-BFO</dc:identifier>
        <rdfs:label xml:lang="en">occurrent</rdfs:label>
        <skos:definition xml:lang="en">(Elucidation) An occurrent is an entity that unfolds itself in time or it is the start or end of such an entity or it is a temporal or spatiotemporal region</skos:definition>
        <skos:example xml:lang="en">As for process, history, process boundary, spatiotemporal region, zero-dimensional temporal region, one-dimensional temporal region, temporal interval, temporal instant.</skos:example>
    </owl:Class>
    


    <!-- http://purl.obolibrary.org/obo/BFO_0000004 -->


    <owl:Class rdf:about="http://purl.obolibrary.org/obo/BFO_0000004">
        <rdfs:subClassOf rdf:resource="http://purl.obolibrary.org/obo/BFO_0000002"/>
        <rdfs:subClassOf>
            <owl:Restriction>
                <owl:onProperty rdf:resource="http://purl.obolibrary.org/obo/BFO_0000176"/>
                <owl:allValuesFrom rdf:resource="http://purl.obolibrary.org/obo/BFO_0000004"/>
            </owl:Restriction>
        </rdfs:subClassOf>
        <dc:identifier>017-BFO</dc:identifier>
        <rdfs:label xml:lang="en">independent continuant</rdfs:label>
        <skos:definition xml:lang="en">b is an independent continuant =Def b is a continuant &amp; there is no c such that b specifically depends on c or b generically depends on c</skos:definition>
        <skos:example xml:lang="en">An atom; a molecule; an organism; a heart; a chair; the bottom right portion of a human torso; a leg; the interior of your mouth; a spatial region; an orchestra</skos:example>
    </owl:Class>
    


    <!-- http://purl.obolibrary.org/obo/BFO_0000006 -->


    <owl:Class rdf:about="http://purl.obolibrary.org/obo/BFO_0000006">
        <rdfs:subClassOf rdf:resource="http://purl.obolibrary.org/obo/BFO_0000141"/>
        <rdfs:subClassOf>
            <owl:Restriction>
                <owl:onProperty rdf:resource="http://purl.obolibrary.org/obo/BFO_0000176"/>
                <owl:allValuesFrom rdf:resource="http://purl.obolibrary.org/obo/BFO_0000006"/>
            </owl:Restriction>
        </rdfs:subClassOf>
        <dc:identifier>035-BFO</dc:identifier>
        <rdfs:label xml:lang="en">spatial region</rdfs:label>
        <skos:definition xml:lang="en">(Elucidation) A spatial region is a continuant entity that is a continuant part of the spatial projection of a portion of spacetime at a given time</skos:definition>
        <skos:example xml:lang="en">As for zero-dimensional spatial region, one-dimensional spatial region, two-dimensional spatial region, three-dimensional spatial region</skos:example>
    </owl:Class>
    


    <!-- http://purl.obolibrary.org/obo/BFO_0000008 -->


    <owl:Class rdf:about="http://purl.obolibrary.org/obo/BFO_0000008">
        <rdfs:subClassOf rdf:resource="http://purl.obolibrary.org/obo/BFO_0000003"/>
        <rdfs:subClassOf>
            <owl:Restriction>
                <owl:onProperty rdf:resource="http://purl.obolibrary.org/obo/BFO_0000132"/>
                <owl:allValuesFrom rdf:resource="http://purl.obolibrary.org/obo/BFO_0000008"/>
            </owl:Restriction>
        </rdfs:subClassOf>
        <rdfs:subClassOf>
            <owl:Restriction>
                <owl:onProperty rdf:resource="http://purl.obolibrary.org/obo/BFO_0000139"/>
                <owl:allValuesFrom rdf:resource="http://purl.obolibrary.org/obo/BFO_0000008"/>
            </owl:Restriction>
        </rdfs:subClassOf>
        <dc:identifier>100-BFO</dc:identifier>
        <rdfs:label xml:lang="en">temporal region</rdfs:label>
        <skos:definition xml:lang="en">(Elucidation) A temporal region is an occurrent over which processes can unfold</skos:definition>
        <skos:example xml:lang="en">As for zero-dimensional temporal region and one-dimensional temporal region</skos:example>
    </owl:Class>
    


    <!-- http://purl.obolibrary.org/obo/BFO_0000009 -->


    <owl:Class rdf:about="http://purl.obolibrary.org/obo/BFO_0000009">
        <rdfs:subClassOf rdf:resource="http://purl.obolibrary.org/obo/BFO_0000006"/>
        <rdfs:subClassOf>
            <owl:Restriction>
                <owl:onProperty rdf:resource="http://purl.obolibrary.org/obo/BFO_0000178"/>
                <owl:allValuesFrom>
                    <owl:Class>
                        <owl:unionOf rdf:parseType="Collection">
                            <rdf:Description rdf:about="http://purl.obolibrary.org/obo/BFO_0000009"/>
                            <rdf:Description rdf:about="http://purl.obolibrary.org/obo/BFO_0000018"/>
                            <rdf:Description rdf:about="http://purl.obolibrary.org/obo/BFO_0000026"/>
                        </owl:unionOf>
                    </owl:Class>
                </owl:allValuesFrom>
            </owl:Restriction>
        </rdfs:subClassOf>
        <dc:identifier>039-BFO</dc:identifier>
        <rdfs:label xml:lang="en">two-dimensional spatial region</rdfs:label>
        <skos:definition xml:lang="en">(Elucidation) A two-dimensional spatial region is a spatial region that is a whole consisting of a surface together with zero or more surfaces which may have spatial regions of lower dimension as parts</skos:definition>
        <skos:example xml:lang="en">The surface of a sphere-shaped part of space; an infinitely thin plane in space</skos:example>
    </owl:Class>
    


    <!-- http://purl.obolibrary.org/obo/BFO_0000011 -->


    <owl:Class rdf:about="http://purl.obolibrary.org/obo/BFO_0000011">
        <rdfs:subClassOf rdf:resource="http://purl.obolibrary.org/obo/BFO_0000003"/>
        <rdfs:subClassOf>
            <owl:Restriction>
                <owl:onProperty rdf:resource="http://purl.obolibrary.org/obo/BFO_0000132"/>
                <owl:allValuesFrom rdf:resource="http://purl.obolibrary.org/obo/BFO_0000011"/>
            </owl:Restriction>
        </rdfs:subClassOf>
        <rdfs:subClassOf>
            <owl:Restriction>
                <owl:onProperty rdf:resource="http://purl.obolibrary.org/obo/BFO_0000139"/>
                <owl:allValuesFrom rdf:resource="http://purl.obolibrary.org/obo/BFO_0000011"/>
            </owl:Restriction>
        </rdfs:subClassOf>
        <dc:identifier>095-BFO</dc:identifier>
        <rdfs:label xml:lang="en">spatiotemporal region</rdfs:label>
        <skos:definition xml:lang="en">(Elucidation) A spatiotemporal region is an occurrent that is an occurrent part of spacetime</skos:definition>
        <skos:example xml:lang="en">The spatiotemporal region occupied by the development of a cancer tumour; the spatiotemporal region occupied by an orbiting satellite</skos:example>
        <skos:scopeNote xml:lang="en">&apos;Spacetime&apos; here refers to the maximal instance of the universal spatiotemporal region.</skos:scopeNote>
    </owl:Class>
    


    <!-- http://purl.obolibrary.org/obo/BFO_0000015 -->


    <owl:Class rdf:about="http://purl.obolibrary.org/obo/BFO_0000015">
        <rdfs:subClassOf rdf:resource="http://purl.obolibrary.org/obo/BFO_0000003"/>
        <rdfs:subClassOf>
            <owl:Restriction>
                <owl:onProperty rdf:resource="http://purl.obolibrary.org/obo/BFO_0000117"/>
                <owl:allValuesFrom>
                    <owl:Class>
                        <owl:unionOf rdf:parseType="Collection">
                            <rdf:Description rdf:about="http://purl.obolibrary.org/obo/BFO_0000015"/>
                            <rdf:Description rdf:about="http://purl.obolibrary.org/obo/BFO_0000035"/>
                        </owl:unionOf>
                    </owl:Class>
                </owl:allValuesFrom>
            </owl:Restriction>
        </rdfs:subClassOf>
        <rdfs:subClassOf>
            <owl:Restriction>
                <owl:onProperty rdf:resource="http://purl.obolibrary.org/obo/BFO_0000132"/>
                <owl:allValuesFrom rdf:resource="http://purl.obolibrary.org/obo/BFO_0000015"/>
            </owl:Restriction>
        </rdfs:subClassOf>
        <rdfs:subClassOf>
            <owl:Restriction>
                <owl:onProperty rdf:resource="http://purl.obolibrary.org/obo/BFO_0000139"/>
                <owl:allValuesFrom rdf:resource="http://purl.obolibrary.org/obo/BFO_0000015"/>
            </owl:Restriction>
        </rdfs:subClassOf>
        <dc:identifier>083-BFO</dc:identifier>
        <rdfs:label xml:lang="en">process</rdfs:label>
        <skos:altLabel xml:lang="en">event</skos:altLabel>
        <skos:definition xml:lang="en">(Elucidation) p is a process means p is an occurrent that has some temporal proper part and for some time t, p has some material entity as participant</skos:definition>
        <skos:example xml:lang="en">An act of selling; the life of an organism; a process of sleeping; a process of cell-division; a beating of the heart; a process of meiosis; the taxiing of an aircraft; the programming of a computer</skos:example>
    </owl:Class>
    


    <!-- http://purl.obolibrary.org/obo/BFO_0000016 -->


    <owl:Class rdf:about="http://purl.obolibrary.org/obo/BFO_0000016">
        <rdfs:subClassOf rdf:resource="http://purl.obolibrary.org/obo/BFO_0000017"/>
        <owl:disjointWith rdf:resource="http://purl.obolibrary.org/obo/BFO_0000023"/>
        <dc:identifier>062-BFO</dc:identifier>
        <rdfs:label xml:lang="en">disposition</rdfs:label>
        <skos:altLabel xml:lang="en">internally-grounded realizable entity</skos:altLabel>
        <skos:definition xml:lang="en">(Elucidation) A disposition b is a realizable entity such that if b ceases to exist then its bearer is physically changed &amp; b&apos;s realization occurs when and because this bearer is in some special physical circumstances &amp; this realization occurs in virtue of the bearer&apos;s physical make-up</skos:definition>
        <skos:example xml:lang="en">An atom of element X has the disposition to decay to an atom of element Y; the cell wall is disposed to transport cellular material through endocytosis and exocytosis; certain people have a predisposition to colon cancer; children are innately disposed to categorize objects in certain ways</skos:example>
    </owl:Class>
    


    <!-- http://purl.obolibrary.org/obo/BFO_0000017 -->


    <owl:Class rdf:about="http://purl.obolibrary.org/obo/BFO_0000017">
        <rdfs:subClassOf rdf:resource="http://purl.obolibrary.org/obo/BFO_0000020"/>
        <owl:disjointWith rdf:resource="http://purl.obolibrary.org/obo/BFO_0000019"/>
        <dc:identifier>058-BFO</dc:identifier>
        <rdfs:label xml:lang="en">realizable entity</rdfs:label>
        <skos:definition xml:lang="en">(Elucidation) A realizable entity is a specifically dependent continuant that inheres in some independent continuant which is not a spatial region &amp; which is of a type some instances of which are realized in processes of a correlated type</skos:definition>
        <skos:example xml:lang="en">The role of being a doctor; the role of this boundary to delineate where Utah and Colorado meet; the function of your reproductive organs; the disposition of your blood to coagulate; the disposition of this piece of metal to conduct electricity</skos:example>
    </owl:Class>
    


    <!-- http://purl.obolibrary.org/obo/BFO_0000018 -->


    <owl:Class rdf:about="http://purl.obolibrary.org/obo/BFO_0000018">
        <rdfs:subClassOf rdf:resource="http://purl.obolibrary.org/obo/BFO_0000006"/>
        <rdfs:subClassOf>
            <owl:Restriction>
                <owl:onProperty rdf:resource="http://purl.obolibrary.org/obo/BFO_0000178"/>
                <owl:allValuesFrom rdf:resource="http://purl.obolibrary.org/obo/BFO_0000018"/>
            </owl:Restriction>
        </rdfs:subClassOf>
        <dc:identifier>037-BFO</dc:identifier>
        <rdfs:label xml:lang="en">zero-dimensional spatial region</rdfs:label>
        <skos:definition xml:lang="en">(Elucidation) A zero-dimensional spatial region is one or a collection of more than one spatially disjoint points in space</skos:definition>
        <skos:example xml:lang="en">The spatial region occupied at some time instant by the North Pole</skos:example>
    </owl:Class>
    


    <!-- http://purl.obolibrary.org/obo/BFO_0000019 -->


    <owl:Class rdf:about="http://purl.obolibrary.org/obo/BFO_0000019">
        <rdfs:subClassOf rdf:resource="http://purl.obolibrary.org/obo/BFO_0000020"/>
        <dc:identifier>055-BFO</dc:identifier>
        <rdfs:label xml:lang="en">quality</rdfs:label>
        <skos:definition xml:lang="en">(Elucidation) A quality is a specifically dependent continuant that, in contrast to roles and dispositions, does not require any further process in order to be realized</skos:definition>
        <skos:example xml:lang="en">The colour of a tomato; the ambient temperature of this portion of air; the length of the circumference of your waist; the shape of your nose; the shape of your nostril; the mass of this piece of gold</skos:example>
    </owl:Class>
    


    <!-- http://purl.obolibrary.org/obo/BFO_0000020 -->


    <owl:Class rdf:about="http://purl.obolibrary.org/obo/BFO_0000020">
        <rdfs:subClassOf rdf:resource="http://purl.obolibrary.org/obo/BFO_0000002"/>
        <dc:identifier>050-BFO</dc:identifier>
        <rdfs:label xml:lang="en">specifically dependent continuant</rdfs:label>
        <skos:definition xml:lang="en">b is a specifically dependent continuant =Def b is a continuant &amp; there is some independent continuant c which is not a spatial region &amp; which is such that b specifically depends on c</skos:definition>
        <skos:example xml:lang="en">(with multiple bearers) John&apos;s love for Mary; the ownership relation between John and this statue; the relation of authority between John and his subordinates</skos:example>
        <skos:example xml:lang="en">(with one bearer) The mass of this tomato; the pink colour of a medium rare piece of grilled filet mignon at its centre; the smell of this portion of mozzarella; the disposition of this fish to decay; the role of being a doctor; the function of this heart to pump blood; the shape of this hole</skos:example>
    </owl:Class>
    


    <!-- http://purl.obolibrary.org/obo/BFO_0000023 -->


    <owl:Class rdf:about="http://purl.obolibrary.org/obo/BFO_0000023">
        <rdfs:subClassOf rdf:resource="http://purl.obolibrary.org/obo/BFO_0000017"/>
        <dc:identifier>061-BFO</dc:identifier>
        <rdfs:label xml:lang="en">role</rdfs:label>
        <skos:altLabel xml:lang="en">externally-grounded realizable entity</skos:altLabel>
        <skos:definition xml:lang="en">(Elucidation) A role b is a realizable entity such that b exists because there is some single bearer that is in some special physical, social, or institutional set of circumstances in which this bearer does not have to be &amp; b is not such that, if it ceases to exist, then the physical make-up of the bearer is thereby changed</skos:definition>
        <skos:example xml:lang="en">The priest role; the student role; the role of subject in a clinical trial; the role of a stone in marking a property boundary; the role of a boundary to demarcate two neighbouring administrative territories; the role of a building in serving as a military target</skos:example>
    </owl:Class>
    


    <!-- http://purl.obolibrary.org/obo/BFO_0000024 -->


    <owl:Class rdf:about="http://purl.obolibrary.org/obo/BFO_0000024">
        <rdfs:subClassOf rdf:resource="http://purl.obolibrary.org/obo/BFO_0000040"/>
        <dc:identifier>027-BFO</dc:identifier>
        <rdfs:label xml:lang="en">fiat object part</rdfs:label>
        <skos:definition xml:lang="en">(Elucidation) A fiat object part b is a material entity &amp; such that if b exists then it is continuant part of some object c &amp; demarcated from the remainder of c by one or more fiat surfaces</skos:definition>
        <skos:example xml:lang="en">The upper and lower lobes of the left lung; the dorsal and ventral surfaces of the body; the Western hemisphere of the Earth; the FMA:regional parts of an intact human body</skos:example>
    </owl:Class>
    


    <!-- http://purl.obolibrary.org/obo/BFO_0000026 -->


    <owl:Class rdf:about="http://purl.obolibrary.org/obo/BFO_0000026">
        <rdfs:subClassOf rdf:resource="http://purl.obolibrary.org/obo/BFO_0000006"/>
        <rdfs:subClassOf>
            <owl:Restriction>
                <owl:onProperty rdf:resource="http://purl.obolibrary.org/obo/BFO_0000178"/>
                <owl:allValuesFrom>
                    <owl:Class>
                        <owl:unionOf rdf:parseType="Collection">
                            <rdf:Description rdf:about="http://purl.obolibrary.org/obo/BFO_0000018"/>
                            <rdf:Description rdf:about="http://purl.obolibrary.org/obo/BFO_0000026"/>
                        </owl:unionOf>
                    </owl:Class>
                </owl:allValuesFrom>
            </owl:Restriction>
        </rdfs:subClassOf>
        <dc:identifier>038-BFO</dc:identifier>
        <rdfs:label xml:lang="en">one-dimensional spatial region</rdfs:label>
        <skos:definition xml:lang="en">(Elucidation) A one-dimensional spatial region is a whole consisting of a line together with zero or more lines which may have points as parts</skos:definition>
        <skos:example xml:lang="en">An edge of a cube-shaped portion of space; a line connecting two points; two parallel lines extended in space</skos:example>
    </owl:Class>
    


    <!-- http://purl.obolibrary.org/obo/BFO_0000027 -->


    <owl:Class rdf:about="http://purl.obolibrary.org/obo/BFO_0000027">
        <rdfs:subClassOf rdf:resource="http://purl.obolibrary.org/obo/BFO_0000040"/>
        <dc:identifier>025-BFO</dc:identifier>
        <rdfs:label xml:lang="en">object aggregate</rdfs:label>
        <skos:definition xml:lang="en">(Elucidation) An object aggregate is a material entity consisting exactly of a plurality (≥1) of objects as member parts which together form a unit</skos:definition>
        <skos:example xml:lang="en">The aggregate of the musicians in a symphony orchestra and their instruments; the aggregate of bearings in a constant velocity axle joint; the nitrogen atoms in the atmosphere; a collection of cells in a blood biobank</skos:example>
        <skos:scopeNote>&apos;Exactly&apos; means that there are no parts of the object aggregate other than its member parts.</skos:scopeNote>
        <skos:scopeNote>The unit can, at certain times, consist of exactly one object, for example, when a wolf litter loses all but one of its pups, but it must at some time have a plurality of member parts.</skos:scopeNote>
    </owl:Class>
    


    <!-- http://purl.obolibrary.org/obo/BFO_0000028 -->


    <owl:Class rdf:about="http://purl.obolibrary.org/obo/BFO_0000028">
        <rdfs:subClassOf rdf:resource="http://purl.obolibrary.org/obo/BFO_0000006"/>
        <rdfs:subClassOf>
            <owl:Restriction>
                <owl:onProperty rdf:resource="http://purl.obolibrary.org/obo/BFO_0000178"/>
                <owl:allValuesFrom rdf:resource="http://purl.obolibrary.org/obo/BFO_0000006"/>
            </owl:Restriction>
        </rdfs:subClassOf>
        <dc:identifier>040-BFO</dc:identifier>
        <rdfs:label xml:lang="en">three-dimensional spatial region</rdfs:label>
        <skos:definition xml:lang="en">(Elucidation) A three-dimensional spatial region is a whole consisting of a spatial volume together with zero or more spatial volumes which may have spatial regions of lower dimension as parts</skos:definition>
        <skos:example xml:lang="en">A cube-shaped region of space; a sphere-shaped region of space; the region of space occupied by all and only the planets in the solar system at some point in time</skos:example>
    </owl:Class>
    


    <!-- http://purl.obolibrary.org/obo/BFO_0000029 -->


    <owl:Class rdf:about="http://purl.obolibrary.org/obo/BFO_0000029">
        <rdfs:subClassOf rdf:resource="http://purl.obolibrary.org/obo/BFO_0000141"/>
        <rdfs:subClassOf>
            <owl:Restriction>
                <owl:onProperty rdf:resource="http://purl.obolibrary.org/obo/BFO_0000176"/>
                <owl:allValuesFrom>
                    <owl:Class>
                        <owl:unionOf rdf:parseType="Collection">
                            <rdf:Description rdf:about="http://purl.obolibrary.org/obo/BFO_0000029"/>
                            <rdf:Description rdf:about="http://purl.obolibrary.org/obo/BFO_0000040"/>
                        </owl:unionOf>
                    </owl:Class>
                </owl:allValuesFrom>
            </owl:Restriction>
        </rdfs:subClassOf>
        <rdfs:subClassOf>
            <owl:Restriction>
                <owl:onProperty rdf:resource="http://purl.obolibrary.org/obo/BFO_0000178"/>
                <owl:allValuesFrom>
                    <owl:Class>
                        <owl:unionOf rdf:parseType="Collection">
                            <rdf:Description rdf:about="http://purl.obolibrary.org/obo/BFO_0000029"/>
                            <rdf:Description rdf:about="http://purl.obolibrary.org/obo/BFO_0000140"/>
                        </owl:unionOf>
                    </owl:Class>
                </owl:allValuesFrom>
            </owl:Restriction>
        </rdfs:subClassOf>
        <rdfs:subClassOf>
            <owl:Restriction>
                <owl:onProperty rdf:resource="http://purl.obolibrary.org/obo/BFO_0000210"/>
                <owl:allValuesFrom rdf:resource="http://purl.obolibrary.org/obo/BFO_0000028"/>
            </owl:Restriction>
        </rdfs:subClassOf>
        <dc:identifier>034-BFO</dc:identifier>
        <rdfs:label xml:lang="en">site</rdfs:label>
        <skos:definition xml:lang="en">(Elucidation) A site is a three-dimensional immaterial entity whose boundaries either (partially or wholly) coincide with the boundaries of one or more material entities or have locations determined in relation to some material entity</skos:definition>
        <skos:example xml:lang="en">A hole in a portion of cheese; a rabbit hole; the Grand Canyon; the Piazza San Marco; the kangaroo-joey-containing hole of a kangaroo pouch; your left nostril (a fiat part - the opening - of your left nasal cavity); the lumen of your gut; the hold of a ship; the interior of the trunk of your car; hole in an engineered floor joist</skos:example>
    </owl:Class>
    


    <!-- http://purl.obolibrary.org/obo/BFO_0000030 -->


    <owl:Class rdf:about="http://purl.obolibrary.org/obo/BFO_0000030">
        <rdfs:subClassOf rdf:resource="http://purl.obolibrary.org/obo/BFO_0000040"/>
        <dc:identifier>024-BFO</dc:identifier>
        <rdfs:label xml:lang="en">object</rdfs:label>
        <skos:definition xml:lang="en">(Elucidation) An object is a material entity which manifests causal unity &amp; is of a type instances of which are maximal relative to the sort of causal unity manifested</skos:definition>
        <skos:example xml:lang="en">An organism; a fish tank; a planet; a laptop; a valve; a block of marble; an ice cube</skos:example>
        <skos:scopeNote xml:lang="en">A description of three primary sorts of causal unity is provided in Basic Formal Ontology 2.0. Specification and User Guide</skos:scopeNote>
    </owl:Class>
    


    <!-- http://purl.obolibrary.org/obo/BFO_0000031 -->


    <owl:Class rdf:about="http://purl.obolibrary.org/obo/BFO_0000031">
        <rdfs:subClassOf rdf:resource="http://purl.obolibrary.org/obo/BFO_0000002"/>
        <dc:identifier>074-BFO</dc:identifier>
        <rdfs:label xml:lang="en">generically dependent continuant</rdfs:label>
        <skos:altLabel xml:lang="en">g-dependent continuant</skos:altLabel>
        <skos:definition xml:lang="en">(Elucidation) A generically dependent continuant is an entity that exists in virtue of the fact that there is at least one of what may be multiple copies which is the content or the pattern that multiple copies would share</skos:definition>
        <skos:example xml:lang="en">The pdf file on your laptop; the pdf file that is a copy thereof on my laptop; the sequence of this protein molecule; the sequence that is a copy thereof in that protein molecule; the content that is shared by a string of dots and dashes written on a page and the transmitted Morse code signal; the content of a sentence; an engineering blueprint</skos:example>
    </owl:Class>
    


    <!-- http://purl.obolibrary.org/obo/BFO_0000034 -->


    <owl:Class rdf:about="http://purl.obolibrary.org/obo/BFO_0000034">
        <rdfs:subClassOf rdf:resource="http://purl.obolibrary.org/obo/BFO_0000016"/>
        <dc:identifier>064-BFO</dc:identifier>
        <rdfs:label xml:lang="en">function</rdfs:label>
        <skos:definition xml:lang="en">(Elucidation) A function is a disposition that exists in virtue of its bearer&apos;s physical make-up &amp; this physical make-up is something the bearer possesses because it came into being either through evolution (in the case of natural biological entities) or through intentional design (in the case of artefacts) in order to realize processes of a certain sort</skos:definition>
        <skos:example xml:lang="en">The function of a hammer to drive in nails; the function of a heart pacemaker to regulate the beating of a heart through electricity</skos:example>
    </owl:Class>
    


    <!-- http://purl.obolibrary.org/obo/BFO_0000035 -->


    <owl:Class rdf:about="http://purl.obolibrary.org/obo/BFO_0000035">
        <rdfs:subClassOf rdf:resource="http://purl.obolibrary.org/obo/BFO_0000003"/>
        <rdfs:subClassOf>
            <owl:Restriction>
                <owl:onProperty rdf:resource="http://purl.obolibrary.org/obo/BFO_0000117"/>
                <owl:allValuesFrom rdf:resource="http://purl.obolibrary.org/obo/BFO_0000035"/>
            </owl:Restriction>
        </rdfs:subClassOf>
        <rdfs:subClassOf>
            <owl:Restriction>
                <owl:onProperty rdf:resource="http://purl.obolibrary.org/obo/BFO_0000121"/>
                <owl:allValuesFrom rdf:resource="http://purl.obolibrary.org/obo/BFO_0000035"/>
            </owl:Restriction>
        </rdfs:subClassOf>
        <rdfs:subClassOf>
            <owl:Restriction>
                <owl:onProperty rdf:resource="http://purl.obolibrary.org/obo/BFO_0000132"/>
                <owl:allValuesFrom>
                    <owl:Class>
                        <owl:unionOf rdf:parseType="Collection">
                            <rdf:Description rdf:about="http://purl.obolibrary.org/obo/BFO_0000015"/>
                            <rdf:Description rdf:about="http://purl.obolibrary.org/obo/BFO_0000035"/>
                        </owl:unionOf>
                    </owl:Class>
                </owl:allValuesFrom>
            </owl:Restriction>
        </rdfs:subClassOf>
        <rdfs:subClassOf>
            <owl:Restriction>
                <owl:onProperty rdf:resource="http://purl.obolibrary.org/obo/BFO_0000139"/>
                <owl:allValuesFrom>
                    <owl:Class>
                        <owl:unionOf rdf:parseType="Collection">
                            <rdf:Description rdf:about="http://purl.obolibrary.org/obo/BFO_0000015"/>
                            <rdf:Description rdf:about="http://purl.obolibrary.org/obo/BFO_0000035"/>
                        </owl:unionOf>
                    </owl:Class>
                </owl:allValuesFrom>
            </owl:Restriction>
        </rdfs:subClassOf>
        <dc:identifier>084-BFO</dc:identifier>
        <rdfs:label xml:lang="en">process boundary</rdfs:label>
        <skos:definition xml:lang="en">p is a process boundary =Def p is a temporal part of a process &amp; p has no proper temporal parts</skos:definition>
        <skos:example xml:lang="en">The boundary between the 2nd and 3rd year of your life</skos:example>
    </owl:Class>
    


    <!-- http://purl.obolibrary.org/obo/BFO_0000038 -->


    <owl:Class rdf:about="http://purl.obolibrary.org/obo/BFO_0000038">
        <rdfs:subClassOf rdf:resource="http://purl.obolibrary.org/obo/BFO_0000008"/>
        <rdfs:subClassOf>
            <owl:Restriction>
                <owl:onProperty rdf:resource="http://purl.obolibrary.org/obo/BFO_0000121"/>
                <owl:allValuesFrom>
                    <owl:Class>
                        <owl:unionOf rdf:parseType="Collection">
                            <rdf:Description rdf:about="http://purl.obolibrary.org/obo/BFO_0000038"/>
                            <rdf:Description rdf:about="http://purl.obolibrary.org/obo/BFO_0000148"/>
                        </owl:unionOf>
                    </owl:Class>
                </owl:allValuesFrom>
            </owl:Restriction>
        </rdfs:subClassOf>
        <rdfs:subClassOf>
            <owl:Restriction>
                <owl:onProperty rdf:resource="http://purl.obolibrary.org/obo/BFO_0000139"/>
                <owl:allValuesFrom rdf:resource="http://purl.obolibrary.org/obo/BFO_0000038"/>
            </owl:Restriction>
        </rdfs:subClassOf>
        <owl:disjointWith rdf:resource="http://purl.obolibrary.org/obo/BFO_0000148"/>
        <dc:identifier>103-BFO</dc:identifier>
        <rdfs:label xml:lang="en">one-dimensional temporal region</rdfs:label>
        <skos:definition xml:lang="en">(Elucidation) A one-dimensional temporal region is a temporal region that is a whole that has a temporal interval and zero or more temporal intervals and temporal instants as parts</skos:definition>
        <skos:example xml:lang="en">The temporal region during which a process occurs</skos:example>
    </owl:Class>
    


    <!-- http://purl.obolibrary.org/obo/BFO_0000040 -->


    <owl:Class rdf:about="http://purl.obolibrary.org/obo/BFO_0000040">
        <rdfs:subClassOf rdf:resource="http://purl.obolibrary.org/obo/BFO_0000004"/>
        <rdfs:subClassOf>
            <owl:Restriction>
                <owl:onProperty rdf:resource="http://purl.obolibrary.org/obo/BFO_0000176"/>
                <owl:allValuesFrom rdf:resource="http://purl.obolibrary.org/obo/BFO_0000040"/>
            </owl:Restriction>
        </rdfs:subClassOf>
        <rdfs:subClassOf>
            <owl:Restriction>
                <owl:onProperty rdf:resource="http://purl.obolibrary.org/obo/BFO_0000178"/>
                <owl:allValuesFrom>
                    <owl:Class>
                        <owl:unionOf rdf:parseType="Collection">
                            <rdf:Description rdf:about="http://purl.obolibrary.org/obo/BFO_0000029"/>
                            <rdf:Description rdf:about="http://purl.obolibrary.org/obo/BFO_0000040"/>
                            <rdf:Description rdf:about="http://purl.obolibrary.org/obo/BFO_0000140"/>
                        </owl:unionOf>
                    </owl:Class>
                </owl:allValuesFrom>
            </owl:Restriction>
        </rdfs:subClassOf>
        <owl:disjointWith rdf:resource="http://purl.obolibrary.org/obo/BFO_0000141"/>
        <dc:identifier>019-BFO</dc:identifier>
        <rdfs:label xml:lang="en">material entity</rdfs:label>
        <skos:definition xml:lang="en">(Elucidation) A material entity is an independent continuant has some portion of matter as continuant part</skos:definition>
        <skos:example xml:lang="en">A human being; the undetached arm of a human being; an aggregate of human beings</skos:example>
    </owl:Class>
    


    <!-- http://purl.obolibrary.org/obo/BFO_0000140 -->


    <owl:Class rdf:about="http://purl.obolibrary.org/obo/BFO_0000140">
        <rdfs:subClassOf rdf:resource="http://purl.obolibrary.org/obo/BFO_0000141"/>
        <rdfs:subClassOf>
            <owl:Restriction>
                <owl:onProperty rdf:resource="http://purl.obolibrary.org/obo/BFO_0000124"/>
                <owl:allValuesFrom rdf:resource="http://purl.obolibrary.org/obo/BFO_0000140"/>
            </owl:Restriction>
        </rdfs:subClassOf>
        <rdfs:subClassOf>
            <owl:Restriction>
                <owl:onProperty rdf:resource="http://purl.obolibrary.org/obo/BFO_0000178"/>
                <owl:allValuesFrom rdf:resource="http://purl.obolibrary.org/obo/BFO_0000140"/>
            </owl:Restriction>
        </rdfs:subClassOf>
        <dc:identifier>029-BFO</dc:identifier>
        <rdfs:label xml:lang="en">continuant fiat boundary</rdfs:label>
        <skos:definition xml:lang="en">(Elucidation) A continuant fiat boundary b is an immaterial entity that is of zero, one or two dimensions &amp; such that there is no time t when b has a spatial region as continuant part &amp; whose location is determined in relation to some material entity</skos:definition>
        <skos:example xml:lang="en">As for fiat point, fiat line, fiat surface</skos:example>
    </owl:Class>
    


    <!-- http://purl.obolibrary.org/obo/BFO_0000141 -->


    <owl:Class rdf:about="http://purl.obolibrary.org/obo/BFO_0000141">
        <rdfs:subClassOf rdf:resource="http://purl.obolibrary.org/obo/BFO_0000004"/>
        <dc:identifier>028-BFO</dc:identifier>
        <rdfs:label xml:lang="en">immaterial entity</rdfs:label>
        <skos:definition xml:lang="en">b is an immaterial entity =Def b is an independent continuant which is such that there is no time t when it has a material entity as continuant part</skos:definition>
        <skos:example xml:lang="en">As for fiat point, fiat line, fiat surface, site</skos:example>
    </owl:Class>
    


    <!-- http://purl.obolibrary.org/obo/BFO_0000142 -->


    <owl:Class rdf:about="http://purl.obolibrary.org/obo/BFO_0000142">
        <rdfs:subClassOf rdf:resource="http://purl.obolibrary.org/obo/BFO_0000140"/>
        <rdfs:subClassOf>
            <owl:Restriction>
                <owl:onProperty rdf:resource="http://purl.obolibrary.org/obo/BFO_0000178"/>
                <owl:allValuesFrom>
                    <owl:Class>
                        <owl:unionOf rdf:parseType="Collection">
                            <rdf:Description rdf:about="http://purl.obolibrary.org/obo/BFO_0000142"/>
                            <rdf:Description rdf:about="http://purl.obolibrary.org/obo/BFO_0000147"/>
                        </owl:unionOf>
                    </owl:Class>
                </owl:allValuesFrom>
            </owl:Restriction>
        </rdfs:subClassOf>
        <dc:identifier>032-BFO</dc:identifier>
        <rdfs:label xml:lang="en">fiat line</rdfs:label>
        <skos:definition xml:lang="en">(Elucidation) A fiat line is a one-dimensional continuant fiat boundary that is continuous</skos:definition>
        <skos:example xml:lang="en">The Equator; all geopolitical boundaries; all lines of latitude and longitude; the median sulcus of your tongue; the line separating the outer surface of the mucosa of the lower lip from the outer surface of the skin of the chin</skos:example>
    </owl:Class>
    


    <!-- http://purl.obolibrary.org/obo/BFO_0000145 -->


    <owl:Class rdf:about="http://purl.obolibrary.org/obo/BFO_0000145">
        <rdfs:subClassOf rdf:resource="http://purl.obolibrary.org/obo/BFO_0000019"/>
        <dc:identifier>057-BFO</dc:identifier>
        <rdfs:label xml:lang="en">relational quality</rdfs:label>
        <skos:definition xml:lang="en">b is a relational quality =Def b is a quality &amp; there exists c and d such that c and d are not identical &amp; b specifically depends on c &amp; b specifically depends on d</skos:definition>
        <skos:example xml:lang="en">A marriage bond; an instance of love; an obligation between one person and another</skos:example>
    </owl:Class>
    


    <!-- http://purl.obolibrary.org/obo/BFO_0000146 -->


    <owl:Class rdf:about="http://purl.obolibrary.org/obo/BFO_0000146">
        <rdfs:subClassOf rdf:resource="http://purl.obolibrary.org/obo/BFO_0000140"/>
        <rdfs:subClassOf>
            <owl:Restriction>
                <owl:onProperty rdf:resource="http://purl.obolibrary.org/obo/BFO_0000178"/>
                <owl:allValuesFrom rdf:resource="http://purl.obolibrary.org/obo/BFO_0000140"/>
            </owl:Restriction>
        </rdfs:subClassOf>
        <dc:identifier>033-BFO</dc:identifier>
        <rdfs:label xml:lang="en">fiat surface</rdfs:label>
        <skos:definition xml:lang="en">(Elucidation) A fiat surface is a two-dimensional continuant fiat boundary that is self-connected</skos:definition>
        <skos:example xml:lang="en">The surface of the Earth; the plane separating the smoking from the non-smoking zone in a restaurant</skos:example>
    </owl:Class>
    


    <!-- http://purl.obolibrary.org/obo/BFO_0000147 -->


    <owl:Class rdf:about="http://purl.obolibrary.org/obo/BFO_0000147">
        <rdfs:subClassOf rdf:resource="http://purl.obolibrary.org/obo/BFO_0000140"/>
        <rdfs:subClassOf>
            <owl:Restriction>
                <owl:onProperty rdf:resource="http://purl.obolibrary.org/obo/BFO_0000178"/>
                <owl:allValuesFrom rdf:resource="http://purl.obolibrary.org/obo/BFO_0000147"/>
            </owl:Restriction>
        </rdfs:subClassOf>
        <dc:identifier>031-BFO</dc:identifier>
        <rdfs:label xml:lang="en">fiat point</rdfs:label>
        <skos:definition xml:lang="en">(Elucidation) A fiat point is a zero-dimensional continuant fiat boundary that consists of a single point</skos:definition>
        <skos:example xml:lang="en">The geographic North Pole; the quadripoint where the boundaries of Colorado, Utah, New Mexico and Arizona meet; the point of origin of some spatial coordinate system</skos:example>
    </owl:Class>
    


    <!-- http://purl.obolibrary.org/obo/BFO_0000148 -->


    <owl:Class rdf:about="http://purl.obolibrary.org/obo/BFO_0000148">
        <rdfs:subClassOf rdf:resource="http://purl.obolibrary.org/obo/BFO_0000008"/>
        <rdfs:subClassOf>
            <owl:Restriction>
                <owl:onProperty rdf:resource="http://purl.obolibrary.org/obo/BFO_0000121"/>
                <owl:allValuesFrom rdf:resource="http://purl.obolibrary.org/obo/BFO_0000148"/>
            </owl:Restriction>
        </rdfs:subClassOf>
        <dc:identifier>102-BFO</dc:identifier>
        <rdfs:label xml:lang="en">zero-dimensional temporal region</rdfs:label>
        <skos:definition xml:lang="en">(Elucidation) A zero-dimensional temporal region is a temporal region that is a whole consisting of one or more separated temporal instants as parts</skos:definition>
        <skos:example xml:lang="en">A temporal region that is occupied by a process boundary; the moment at which a finger is detached in an industrial accident</skos:example>
    </owl:Class>
    


    <!-- http://purl.obolibrary.org/obo/BFO_0000182 -->


    <owl:Class rdf:about="http://purl.obolibrary.org/obo/BFO_0000182">
        <rdfs:subClassOf rdf:resource="http://purl.obolibrary.org/obo/BFO_0000015"/>
        <dc:identifier>138-BFO</dc:identifier>
        <rdfs:label xml:lang="en">history</rdfs:label>
        <skos:definition xml:lang="en">(Elucidation) A history is a process that is the sum of the totality of processes taking place in the spatiotemporal region occupied by the material part of a material entity</skos:definition>
        <skos:example xml:lang="en">The life of an organism from the beginning to the end of its existence</skos:example>
    </owl:Class>
    


    <!-- http://purl.obolibrary.org/obo/BFO_0000202 -->


    <owl:Class rdf:about="http://purl.obolibrary.org/obo/BFO_0000202">
        <rdfs:subClassOf rdf:resource="http://purl.obolibrary.org/obo/BFO_0000038"/>
        <dc:identifier>155-BFO</dc:identifier>
        <rdfs:label xml:lang="en">temporal interval</rdfs:label>
        <skos:definition xml:lang="en">(Elucidation) A temporal interval is a one-dimensional temporal region that is continuous, thus without gaps or breaks</skos:definition>
        <skos:example xml:lang="en">The year 2018.</skos:example>
        <skos:scopeNote xml:lang="en">A one-dimensional temporal region can include as parts not only temporal intervals but also temporal instants separated from other parts by gaps.</skos:scopeNote>
    </owl:Class>
    


    <!-- http://purl.obolibrary.org/obo/BFO_0000203 -->


    <owl:Class rdf:about="http://purl.obolibrary.org/obo/BFO_0000203">
        <rdfs:subClassOf rdf:resource="http://purl.obolibrary.org/obo/BFO_0000148"/>
        <dc:identifier>209-BFO</dc:identifier>
        <rdfs:label xml:lang="en">temporal instant</rdfs:label>
        <skos:definition xml:lang="en">(Elucidation) A temporal instant is a zero-dimensional temporal region that has no proper temporal part</skos:definition>
        <skos:example xml:lang="en">The millennium</skos:example>
    </owl:Class>
    


    <!-- http://purl.org/dc/terms/LicenseDocument -->


    <owl:Class rdf:about="http://purl.org/dc/terms/LicenseDocument">
        <owl:equivalentClass rdf:resource="http://web-development-ontology.netlify.app/wdo#License"/>
    </owl:Class>
    


    <!-- http://usefulinc.com/ns/doap#Project -->


    <owl:Class rdf:about="http://usefulinc.com/ns/doap#Project">
        <owl:equivalentClass rdf:resource="http://web-development-ontology.netlify.app/wdo#WebDevelopmentProject"/>
    </owl:Class>
    


    <!-- http://usefulinc.com/ns/doap#Repository -->


    <owl:Class rdf:about="http://usefulinc.com/ns/doap#Repository">
        <owl:equivalentClass rdf:resource="http://web-development-ontology.netlify.app/wdo#Repository"/>
    </owl:Class>
    


    <!-- http://web-development-ontology.netlify.app/wdo#APIDocumentation -->


    <owl:Class rdf:about="http://web-development-ontology.netlify.app/wdo#APIDocumentation">
        <rdfs:subClassOf rdf:resource="http://web-development-ontology.netlify.app/wdo#Documentation"/>
        <rdfs:subClassOf rdf:resource="https://schema.org/APIReference"/>
        <dc:identifier>WDO:0000081</dc:identifier>
        <rdfs:label xml:lang="en">API Documentation</rdfs:label>
        <skos:definition xml:lang="en">An API Documentation is a type of Documentation that describes an Application Programming Interface (API), including its endpoints, methods, parameters, and return values.</skos:definition>
        <skos:example xml:lang="en">A specification generated by Swagger/OpenAPI; documentation for a REST or GraphQL API.</skos:example>
    </owl:Class>
    


    <!-- http://web-development-ontology.netlify.app/wdo#ArchitecturalDecisionRecord -->


    <owl:Class rdf:about="http://web-development-ontology.netlify.app/wdo#ArchitecturalDecisionRecord">
        <rdfs:subClassOf rdf:resource="http://web-development-ontology.netlify.app/wdo#Documentation"/>
        <dc:identifier>WDO:0000082</dc:identifier>
        <rdfs:label xml:lang="en">Architectural Decision Record</rdfs:label>
        <skos:definition xml:lang="en">An Architectural Decision Record is a type of Documentation that captures an important architectural decision made along with its context and consequences.</skos:definition>
    </owl:Class>
    


    <!-- http://web-development-ontology.netlify.app/wdo#ArchiveFile -->


    <owl:Class rdf:about="http://web-development-ontology.netlify.app/wdo#ArchiveFile">
        <rdfs:subClassOf rdf:resource="http://web-development-ontology.netlify.app/wdo#DigitalInformationCarrier"/>
        <rdfs:subClassOf rdf:resource="https://schema.org/ArchiveComponent"/>
        <dc:identifier>WDO:0000111</dc:identifier>
        <rdfs:label xml:lang="en">Archive File</rdfs:label>
        <skos:definition xml:lang="en">An Archive File is a Digital Information Carrier that packages and optionally compresses one or more other files into a single file.</skos:definition>
        <skos:example xml:lang="en">A file named &apos;project.zip&apos;, &apos;backup.tar.gz&apos;, &apos;library.jar&apos;, or &apos;archive.7z&apos;.</skos:example>
    </owl:Class>
    


    <!-- http://web-development-ontology.netlify.app/wdo#Argument -->


    <owl:Class rdf:about="http://web-development-ontology.netlify.app/wdo#Argument">
        <rdfs:subClassOf rdf:resource="http://web-development-ontology.netlify.app/wdo#CodeConstruct"/>
        <dc:identifier>WDO:0000120</dc:identifier>
        <rdfs:label xml:lang="en">Argument</rdfs:label>
        <skos:definition xml:lang="en">An Argument is a CodeConstruct representing the use of a value (variable, attribute, or literal) as an argument at a specific function callsite. It may refer to a VariableDeclaration, AttributeDeclaration, or be a literal value.</skos:definition>
    </owl:Class>
    


    <!-- http://web-development-ontology.netlify.app/wdo#AssetFile -->


    <owl:Class rdf:about="http://web-development-ontology.netlify.app/wdo#AssetFile">
        <rdfs:subClassOf rdf:resource="http://web-development-ontology.netlify.app/wdo#DigitalInformationCarrier"/>
        <rdfs:subClassOf rdf:resource="https://schema.org/MediaObject"/>
        <dc:identifier>WDO:0000036</dc:identifier>
        <rdfs:label xml:lang="en">Asset File</rdfs:label>
        <skos:definition xml:lang="en">An Asset File is a Digital Information Carrier that bears the content of a non-code, non-documentation digital resource, such as an image, video, or font. This is an abstract class.</skos:definition>
        <skos:example xml:lang="en">An image file &apos;hero-banner.jpg&apos;; an audio file &apos;notification.mp3&apos;; a font file &apos;Roboto-Regular.ttf&apos;.</skos:example>
    </owl:Class>
    


    <!-- http://web-development-ontology.netlify.app/wdo#AttributeDeclaration -->


    <owl:Class rdf:about="http://web-development-ontology.netlify.app/wdo#AttributeDeclaration">
        <rdfs:subClassOf rdf:resource="http://web-development-ontology.netlify.app/wdo#CodeConstruct"/>
        <rdfs:subClassOf rdf:resource="https://schema.org/PropertyValue"/>
        <dc:identifier>WDO:0000010</dc:identifier>
        <rdfs:label xml:lang="en">Attribute Declaration</rdfs:label>
        <skos:definition xml:lang="en">An Attribute Declaration is a Code Construct which is the declaration of a field, attribute, or property within a class, struct, or interface.</skos:definition>
        <skos:example xml:lang="en">The declaration &apos;private String username;&apos; within a Java class; &apos;const API_KEY = &quot;...&quot;&apos; in a JavaScript module.</skos:example>
    </owl:Class>
    


    <!-- http://web-development-ontology.netlify.app/wdo#AudioDescription -->


    <owl:Class rdf:about="http://web-development-ontology.netlify.app/wdo#AudioDescription">
        <rdfs:subClassOf rdf:resource="http://web-development-ontology.netlify.app/wdo#DigitalAssetDescription"/>
        <dc:identifier>WDO:0000026</dc:identifier>
        <rdfs:label xml:lang="en">Audio Description</rdfs:label>
        <skos:definition xml:lang="en">An Audio Description is a Digital Asset Description that represents the informational nature of an audio recording, such as its duration, sample rate, and encoding.</skos:definition>
    </owl:Class>
    


    <!-- http://web-development-ontology.netlify.app/wdo#AudioFile -->


    <owl:Class rdf:about="http://web-development-ontology.netlify.app/wdo#AudioFile">
        <rdfs:subClassOf rdf:resource="http://web-development-ontology.netlify.app/wdo#AssetFile"/>
        <rdfs:subClassOf rdf:resource="https://schema.org/AudioObject"/>
        <dc:identifier>WDO:0000039</dc:identifier>
        <rdfs:label xml:lang="en">Audio File</rdfs:label>
        <skos:definition xml:lang="en">An Audio File is an Asset File that bears an Audio Description.</skos:definition>
        <skos:example xml:lang="en">A file named &apos;ui_click.wav&apos; or &apos;theme_song.ogg&apos;.</skos:example>
    </owl:Class>
    


    <!-- http://web-development-ontology.netlify.app/wdo#BestPracticeGuideline -->


    <owl:Class rdf:about="http://web-development-ontology.netlify.app/wdo#BestPracticeGuideline">
        <rdfs:subClassOf rdf:resource="http://web-development-ontology.netlify.app/wdo#Documentation"/>
        <rdfs:subClassOf rdf:resource="https://schema.org/HowTo"/>
        <dc:identifier>WDO:0000021</dc:identifier>
        <rdfs:label xml:lang="en">Best Practice Guideline</rdfs:label>
        <skos:definition xml:lang="en">A Best Practice Guideline is a type of Documentation that describes recommended methods or techniques for development.</skos:definition>
        <skos:example xml:lang="en">A document outlining &apos;Secure Coding Practices&apos;; a style guide for writing maintainable CSS.</skos:example>
    </owl:Class>
    


    <!-- http://web-development-ontology.netlify.app/wdo#Blockquote -->


    <owl:Class rdf:about="http://web-development-ontology.netlify.app/wdo#Blockquote">
        <rdfs:subClassOf rdf:resource="http://web-development-ontology.netlify.app/wdo#TextualElement"/>
        <dc:identifier>WDO:0000057</dc:identifier>
        <rdfs:label xml:lang="en">Blockquote</rdfs:label>
        <skos:definition xml:lang="en">A Blockquote is a Textual Element which consists of a block of quoted text.</skos:definition>
        <skos:example xml:lang="en">A customer testimonial quoted in a README file, often prefixed with &apos;&gt;&apos; in Markdown.</skos:example>
    </owl:Class>
    


    <!-- http://web-development-ontology.netlify.app/wdo#BuildFile -->


    <owl:Class rdf:about="http://web-development-ontology.netlify.app/wdo#BuildFile">
        <rdfs:subClassOf rdf:resource="http://web-development-ontology.netlify.app/wdo#DigitalInformationCarrier"/>
        <dc:identifier>WDO:0000049</dc:identifier>
        <rdfs:label xml:lang="en">Build File</rdfs:label>
        <skos:definition xml:lang="en">A Build File is a Digital Information Carrier that bears a Build Script.</skos:definition>
        <skos:example xml:lang="en">A file named &apos;pom.xml&apos; (Maven), &apos;build.gradle&apos; (Gradle), or &apos;Makefile&apos;.</skos:example>
    </owl:Class>
    


    <!-- http://web-development-ontology.netlify.app/wdo#BuildScript -->


    <owl:Class rdf:about="http://web-development-ontology.netlify.app/wdo#BuildScript">
        <rdfs:subClassOf rdf:resource="http://web-development-ontology.netlify.app/wdo#InformationContentEntity"/>
        <rdfs:subClassOf rdf:resource="https://schema.org/SoftwareSourceCode"/>
        <dc:identifier>WDO:0000070</dc:identifier>
        <rdfs:label xml:lang="en">Build Script</rdfs:label>
        <skos:definition xml:lang="en">A Build Script is an Information Content Entity that specifies the instructions, tasks, and dependencies for a build system to compile, test, and package a software project.</skos:definition>
        <skos:example xml:lang="en">The XML content of a pom.xml file defining project dependencies; the Groovy script within a build.gradle file.</skos:example>
    </owl:Class>
    


    <!-- http://web-development-ontology.netlify.app/wdo#CSSCode -->


    <owl:Class rdf:about="http://web-development-ontology.netlify.app/wdo#CSSCode">
        <rdfs:subClassOf rdf:resource="http://web-development-ontology.netlify.app/wdo#Stylesheet"/>
        <dc:identifier>WDO:0000076</dc:identifier>
        <rdfs:label xml:lang="en">CSS Code</rdfs:label>
        <skos:definition xml:lang="en">A CSS Code is a Stylesheet written in the Cascading Style Sheets (CSS) language.</skos:definition>
    </owl:Class>
    


    <!-- http://web-development-ontology.netlify.app/wdo#CSSFramework -->


    <owl:Class rdf:about="http://web-development-ontology.netlify.app/wdo#CSSFramework">
        <rdfs:subClassOf rdf:resource="http://web-development-ontology.netlify.app/wdo#SoftwareFramework"/>
        <dc:identifier>WDO:0000093</dc:identifier>
        <rdfs:label xml:lang="en">CSS Framework</rdfs:label>
        <skos:definition xml:lang="en">A CSS Framework is a Software Framework that provides a collection of pre-written CSS files and other assets to facilitate web design.</skos:definition>
        <skos:example xml:lang="en">Bootstrap, Foundation, Tailwind CSS.</skos:example>
    </owl:Class>
    


    <!-- http://web-development-ontology.netlify.app/wdo#CSharpCode -->


    <owl:Class rdf:about="http://web-development-ontology.netlify.app/wdo#CSharpCode">
        <rdfs:subClassOf rdf:resource="http://web-development-ontology.netlify.app/wdo#StaticallyTypedLanguageCode"/>
        <dc:identifier>WDO:0000101</dc:identifier>
        <rdfs:label xml:lang="en">C# Code</rdfs:label>
        <skos:definition xml:lang="en">A C# Code is a Statically Typed Language Code written in the C# programming language.</skos:definition>
    </owl:Class>
    


    <!-- http://web-development-ontology.netlify.app/wdo#Changelog -->


    <owl:Class rdf:about="http://web-development-ontology.netlify.app/wdo#Changelog">
        <rdfs:subClassOf rdf:resource="http://web-development-ontology.netlify.app/wdo#Documentation"/>
        <dc:identifier>WDO:0000083</dc:identifier>
        <rdfs:label xml:lang="en">Changelog</rdfs:label>
        <skos:definition xml:lang="en">A Changelog is a type of Documentation that consists of a chronologically ordered list of notable changes made to a project.</skos:definition>
    </owl:Class>
    


    <!-- http://web-development-ontology.netlify.app/wdo#ClassDefinition -->


    <owl:Class rdf:about="http://web-development-ontology.netlify.app/wdo#ClassDefinition">
        <rdfs:subClassOf rdf:resource="http://web-development-ontology.netlify.app/wdo#ComplexType"/>
        <dc:identifier>WDO:0000007</dc:identifier>
        <rdfs:label xml:lang="en">Class Definition</rdfs:label>
        <skos:definition xml:lang="en">A Class Definition is a Complex Type which is the specification of a class, defining a template for objects with data attributes and methods.</skos:definition>
        <skos:example xml:lang="en">The complete source code defining the &apos;OrderProcessor&apos; class.</skos:example>
    </owl:Class>
    


    <!-- http://web-development-ontology.netlify.app/wdo#CodeBlock -->


    <owl:Class rdf:about="http://web-development-ontology.netlify.app/wdo#CodeBlock">
        <rdfs:subClassOf rdf:resource="http://web-development-ontology.netlify.app/wdo#TextualElement"/>
        <dc:identifier>WDO:0000019</dc:identifier>
        <rdfs:label xml:lang="en">Code Block</rdfs:label>
        <skos:definition xml:lang="en">A Code Block is a Textual Element which consists of a formatted block of example source code within a document.</skos:definition>
        <skos:example xml:lang="en">A snippet of Python code demonstrating API usage, enclosed in triple backticks in a Markdown file.</skos:example>
    </owl:Class>
    


    <!-- http://web-development-ontology.netlify.app/wdo#CodeComment -->


    <owl:Class rdf:about="http://web-development-ontology.netlify.app/wdo#CodeComment">
        <rdfs:subClassOf rdf:resource="http://web-development-ontology.netlify.app/wdo#Documentation"/>
        <rdfs:subClassOf rdf:resource="https://schema.org/Comment"/>
        <dc:identifier>WDO:0000015</dc:identifier>
        <rdfs:label xml:lang="en">Code Comment</rdfs:label>
        <skos:definition xml:lang="en">A Code Comment is a type of Documentation which is embedded within source code to explain parts of the code.</skos:definition>
        <skos:example xml:lang="en">A Javadoc block above a method; an inline comment like &apos;// Temporary fix for bug #123&apos;.</skos:example>
    </owl:Class>
    


    <!-- http://web-development-ontology.netlify.app/wdo#CodeConstruct -->


    <owl:Class rdf:about="http://web-development-ontology.netlify.app/wdo#CodeConstruct">
        <rdfs:subClassOf rdf:resource="http://web-development-ontology.netlify.app/wdo#SoftwareCode"/>
        <dc:identifier>WDO:0000114</dc:identifier>
        <rdfs:label xml:lang="en">Code Construct</rdfs:label>
        <skos:definition xml:lang="en">A Code Construct is a type of Software Code that represents a syntactically atomic unit of a programming language, such as a type, a function definition, or a declaration. This is an abstract class.</skos:definition>
    </owl:Class>
    


    <!-- http://web-development-ontology.netlify.app/wdo#Commit -->


    <owl:Class rdf:about="http://web-development-ontology.netlify.app/wdo#Commit">
        <rdfs:subClassOf rdf:resource="http://purl.obolibrary.org/obo/BFO_0000015"/>
        <rdfs:subClassOf rdf:resource="https://schema.org/UpdateAction"/>
        <dc:identifier>WDO:0000108</dc:identifier>
        <rdfs:label xml:lang="en">Commit</rdfs:label>
        <skos:definition xml:lang="en">A Commit is a process that records a snapshot of changes to one or more files in a repository at a specific time.</skos:definition>
        <skos:example xml:lang="en">The Git process initiated by `git commit` which creates a new point in the project history.</skos:example>
    </owl:Class>
    


    <!-- http://web-development-ontology.netlify.app/wdo#CommitMessage -->


    <owl:Class rdf:about="http://web-development-ontology.netlify.app/wdo#CommitMessage">
        <rdfs:subClassOf rdf:resource="http://web-development-ontology.netlify.app/wdo#InformationContentEntity"/>
        <rdfs:subClassOf rdf:resource="https://schema.org/Message"/>
        <dc:identifier>WDO:0000113</dc:identifier>
        <rdfs:label xml:lang="en">Commit Message</rdfs:label>
        <skos:definition xml:lang="en">A Commit Message is an Information Content Entity that is a textual description of the changes made in a specific commit process.</skos:definition>
        <skos:example xml:lang="en">&quot;feat: Add user authentication endpoint&quot; or &quot;fix: Correct calculation error in shopping cart (closes #241)&quot;.</skos:example>
    </owl:Class>
    


    <!-- http://web-development-ontology.netlify.app/wdo#ComplexType -->


    <owl:Class rdf:about="http://web-development-ontology.netlify.app/wdo#ComplexType">
        <rdfs:subClassOf rdf:resource="http://web-development-ontology.netlify.app/wdo#TypeDeclaration"/>
        <dc:identifier>WDO:0000006</dc:identifier>
        <rdfs:label xml:lang="en">Complex Type</rdfs:label>
        <skos:definition xml:lang="en">A Complex Type is a Type which represents a composite data type, such as a class, interface, or enumeration. This is an abstract class.</skos:definition>
    </owl:Class>
    


    <!-- http://web-development-ontology.netlify.app/wdo#ConfigurationFile -->


    <owl:Class rdf:about="http://web-development-ontology.netlify.app/wdo#ConfigurationFile">
        <rdfs:subClassOf rdf:resource="http://web-development-ontology.netlify.app/wdo#DigitalInformationCarrier"/>
        <dc:identifier>WDO:0000035</dc:identifier>
        <rdfs:label xml:lang="en">Configuration File</rdfs:label>
        <skos:definition xml:lang="en">A Configuration File is a Digital Information Carrier that bears one or more Configuration Settings.</skos:definition>
        <skos:example xml:lang="en">A &apos;.env&apos; file storing environment variables; a &apos;webpack.config.js&apos; file; a &apos;settings.json&apos; file.</skos:example>
    </owl:Class>
    


    <!-- http://web-development-ontology.netlify.app/wdo#ConfigurationSetting -->


    <owl:Class rdf:about="http://web-development-ontology.netlify.app/wdo#ConfigurationSetting">
        <rdfs:subClassOf rdf:resource="http://web-development-ontology.netlify.app/wdo#InformationContentEntity"/>
        <rdfs:subClassOf rdf:resource="https://schema.org/PropertyValue"/>
        <dc:identifier>WDO:0000022</dc:identifier>
        <rdfs:label xml:lang="en">Configuration Setting</rdfs:label>
        <skos:definition xml:lang="en">A Configuration Setting is an Information Content Entity that is a parameter or setting used to control the behavior of a software application or system.</skos:definition>
        <skos:example xml:lang="en">The content of a &apos;database_url = ...&apos; setting in a .env file; a JSON object defining feature flags.</skos:example>
    </owl:Class>
    


    <!-- http://web-development-ontology.netlify.app/wdo#ContainerImage -->


    <owl:Class rdf:about="http://web-development-ontology.netlify.app/wdo#ContainerImage">
        <rdfs:subClassOf rdf:resource="http://web-development-ontology.netlify.app/wdo#DigitalInformationCarrier"/>
        <rdfs:subClassOf rdf:resource="https://schema.org/SoftwareApplication"/>
        <dc:identifier>WDO:0000110</dc:identifier>
        <rdfs:label xml:lang="en">Container Image</rdfs:label>
        <skos:definition xml:lang="en">A Container Image is a Digital Information Carrier that bears a specification for creating a runnable software container, which is a standalone, executable package including all necessary code, runtime, and tools.</skos:definition>
        <skos:example xml:lang="en">A Docker image such as &apos;nginx:latest&apos; or a custom-built image like &apos;my-app:1.2.0&apos;.</skos:example>
    </owl:Class>
    


    <!-- http://web-development-ontology.netlify.app/wdo#ContributionGuide -->


    <owl:Class rdf:about="http://web-development-ontology.netlify.app/wdo#ContributionGuide">
        <rdfs:subClassOf rdf:resource="http://web-development-ontology.netlify.app/wdo#Guide"/>
        <dc:identifier>WDO:0000084</dc:identifier>
        <rdfs:label xml:lang="en">Contribution Guide</rdfs:label>
        <skos:definition xml:lang="en">A Contribution Guide is a type of Guide that explains how to contribute to a project.</skos:definition>
        <skos:example xml:lang="en">A CONTRIBUTING.md file outlining the process for submitting pull requests.</skos:example>
    </owl:Class>
    


    <!-- http://web-development-ontology.netlify.app/wdo#Contributor -->


    <owl:Class rdf:about="http://web-development-ontology.netlify.app/wdo#Contributor">
        <rdfs:subClassOf rdf:resource="http://xmlns.com/foaf/0.1/Person"/>
        <dc:identifier>WDO:0000124</dc:identifier>
        <rdfs:label xml:lang="en">Contributor</rdfs:label>
        <skos:definition xml:lang="en">A person who has contributed to a project or repository in any capacity, including but not limited to code, documentation, design, or support.</skos:definition>
    </owl:Class>
    


    <!-- http://web-development-ontology.netlify.app/wdo#DataFormat -->


    <owl:Class rdf:about="http://web-development-ontology.netlify.app/wdo#DataFormat">
        <rdfs:subClassOf rdf:resource="http://web-development-ontology.netlify.app/wdo#InformationContentEntity"/>
        <dc:identifier>WDO:0000095</dc:identifier>
        <rdfs:label xml:lang="en">Data Format</rdfs:label>
        <skos:definition xml:lang="en">A Data Format is an Information Content Entity that defines the structure and syntax for serializing data for storage or transmission. This is an abstract class.</skos:definition>
    </owl:Class>
    


    <!-- http://web-development-ontology.netlify.app/wdo#DatabaseSchema -->


    <owl:Class rdf:about="http://web-development-ontology.netlify.app/wdo#DatabaseSchema">
        <rdfs:subClassOf rdf:resource="http://web-development-ontology.netlify.app/wdo#SQLCode"/>
        <dc:identifier>WDO:0000066</dc:identifier>
        <rdfs:label xml:lang="en">Database Schema</rdfs:label>
        <skos:definition xml:lang="en">A Database Schema is a form of SQL Code which defines the structure, tables, columns, and relationships of a database using Data Definition Language (DDL) statements.</skos:definition>
        <skos:example xml:lang="en">The content of a .sql file containing `CREATE TABLE` statements.</skos:example>
    </owl:Class>
    


    <!-- http://web-development-ontology.netlify.app/wdo#DigitalAssetDescription -->


    <owl:Class rdf:about="http://web-development-ontology.netlify.app/wdo#DigitalAssetDescription">
        <rdfs:subClassOf rdf:resource="http://web-development-ontology.netlify.app/wdo#InformationContentEntity"/>
        <dc:identifier>WDO:0000023</dc:identifier>
        <rdfs:label xml:lang="en">Digital Asset Description</rdfs:label>
        <skos:definition xml:lang="en">A Digital Asset Description is an Information Content Entity that defines the characteristics, design, or descriptive metadata for a digital asset. This is an abstract class.</skos:definition>
        <skos:example xml:lang="en">A description for a banner image including its required dimensions; metadata describing an audio clip&apos;s purpose.</skos:example>
    </owl:Class>
    


    <!-- http://web-development-ontology.netlify.app/wdo#DigitalInformationCarrier -->


    <owl:Class rdf:about="http://web-development-ontology.netlify.app/wdo#DigitalInformationCarrier">
        <owl:equivalentClass rdf:resource="https://schema.org/DigitalDocument"/>
        <rdfs:subClassOf rdf:resource="http://purl.obolibrary.org/obo/BFO_0000031"/>
        <dc:identifier>WDO:0000030</dc:identifier>
        <rdfs:label xml:lang="en">Digital Information Carrier</rdfs:label>
        <skos:definition xml:lang="en">A Digital Information Carrier is a generically dependent continuant that is a digital object, typically a file, which serves to encode or bear an Information Content Entity. This is an abstract class.</skos:definition>
        <skos:example xml:lang="en">A specific file named &apos;styles.css&apos;; an image file &apos;logo.png&apos;; a document &apos;API_Guide.pdf&apos;.</skos:example>
    </owl:Class>
    


    <!-- http://web-development-ontology.netlify.app/wdo#Dockerfile -->


    <owl:Class rdf:about="http://web-development-ontology.netlify.app/wdo#Dockerfile">
        <rdfs:subClassOf rdf:resource="http://web-development-ontology.netlify.app/wdo#DigitalInformationCarrier"/>
        <dc:identifier>WDO:0000048</dc:identifier>
        <rdfs:label xml:lang="en">Dockerfile</rdfs:label>
        <skos:definition xml:lang="en">A Dockerfile is a Digital Information Carrier that bears a Dockerfile Specification.</skos:definition>
        <skos:example xml:lang="en">A text file named &apos;Dockerfile&apos; used to build a container image.</skos:example>
    </owl:Class>
    


    <!-- http://web-development-ontology.netlify.app/wdo#DockerfileSpecification -->


    <owl:Class rdf:about="http://web-development-ontology.netlify.app/wdo#DockerfileSpecification">
        <rdfs:subClassOf rdf:resource="http://web-development-ontology.netlify.app/wdo#InformationContentEntity"/>
        <dc:identifier>WDO:0000069</dc:identifier>
        <rdfs:label xml:lang="en">Dockerfile Specification</rdfs:label>
        <skos:definition xml:lang="en">A Dockerfile Specification is an Information Content Entity that is a set of instructions for building a Docker container image.</skos:definition>
        <skos:example xml:lang="en">The sequence of commands like `FROM`, `RUN`, and `COPY` inside a Dockerfile.</skos:example>
    </owl:Class>
    


    <!-- http://web-development-ontology.netlify.app/wdo#DocumentSection -->


    <owl:Class rdf:about="http://web-development-ontology.netlify.app/wdo#DocumentSection">
        <rdfs:subClassOf rdf:resource="http://web-development-ontology.netlify.app/wdo#TextualElement"/>
        <dc:identifier>WDO:0000017</dc:identifier>
        <rdfs:label xml:lang="en">Document Section</rdfs:label>
        <skos:definition xml:lang="en">A Document Section is a Textual Element whose role is to group a set of thematically related textual elements within a larger document.</skos:definition>
        <skos:example xml:lang="en">The &apos;API Endpoints&apos; section in a technical specification document.</skos:example>
    </owl:Class>
    


    <!-- http://web-development-ontology.netlify.app/wdo#Documentation -->


    <owl:Class rdf:about="http://web-development-ontology.netlify.app/wdo#Documentation">
        <rdfs:subClassOf rdf:resource="http://web-development-ontology.netlify.app/wdo#InformationContentEntity"/>
        <rdfs:subClassOf rdf:resource="https://schema.org/TechArticle"/>
        <dc:identifier>WDO:0000013</dc:identifier>
        <rdfs:label xml:lang="en">Documentation</rdfs:label>
        <skos:definition xml:lang="en">Documentation is an Information Content Entity that provides explanatory or reference information about a system, software, or process. This is an abstract class.</skos:definition>
        <skos:example xml:lang="en">The content of a user manual; API documentation generated by Javadoc; inline code comments.</skos:example>
    </owl:Class>
    


    <!-- http://web-development-ontology.netlify.app/wdo#DocumentationFile -->


    <owl:Class rdf:about="http://web-development-ontology.netlify.app/wdo#DocumentationFile">
        <rdfs:subClassOf rdf:resource="http://web-development-ontology.netlify.app/wdo#DigitalInformationCarrier"/>
        <dc:identifier>WDO:0000032</dc:identifier>
        <rdfs:label xml:lang="en">Documentation File</rdfs:label>
        <skos:definition xml:lang="en">A Documentation File is a Digital Information Carrier that primarily bears Documentation.</skos:definition>
        <skos:example xml:lang="en">A &apos;CONTRIBUTING.md&apos; Markdown file; a &apos;user_guide.docx&apos; Word document; a &apos;README.md&apos; file.</skos:example>
    </owl:Class>
    


    <!-- http://web-development-ontology.netlify.app/wdo#EnumDefinition -->


    <owl:Class rdf:about="http://web-development-ontology.netlify.app/wdo#EnumDefinition">
        <rdfs:subClassOf rdf:resource="http://web-development-ontology.netlify.app/wdo#ComplexType"/>
        <rdfs:subClassOf rdf:resource="https://schema.org/Enumeration"/>
        <dc:identifier>WDO:0000060</dc:identifier>
        <rdfs:label xml:lang="en">Enum Definition</rdfs:label>
        <skos:definition xml:lang="en">An Enum Definition is a Complex Type that defines an enumeration, a special data type consisting of a set of named constants.</skos:definition>
        <skos:example xml:lang="en">The definition `enum Status { PENDING, PROCESSING, COMPLETED }` in Java or TypeScript.</skos:example>
    </owl:Class>
    


    <!-- http://web-development-ontology.netlify.app/wdo#FontDescription -->


    <owl:Class rdf:about="http://web-development-ontology.netlify.app/wdo#FontDescription">
        <rdfs:subClassOf rdf:resource="http://web-development-ontology.netlify.app/wdo#DigitalAssetDescription"/>
        <dc:identifier>WDO:0000027</dc:identifier>
        <rdfs:label xml:lang="en">Font Description</rdfs:label>
        <skos:definition xml:lang="en">A Font Description is a Digital Asset Description that defines the characteristics of a font, such as its family name and style.</skos:definition>
    </owl:Class>
    


    <!-- http://web-development-ontology.netlify.app/wdo#FontFile -->


    <owl:Class rdf:about="http://web-development-ontology.netlify.app/wdo#FontFile">
        <rdfs:subClassOf rdf:resource="http://web-development-ontology.netlify.app/wdo#AssetFile"/>
        <dc:identifier>WDO:0000040</dc:identifier>
        <rdfs:label xml:lang="en">Font File</rdfs:label>
        <skos:definition xml:lang="en">A Font File is an Asset File that bears a Font Description.</skos:definition>
        <skos:example xml:lang="en">A file named &apos;MyCustomFont.otf&apos; or &apos;webfont.woff2&apos;.</skos:example>
    </owl:Class>
    


    <!-- http://web-development-ontology.netlify.app/wdo#FunctionCallSite -->


    <owl:Class rdf:about="http://web-development-ontology.netlify.app/wdo#FunctionCallSite">
        <rdfs:subClassOf rdf:resource="http://web-development-ontology.netlify.app/wdo#CodeConstruct"/>
        <dc:identifier>WDO:0000111</dc:identifier>
        <rdfs:label xml:lang="en">Function Call Site</rdfs:label>
        <skos:definition xml:lang="en">A Function Call Site is a Code Construct that represents a single, specific invocation of a function or method.</skos:definition>
        <skos:example xml:lang="en">The specific code `calculatePrice(item, 10)` in a line of a script.</skos:example>
    </owl:Class>
    


    <!-- http://web-development-ontology.netlify.app/wdo#FunctionDefinition -->


    <owl:Class rdf:about="http://web-development-ontology.netlify.app/wdo#FunctionDefinition">
        <rdfs:subClassOf rdf:resource="http://web-development-ontology.netlify.app/wdo#CodeConstruct"/>
        <rdfs:subClassOf rdf:resource="https://schema.org/Function"/>
        <dc:identifier>WDO:0000009</dc:identifier>
        <rdfs:label xml:lang="en">Function Definition</rdfs:label>
        <skos:definition xml:lang="en">A Function Definition is a Code Construct which is the specification of a function, method, or constructor, including its signature and body.</skos:definition>
        <skos:example xml:lang="en">The source code for a &apos;getUserById(userId)&apos; method; the definition of a &apos;Product()&apos; constructor.</skos:example>
    </owl:Class>
    


    <!-- http://web-development-ontology.netlify.app/wdo#GoCode -->


    <owl:Class rdf:about="http://web-development-ontology.netlify.app/wdo#GoCode">
        <rdfs:subClassOf rdf:resource="http://web-development-ontology.netlify.app/wdo#StaticallyTypedLanguageCode"/>
        <dc:identifier>WDO:0000088</dc:identifier>
        <rdfs:label xml:lang="en">Go Code</rdfs:label>
        <skos:definition xml:lang="en">A Go Code is a Statically Typed Language Code written in the Go programming language.</skos:definition>
    </owl:Class>
    


    <!-- http://web-development-ontology.netlify.app/wdo#GraphQLCode -->


    <owl:Class rdf:about="http://web-development-ontology.netlify.app/wdo#GraphQLCode">
        <rdfs:subClassOf rdf:resource="http://web-development-ontology.netlify.app/wdo#QueryLanguageCode"/>
        <dc:identifier>WDO:0000090</dc:identifier>
        <rdfs:label xml:lang="en">GraphQL Code</rdfs:label>
        <skos:definition xml:lang="en">A GraphQL Code is a Query Language Code that is a query or schema written in the GraphQL language.</skos:definition>
    </owl:Class>
    


    <!-- http://web-development-ontology.netlify.app/wdo#Guide -->


    <owl:Class rdf:about="http://web-development-ontology.netlify.app/wdo#Guide">
        <rdfs:subClassOf rdf:resource="http://web-development-ontology.netlify.app/wdo#Documentation"/>
        <rdfs:subClassOf rdf:resource="https://schema.org/HowTo"/>
        <dc:identifier>WDO:0000085</dc:identifier>
        <rdfs:label xml:lang="en">Guide</rdfs:label>
        <skos:definition xml:lang="en">A Guide is a type of Documentation that provides instructions on how to use, set up, or contribute to a project. This is an abstract class.</skos:definition>
    </owl:Class>
    


    <!-- http://web-development-ontology.netlify.app/wdo#HTMLCode -->


    <owl:Class rdf:about="http://web-development-ontology.netlify.app/wdo#HTMLCode">
        <rdfs:subClassOf rdf:resource="http://web-development-ontology.netlify.app/wdo#Markup"/>
        <dc:identifier>WDO:0000078</dc:identifier>
        <rdfs:label xml:lang="en">HTML Code</rdfs:label>
        <skos:definition xml:lang="en">An HTML Code is a Markup written in the HyperText Markup Language (HTML).</skos:definition>
    </owl:Class>
    


    <!-- http://web-development-ontology.netlify.app/wdo#Heading -->


    <owl:Class rdf:about="http://web-development-ontology.netlify.app/wdo#Heading">
        <rdfs:subClassOf rdf:resource="http://web-development-ontology.netlify.app/wdo#TextualElement"/>
        <dc:identifier>WDO:0000055</dc:identifier>
        <rdfs:label xml:lang="en">Heading</rdfs:label>
        <skos:definition xml:lang="en">A Heading is a Textual Element which is the title that introduces a section of a document.</skos:definition>
        <skos:example xml:lang="en">The content of a markdown heading `## Installation`.</skos:example>
    </owl:Class>
    


    <!-- http://web-development-ontology.netlify.app/wdo#ImageDescription -->


    <owl:Class rdf:about="http://web-development-ontology.netlify.app/wdo#ImageDescription">
        <rdfs:subClassOf rdf:resource="http://web-development-ontology.netlify.app/wdo#DigitalAssetDescription"/>
        <dc:identifier>WDO:0000024</dc:identifier>
        <rdfs:label xml:lang="en">Image Description</rdfs:label>
        <skos:definition xml:lang="en">An Image Description is a Digital Asset Description that defines the characteristics of a raster or vector image, such as its dimensions and format.</skos:definition>
    </owl:Class>
    


    <!-- http://web-development-ontology.netlify.app/wdo#ImageFile -->


    <owl:Class rdf:about="http://web-development-ontology.netlify.app/wdo#ImageFile">
        <rdfs:subClassOf rdf:resource="http://web-development-ontology.netlify.app/wdo#AssetFile"/>
        <rdfs:subClassOf rdf:resource="https://schema.org/ImageObject"/>
        <dc:identifier>WDO:0000037</dc:identifier>
        <rdfs:label xml:lang="en">Image File</rdfs:label>
        <skos:definition xml:lang="en">An Image File is an Asset File that bears an Image Description.</skos:definition>
        <skos:example xml:lang="en">A file named &apos;icon.svg&apos; or &apos;background.png&apos;.</skos:example>
    </owl:Class>
    


    <!-- http://web-development-ontology.netlify.app/wdo#ImportDeclaration -->


    <owl:Class rdf:about="http://web-development-ontology.netlify.app/wdo#ImportDeclaration">
        <rdfs:subClassOf rdf:resource="http://web-development-ontology.netlify.app/wdo#CodeConstruct"/>
        <dc:identifier>WDO:0000062</dc:identifier>
        <rdfs:label xml:lang="en">Import Declaration</rdfs:label>
        <skos:definition xml:lang="en">An Import Declaration is a Code Construct that is a statement making entities from another module or package available for use.</skos:definition>
        <skos:example xml:lang="en">The statement `import React from &apos;react&apos;;` in JavaScript or `from collections import Counter` in Python.</skos:example>
    </owl:Class>
    


    <!-- http://web-development-ontology.netlify.app/wdo#InformationContentEntity -->


    <owl:Class rdf:about="http://web-development-ontology.netlify.app/wdo#InformationContentEntity">
        <rdfs:subClassOf rdf:resource="http://purl.obolibrary.org/obo/BFO_0000031"/>
        <rdfs:subClassOf rdf:resource="https://schema.org/CreativeWork"/>
        <dc:identifier>WDO:0000002</dc:identifier>
        <rdfs:label xml:lang="en">Information Content Entity</rdfs:label>
        <skos:definition xml:lang="en">An Information Content Entity is a generically dependent continuant that is dependent on some information bearer for its concretization and is about some entity. This is an abstract class.</skos:definition>
        <skos:example xml:lang="en">The textual content of a specific license agreement; the set of instructions defining a particular JavaScript function; the design description for a company logo.</skos:example>
    </owl:Class>
    


    <!-- http://web-development-ontology.netlify.app/wdo#InterfaceDefinition -->


    <owl:Class rdf:about="http://web-development-ontology.netlify.app/wdo#InterfaceDefinition">
        <rdfs:subClassOf rdf:resource="http://web-development-ontology.netlify.app/wdo#ComplexType"/>
        <dc:identifier>WDO:0000008</dc:identifier>
        <rdfs:label xml:lang="en">Interface Definition</rdfs:label>
        <skos:definition xml:lang="en">An Interface Definition is a Complex Type which is the specification of an abstract type used to define a contract of methods that a class must implement.</skos:definition>
        <skos:example xml:lang="en">The content defining the &apos;Serializable&apos; interface in Java.</skos:example>
    </owl:Class>
    


    <!-- http://web-development-ontology.netlify.app/wdo#InterpretedLanguageCode -->


    <owl:Class rdf:about="http://web-development-ontology.netlify.app/wdo#InterpretedLanguageCode">
        <rdfs:subClassOf rdf:resource="http://web-development-ontology.netlify.app/wdo#ProgrammingLanguageCode"/>
        <dc:identifier>WDO:0000072</dc:identifier>
        <rdfs:label xml:lang="en">Interpreted Language Code</rdfs:label>
        <skos:definition xml:lang="en">An Interpreted Language Code is a Programming Language Code written in a language that is executed by an interpreter without prior compilation. This is an abstract class.</skos:definition>
    </owl:Class>
    


    <!-- http://web-development-ontology.netlify.app/wdo#Issue -->


    <owl:Class rdf:about="http://web-development-ontology.netlify.app/wdo#Issue">
        <rdfs:subClassOf rdf:resource="http://web-development-ontology.netlify.app/wdo#InformationContentEntity"/>
        <dc:identifier>WDO:0000109</dc:identifier>
        <rdfs:label xml:lang="en">Issue</rdfs:label>
        <skos:definition xml:lang="en">An Issue is an Information Content Entity that describes a unit of work to be done, such as a bug, task, or enhancement request in a project.</skos:definition>
        <skos:example xml:lang="en">A bug report titled &quot;User cannot log in with valid credentials&quot; in a Jira or GitHub issue tracker.</skos:example>
    </owl:Class>
    


    <!-- http://web-development-ontology.netlify.app/wdo#JSON -->


    <owl:Class rdf:about="http://web-development-ontology.netlify.app/wdo#JSON">
        <rdfs:subClassOf rdf:resource="http://web-development-ontology.netlify.app/wdo#DataFormat"/>
        <dc:identifier>WDO:0000096</dc:identifier>
        <rdfs:label xml:lang="en">JSON</rdfs:label>
        <skos:definition xml:lang="en">A JSON is a Data Format that structures data according to the JavaScript Object Notation syntax.</skos:definition>
    </owl:Class>
    


    <!-- http://web-development-ontology.netlify.app/wdo#JavaCode -->


    <owl:Class rdf:about="http://web-development-ontology.netlify.app/wdo#JavaCode">
        <rdfs:subClassOf rdf:resource="http://web-development-ontology.netlify.app/wdo#StaticallyTypedLanguageCode"/>
        <dc:identifier>WDO:0000100</dc:identifier>
        <rdfs:label xml:lang="en">Java Code</rdfs:label>
        <skos:definition xml:lang="en">A Java Code is a Statically Typed Language Code written in the Java programming language.</skos:definition>
    </owl:Class>
    


    <!-- http://web-development-ontology.netlify.app/wdo#JavaScriptCode -->


    <owl:Class rdf:about="http://web-development-ontology.netlify.app/wdo#JavaScriptCode">
        <rdfs:subClassOf rdf:resource="http://web-development-ontology.netlify.app/wdo#InterpretedLanguageCode"/>
        <dc:identifier>WDO:0000074</dc:identifier>
        <rdfs:label xml:lang="en">JavaScript Code</rdfs:label>
        <skos:definition xml:lang="en">A JavaScript Code is an Interpreted Language Code written in the JavaScript programming language.</skos:definition>
    </owl:Class>
    


    <!-- http://web-development-ontology.netlify.app/wdo#JavaScriptFramework -->


    <owl:Class rdf:about="http://web-development-ontology.netlify.app/wdo#JavaScriptFramework">
        <rdfs:subClassOf rdf:resource="http://web-development-ontology.netlify.app/wdo#SoftwareFramework"/>
        <dc:identifier>WDO:0000094</dc:identifier>
        <rdfs:label xml:lang="en">JavaScript Framework</rdfs:label>
        <skos:definition xml:lang="en">A JavaScript Framework is a Software Framework written in JavaScript that provides structure for building web applications.</skos:definition>
        <skos:example xml:lang="en">React, Angular, Vue.js.</skos:example>
    </owl:Class>
    


    <!-- http://web-development-ontology.netlify.app/wdo#JupyterNotebook -->


    <owl:Class rdf:about="http://web-development-ontology.netlify.app/wdo#JupyterNotebook">
        <rdfs:subClassOf rdf:resource="http://web-development-ontology.netlify.app/wdo#Notebook"/>
        <dc:identifier>WDO:0000068</dc:identifier>
        <rdfs:label xml:lang="en">Jupyter Notebook</rdfs:label>
        <skos:definition xml:lang="en">A Jupyter Notebook is a type of Notebook that conforms to the .ipynb format structure, containing a list of cells with code, text, and output.</skos:definition>
        <skos:example xml:lang="en">The JSON content of an .ipynb file describing a sequence of executable Python code and Markdown cells for data analysis.</skos:example>
    </owl:Class>
    


    <!-- http://web-development-ontology.netlify.app/wdo#License -->


    <owl:Class rdf:about="http://web-development-ontology.netlify.app/wdo#License">
        <rdfs:subClassOf rdf:resource="http://web-development-ontology.netlify.app/wdo#InformationContentEntity"/>
        <dc:identifier>WDO:0000020</dc:identifier>
        <rdfs:label xml:lang="en">License</rdfs:label>
        <skos:definition xml:lang="en">A License is an Information Content Entity that specifies the terms and conditions for software use, modification, and distribution.</skos:definition>
        <skos:example xml:lang="en">The full text of the MIT License; the specific clauses of the Apache License 2.0.</skos:example>
    </owl:Class>
    


    <!-- http://web-development-ontology.netlify.app/wdo#LicenseFile -->


    <owl:Class rdf:about="http://web-development-ontology.netlify.app/wdo#LicenseFile">
        <rdfs:subClassOf rdf:resource="http://web-development-ontology.netlify.app/wdo#DigitalInformationCarrier"/>
        <dc:identifier>WDO:0000033</dc:identifier>
        <rdfs:label xml:lang="en">License File</rdfs:label>
        <skos:definition xml:lang="en">A License File is a Digital Information Carrier that primarily bears a License.</skos:definition>
        <skos:example xml:lang="en">A file named &apos;LICENSE.txt&apos; containing the MIT license text.</skos:example>
    </owl:Class>
    


    <!-- http://web-development-ontology.netlify.app/wdo#List -->


    <owl:Class rdf:about="http://web-development-ontology.netlify.app/wdo#List">
        <rdfs:subClassOf rdf:resource="http://web-development-ontology.netlify.app/wdo#TextualElement"/>
        <rdfs:subClassOf rdf:resource="https://schema.org/ItemList"/>
        <dc:identifier>WDO:0000056</dc:identifier>
        <rdfs:label xml:lang="en">List</rdfs:label>
        <skos:definition xml:lang="en">A List is a Textual Element which consists of a series of items arranged in a sequence.</skos:definition>
        <skos:example xml:lang="en">An unordered list of features in a README file; an ordered list of installation steps.</skos:example>
    </owl:Class>
    


    <!-- http://web-development-ontology.netlify.app/wdo#Log -->


    <owl:Class rdf:about="http://web-development-ontology.netlify.app/wdo#Log">
        <rdfs:subClassOf rdf:resource="http://web-development-ontology.netlify.app/wdo#InformationContentEntity"/>
        <dc:identifier>WDO:0000071</dc:identifier>
        <rdfs:label xml:lang="en">Log</rdfs:label>
        <skos:definition xml:lang="en">A Log is an Information Content Entity that is a record of events that occurred while a software application was running.</skos:definition>
        <skos:example xml:lang="en">A textual entry like &apos;2025-07-06 12:00:00, ERROR: Database connection failed&apos;.</skos:example>
    </owl:Class>
    


    <!-- http://web-development-ontology.netlify.app/wdo#LogFile -->


    <owl:Class rdf:about="http://web-development-ontology.netlify.app/wdo#LogFile">
        <rdfs:subClassOf rdf:resource="http://web-development-ontology.netlify.app/wdo#DigitalInformationCarrier"/>
        <dc:identifier>WDO:0000050</dc:identifier>
        <rdfs:label xml:lang="en">Log File</rdfs:label>
        <skos:definition xml:lang="en">A Log File is a Digital Information Carrier that bears Log information.</skos:definition>
        <skos:example xml:lang="en">A file named `application.log` or `access.log`.</skos:example>
    </owl:Class>
    


    <!-- http://web-development-ontology.netlify.app/wdo#Markup -->


    <owl:Class rdf:about="http://web-development-ontology.netlify.app/wdo#Markup">
        <rdfs:subClassOf rdf:resource="http://web-development-ontology.netlify.app/wdo#WebPresentationCode"/>
        <dc:identifier>WDO:0000063</dc:identifier>
        <rdfs:label xml:lang="en">Markup</rdfs:label>
        <skos:definition xml:lang="en">A Markup is a type of Web Presentation Code that defines the structure and semantics of a document using a system of tags. This is an abstract class.</skos:definition>
        <skos:example xml:lang="en">An HTML document defining headings, paragraphs, and links.</skos:example>
    </owl:Class>
    


    <!-- http://web-development-ontology.netlify.app/wdo#MarkupFile -->


    <owl:Class rdf:about="http://web-development-ontology.netlify.app/wdo#MarkupFile">
        <rdfs:subClassOf rdf:resource="http://web-development-ontology.netlify.app/wdo#DigitalInformationCarrier"/>
        <dc:identifier>WDO:0000043</dc:identifier>
        <rdfs:label xml:lang="en">Markup File</rdfs:label>
        <skos:definition xml:lang="en">A Markup File is a Digital Information Carrier that bears Markup code.</skos:definition>
        <skos:example xml:lang="en">A file named `index.html`, `main.jsx`, or `document.xml`.</skos:example>
    </owl:Class>
    


    <!-- http://web-development-ontology.netlify.app/wdo#Module -->


    <owl:Class rdf:about="http://web-development-ontology.netlify.app/wdo#Module">
        <rdfs:subClassOf rdf:resource="http://web-development-ontology.netlify.app/wdo#SoftwarePackage"/>
        <dc:identifier>WDO:0000061</dc:identifier>
        <rdfs:label xml:lang="en">Module</rdfs:label>
        <skos:definition xml:lang="en">A Module is a Software Package which is a self-contained unit of code (often corresponding to a single file) that encapsulates related functionality and can be imported for reuse.</skos:definition>
        <skos:example xml:lang="en">A Python file (`utils.py`) or a JavaScript file (`api.js`) that exports functions or classes.</skos:example>
    </owl:Class>
    


    <!-- http://web-development-ontology.netlify.app/wdo#Notebook -->


    <owl:Class rdf:about="http://web-development-ontology.netlify.app/wdo#Notebook">
        <rdfs:subClassOf rdf:resource="http://web-development-ontology.netlify.app/wdo#InformationContentEntity"/>
        <dc:identifier>WDO:0000104</dc:identifier>
        <rdfs:label xml:lang="en">Notebook</rdfs:label>
        <skos:definition xml:lang="en">A Notebook is an Information Content Entity which represents the structured content of a computational notebook, including code cells, documentation, and outputs. This is an abstract class.</skos:definition>
    </owl:Class>
    


    <!-- http://web-development-ontology.netlify.app/wdo#NotebookFile -->


    <owl:Class rdf:about="http://web-development-ontology.netlify.app/wdo#NotebookFile">
        <rdfs:subClassOf rdf:resource="http://web-development-ontology.netlify.app/wdo#DigitalInformationCarrier"/>
        <dc:identifier>WDO:0000047</dc:identifier>
        <rdfs:label xml:lang="en">Notebook File</rdfs:label>
        <skos:definition xml:lang="en">A Notebook File is a Digital Information Carrier that bears Notebook content.</skos:definition>
        <skos:example xml:lang="en">A file named `data_analysis.ipynb`.</skos:example>
    </owl:Class>
    


    <!-- http://web-development-ontology.netlify.app/wdo#Organization -->


    <owl:Class rdf:about="http://web-development-ontology.netlify.app/wdo#Organization">
        <owl:equivalentClass rdf:resource="http://xmlns.com/foaf/0.1/Organization"/>
        <rdfs:subClassOf rdf:resource="http://purl.obolibrary.org/obo/BFO_0000027"/>
        <dc:identifier>WDO:0000112</dc:identifier>
        <rdfs:label xml:lang="en">Organization</rdfs:label>
        <skos:definition xml:lang="en">An Organization is an Object Aggregate whose parts are people and assets, which acts as a social or legal agent to manage projects and own repositories.</skos:definition>
        <skos:example xml:lang="en">A software company like &apos;Thinkster&apos;, the &apos;Apache Software Foundation&apos;, or a university department.</skos:example>
    </owl:Class>
    


    <!-- http://web-development-ontology.netlify.app/wdo#PHPCode -->


    <owl:Class rdf:about="http://web-development-ontology.netlify.app/wdo#PHPCode">
        <rdfs:subClassOf rdf:resource="http://web-development-ontology.netlify.app/wdo#InterpretedLanguageCode"/>
        <dc:identifier>WDO:0000086</dc:identifier>
        <rdfs:label xml:lang="en">PHP Code</rdfs:label>
        <skos:definition xml:lang="en">A PHP Code is an Interpreted Language Code written in the PHP programming language.</skos:definition>
    </owl:Class>
    


    <!-- http://web-development-ontology.netlify.app/wdo#PackageDeclaration -->


    <owl:Class rdf:about="http://web-development-ontology.netlify.app/wdo#PackageDeclaration">
        <rdfs:subClassOf rdf:resource="http://web-development-ontology.netlify.app/wdo#ComplexType"/>
        <dc:identifier>WDO:0000115</dc:identifier>
        <rdfs:label xml:lang="en">Package Declaration</rdfs:label>
        <skos:definition xml:lang="en">A Package Declaration is a Complex Type that is a statement defining the namespace to which a particular code file belongs.</skos:definition>
        <skos:example xml:lang="en">The statement `package com.example.service;` at the top of a Java file.</skos:example>
    </owl:Class>
    


    <!-- http://web-development-ontology.netlify.app/wdo#Paragraph -->


    <owl:Class rdf:about="http://web-development-ontology.netlify.app/wdo#Paragraph">
        <rdfs:subClassOf rdf:resource="http://web-development-ontology.netlify.app/wdo#TextualElement"/>
        <dc:identifier>WDO:0000018</dc:identifier>
        <rdfs:label xml:lang="en">Paragraph</rdfs:label>
        <skos:definition xml:lang="en">A Paragraph is a Textual Element which is a self-contained unit of discourse dealing with a particular point or idea.</skos:definition>
        <skos:example xml:lang="en">A block of text in a README file explaining a specific feature.</skos:example>
    </owl:Class>
    


    <!-- http://web-development-ontology.netlify.app/wdo#Parameter -->


    <owl:Class rdf:about="http://web-development-ontology.netlify.app/wdo#Parameter">
        <rdfs:subClassOf rdf:resource="http://web-development-ontology.netlify.app/wdo#CodeConstruct"/>
        <rdfs:subClassOf rdf:resource="https://schema.org/PropertyValue"/>
        <dc:identifier>WDO:0000011</dc:identifier>
        <rdfs:label xml:lang="en">Parameter</rdfs:label>
        <skos:definition xml:lang="en">A Parameter is a Code Construct which is the specification of a variable bound within the scope of a function or method signature.</skos:definition>
        <skos:example xml:lang="en">The &apos;int count&apos; parameter in a function signature &apos;void printItems(int count)&apos;.</skos:example>
    </owl:Class>
    


    <!-- http://web-development-ontology.netlify.app/wdo#PrimitiveType -->


    <owl:Class rdf:about="http://web-development-ontology.netlify.app/wdo#PrimitiveType">
        <rdfs:subClassOf rdf:resource="http://web-development-ontology.netlify.app/wdo#TypeDeclaration"/>
        <dc:identifier>WDO:0000005</dc:identifier>
        <rdfs:label xml:lang="en">Primitive Type</rdfs:label>
        <skos:definition xml:lang="en">A Primitive Type is a Type which represents a basic data type provided by a programming language, such as an integer, boolean, or string.</skos:definition>
        <skos:example xml:lang="en">The &apos;boolean&apos; type in Python; the &apos;int&apos; type specification in C++.</skos:example>
    </owl:Class>
    


    <!-- http://web-development-ontology.netlify.app/wdo#ProgrammingLanguageCode -->


    <owl:Class rdf:about="http://web-development-ontology.netlify.app/wdo#ProgrammingLanguageCode">
        <rdfs:subClassOf rdf:resource="http://web-development-ontology.netlify.app/wdo#SoftwareCode"/>
        <dc:identifier>WDO:0000117</dc:identifier>
        <rdfs:label xml:lang="en">Programming Language Code</rdfs:label>
        <skos:definition xml:lang="en">A Programming Language Code is a type of Software Code written in a language with formal syntax, typically used to implement application logic. This is an abstract class.</skos:definition>
    </owl:Class>
    


    <!-- http://web-development-ontology.netlify.app/wdo#PythonCode -->


    <owl:Class rdf:about="http://web-development-ontology.netlify.app/wdo#PythonCode">
        <rdfs:subClassOf rdf:resource="http://web-development-ontology.netlify.app/wdo#InterpretedLanguageCode"/>
        <dc:identifier>WDO:0000073</dc:identifier>
        <rdfs:label xml:lang="en">Python Code</rdfs:label>
        <skos:definition xml:lang="en">A Python Code is an Interpreted Language Code written in the Python programming language.</skos:definition>
    </owl:Class>
    


    <!-- http://web-development-ontology.netlify.app/wdo#QueryLanguageCode -->


    <owl:Class rdf:about="http://web-development-ontology.netlify.app/wdo#QueryLanguageCode">
        <rdfs:subClassOf rdf:resource="http://web-development-ontology.netlify.app/wdo#ProgrammingLanguageCode"/>
        <dc:identifier>WDO:0000091</dc:identifier>
        <rdfs:label xml:lang="en">Query Language Code</rdfs:label>
        <skos:definition xml:lang="en">A Query Language Code is a Programming Language Code written in a language used to make queries in databases and information systems. This is an abstract class.</skos:definition>
    </owl:Class>
    


    <!-- http://web-development-ontology.netlify.app/wdo#Readme -->


    <owl:Class rdf:about="http://web-development-ontology.netlify.app/wdo#Readme">
        <rdfs:subClassOf rdf:resource="http://web-development-ontology.netlify.app/wdo#Documentation"/>
        <dc:identifier>WDO:0000014</dc:identifier>
        <rdfs:label xml:lang="en">Readme</rdfs:label>
        <skos:definition xml:lang="en">A Readme is a type of Documentation that provides essential information about a software project, typically serving as the entry point for a repository.</skos:definition>
        <skos:example xml:lang="en">The textual content and structure within a &apos;README.md&apos; file, including sections like &apos;Installation&apos; and &apos;Usage&apos;.</skos:example>
    </owl:Class>
    


    <!-- http://web-development-ontology.netlify.app/wdo#Repository -->


    <owl:Class rdf:about="http://web-development-ontology.netlify.app/wdo#Repository">
        <rdfs:subClassOf rdf:resource="http://purl.obolibrary.org/obo/BFO_0000027"/>
        <dc:identifier>WDO:0000107</dc:identifier>
        <rdfs:label xml:lang="en">Repository</rdfs:label>
        <skos:definition xml:lang="en">A Repository is an Object Aggregate whose parts are a collection of digital information carriers (files) and their revision history, managed by a version control system.</skos:definition>
        <skos:example xml:lang="en">A local or remote Git repository for a web application project.</skos:example>
    </owl:Class>
    


    <!-- http://web-development-ontology.netlify.app/wdo#RubyCode -->


    <owl:Class rdf:about="http://web-development-ontology.netlify.app/wdo#RubyCode">
        <rdfs:subClassOf rdf:resource="http://web-development-ontology.netlify.app/wdo#InterpretedLanguageCode"/>
        <dc:identifier>WDO:0000087</dc:identifier>
        <rdfs:label xml:lang="en">Ruby Code</rdfs:label>
        <skos:definition xml:lang="en">A Ruby Code is an Interpreted Language Code written in the Ruby programming language.</skos:definition>
    </owl:Class>
    


    <!-- http://web-development-ontology.netlify.app/wdo#RustCode -->


    <owl:Class rdf:about="http://web-development-ontology.netlify.app/wdo#RustCode">
        <rdfs:subClassOf rdf:resource="http://web-development-ontology.netlify.app/wdo#StaticallyTypedLanguageCode"/>
        <dc:identifier>WDO:0000102</dc:identifier>
        <rdfs:label xml:lang="en">Rust Code</rdfs:label>
        <skos:definition xml:lang="en">A Rust Code is a Statically Typed Language Code written in the Rust programming language.</skos:definition>
    </owl:Class>
    


    <!-- http://web-development-ontology.netlify.app/wdo#SQLCode -->


    <owl:Class rdf:about="http://web-development-ontology.netlify.app/wdo#SQLCode">
        <rdfs:subClassOf rdf:resource="http://web-development-ontology.netlify.app/wdo#QueryLanguageCode"/>
        <dc:identifier>WDO:0000089</dc:identifier>
        <rdfs:label xml:lang="en">SQL Code</rdfs:label>
        <skos:definition xml:lang="en">An SQL Code is a Query Language Code that is a query or schema written in the Structured Query Language (SQL).</skos:definition>
    </owl:Class>
    


    <!-- http://web-development-ontology.netlify.app/wdo#SoftwareCode -->


    <owl:Class rdf:about="http://web-development-ontology.netlify.app/wdo#SoftwareCode">
        <owl:equivalentClass rdf:resource="https://schema.org/SoftwareSourceCode"/>
        <rdfs:subClassOf rdf:resource="http://web-development-ontology.netlify.app/wdo#InformationContentEntity"/>
        <dc:identifier>WDO:0000003</dc:identifier>
        <rdfs:label xml:lang="en">Software Code</rdfs:label>
        <skos:definition xml:lang="en">A Software Code is an Information Content Entity which is a set of instructions or declarations written in a formal language, intended to be processed by a computer. This is an abstract class.</skos:definition>
        <skos:example xml:lang="en">A &apos;User.java&apos; class definition; the algorithm in a &apos;calculatePrice&apos; function; declarations in a CSS stylesheet.</skos:example>
    </owl:Class>
    


    <!-- http://web-development-ontology.netlify.app/wdo#SoftwareFramework -->


    <owl:Class rdf:about="http://web-development-ontology.netlify.app/wdo#SoftwareFramework">
        <rdfs:subClassOf rdf:resource="http://web-development-ontology.netlify.app/wdo#InformationContentEntity"/>
        <rdfs:subClassOf rdf:resource="https://schema.org/SoftwareApplication"/>
        <dc:identifier>WDO:0000092</dc:identifier>
        <rdfs:label xml:lang="en">Software Framework</rdfs:label>
        <skos:definition xml:lang="en">A Software Framework is an Information Content Entity that provides a reusable, generic platform of code for software applications, so that developers can focus on the specific logic of their application. This is an abstract class.</skos:definition>
    </owl:Class>
    


    <!-- http://web-development-ontology.netlify.app/wdo#SoftwarePackage -->


    <owl:Class rdf:about="http://web-development-ontology.netlify.app/wdo#SoftwarePackage">
        <rdfs:subClassOf rdf:resource="http://web-development-ontology.netlify.app/wdo#InformationContentEntity"/>
        <rdfs:subClassOf rdf:resource="https://schema.org/SoftwareApplication"/>
        <dc:identifier>WDO:0000012</dc:identifier>
        <rdfs:label xml:lang="en">Software Package</rdfs:label>
        <skos:definition xml:lang="en">A Software Package is an Information Content Entity which represents a distributable unit of reusable code, such as a library or module. This is an abstract class.</skos:definition>
        <skos:example xml:lang="en">The &apos;requests&apos; package in Python; the &apos;lodash&apos; package in NPM.</skos:example>
    </owl:Class>
    


    <!-- http://web-development-ontology.netlify.app/wdo#SourceCodeFile -->


    <owl:Class rdf:about="http://web-development-ontology.netlify.app/wdo#SourceCodeFile">
        <rdfs:subClassOf rdf:resource="http://web-development-ontology.netlify.app/wdo#DigitalInformationCarrier"/>
        <dc:identifier>WDO:0000031</dc:identifier>
        <rdfs:label xml:lang="en">Source Code File</rdfs:label>
        <skos:definition xml:lang="en">A Source Code File is a Digital Information Carrier that primarily bears Software Code. This is an abstract class.</skos:definition>
        <skos:example xml:lang="en">The file &apos;server.js&apos; containing JavaScript code; &apos;models.py&apos; containing Python classes; &apos;database_schema.sql&apos; containing SQL DDL statements.</skos:example>
    </owl:Class>
    


    <!-- http://web-development-ontology.netlify.app/wdo#StaticallyTypedLanguageCode -->


    <owl:Class rdf:about="http://web-development-ontology.netlify.app/wdo#StaticallyTypedLanguageCode">
        <rdfs:subClassOf rdf:resource="http://web-development-ontology.netlify.app/wdo#ProgrammingLanguageCode"/>
        <dc:identifier>WDO:0000080</dc:identifier>
        <rdfs:label xml:lang="en">Statically Typed Language Code</rdfs:label>
        <skos:definition xml:lang="en">A Statically Typed Language Code is a Programming Language Code written in a language where variable types are checked at compile-time. This is an abstract class.</skos:definition>
    </owl:Class>
    


    <!-- http://web-development-ontology.netlify.app/wdo#StructDefinition -->


    <owl:Class rdf:about="http://web-development-ontology.netlify.app/wdo#StructDefinition">
        <rdfs:subClassOf rdf:resource="http://web-development-ontology.netlify.app/wdo#ComplexType"/>
        <dc:identifier>WDO:0000059</dc:identifier>
        <rdfs:label xml:lang="en">Struct Definition</rdfs:label>
        <skos:definition xml:lang="en">A Struct Definition is a Complex Type that defines a struct, a composite data type that groups variables under a single name.</skos:definition>
        <skos:example xml:lang="en">The definition `struct Point { int x; int y; }` in C or Go.</skos:example>
    </owl:Class>
    


    <!-- http://web-development-ontology.netlify.app/wdo#Stylesheet -->


    <owl:Class rdf:about="http://web-development-ontology.netlify.app/wdo#Stylesheet">
        <rdfs:subClassOf rdf:resource="http://web-development-ontology.netlify.app/wdo#WebPresentationCode"/>
        <dc:identifier>WDO:0000064</dc:identifier>
        <rdfs:label xml:lang="en">Stylesheet</rdfs:label>
        <skos:definition xml:lang="en">A Stylesheet is a type of Web Presentation Code which defines the presentation and styling rules for a markup document. This is an abstract class.</skos:definition>
        <skos:example xml:lang="en">A CSS file defining colors, fonts, and layout; an SASS or LESS file.</skos:example>
    </owl:Class>
    


    <!-- http://web-development-ontology.netlify.app/wdo#StylesheetFile -->


    <owl:Class rdf:about="http://web-development-ontology.netlify.app/wdo#StylesheetFile">
        <rdfs:subClassOf rdf:resource="http://web-development-ontology.netlify.app/wdo#DigitalInformationCarrier"/>
        <dc:identifier>WDO:0000044</dc:identifier>
        <rdfs:label xml:lang="en">Stylesheet File</rdfs:label>
        <skos:definition xml:lang="en">A Stylesheet File is a Digital Information Carrier that bears a Stylesheet.</skos:definition>
        <skos:example xml:lang="en">A file named `styles.css` or `theme.scss`.</skos:example>
    </owl:Class>
    


    <!-- http://web-development-ontology.netlify.app/wdo#Table -->


    <owl:Class rdf:about="http://web-development-ontology.netlify.app/wdo#Table">
        <rdfs:subClassOf rdf:resource="http://web-development-ontology.netlify.app/wdo#TextualElement"/>
        <rdfs:subClassOf rdf:resource="https://schema.org/Table"/>
        <dc:identifier>WDO:0000058</dc:identifier>
        <rdfs:label xml:lang="en">Table</rdfs:label>
        <skos:definition xml:lang="en">A Table is a Textual Element which consists of data arranged in rows and columns.</skos:definition>
        <skos:example xml:lang="en">A table comparing feature plans in documentation, often created with pipe characters (`|`) in Markdown.</skos:example>
    </owl:Class>
    


    <!-- http://web-development-ontology.netlify.app/wdo#Template -->


    <owl:Class rdf:about="http://web-development-ontology.netlify.app/wdo#Template">
        <rdfs:subClassOf rdf:resource="http://web-development-ontology.netlify.app/wdo#Markup"/>
        <dc:identifier>WDO:0000065</dc:identifier>
        <rdfs:label xml:lang="en">Template</rdfs:label>
        <skos:definition xml:lang="en">A Template is a type of Markup which defines a pre-formatted structure that can be filled with data to produce a final document.</skos:definition>
        <skos:example xml:lang="en">A Handlebars (.hbs) or EJS (.ejs) file containing placeholders for dynamic data.</skos:example>
    </owl:Class>
    


    <!-- http://web-development-ontology.netlify.app/wdo#TestCode -->


    <owl:Class rdf:about="http://web-development-ontology.netlify.app/wdo#TestCode">
        <rdfs:subClassOf rdf:resource="http://web-development-ontology.netlify.app/wdo#SoftwareCode"/>
        <dc:identifier>WDO:0000119</dc:identifier>
        <rdfs:label xml:lang="en">Test Code</rdfs:label>
        <skos:definition xml:lang="en">A Test Code is a type of Software Code whose purpose is to verify the correctness of other software code.</skos:definition>
        <skos:example xml:lang="en">A unit test written using JUnit or PyTest; an integration test script.</skos:example>
    </owl:Class>
    


    <!-- http://web-development-ontology.netlify.app/wdo#TextualElement -->


    <owl:Class rdf:about="http://web-development-ontology.netlify.app/wdo#TextualElement">
        <rdfs:subClassOf rdf:resource="http://web-development-ontology.netlify.app/wdo#InformationContentEntity"/>
        <dc:identifier>WDO:0000016</dc:identifier>
        <rdfs:label xml:lang="en">Textual Element</rdfs:label>
        <skos:definition xml:lang="en">A Textual Element is an Information Content Entity which is a discrete piece of text forming part of a larger document structure. This is an abstract class.</skos:definition>
        <skos:example xml:lang="en">The content of a heading &apos;Setup Instructions&apos;; the text of a single sentence within a paragraph.</skos:example>
    </owl:Class>
    


    <!-- http://web-development-ontology.netlify.app/wdo#ThreeDimensionalModelDescription -->


    <owl:Class rdf:about="http://web-development-ontology.netlify.app/wdo#ThreeDimensionalModelDescription">
        <rdfs:subClassOf rdf:resource="http://web-development-ontology.netlify.app/wdo#DigitalAssetDescription"/>
        <rdfs:subClassOf rdf:resource="https://schema.org/3DModel"/>
        <dc:identifier>WDO:0000028</dc:identifier>
        <rdfs:label xml:lang="en">Three-Dimensional Model Description</rdfs:label>
        <skos:definition xml:lang="en">A Three-Dimensional Model Description is a Digital Asset Description that defines the characteristics of a 3D model, such as its geometry and textures.</skos:definition>
    </owl:Class>
    


    <!-- http://web-development-ontology.netlify.app/wdo#ThreeDimensionalModelFile -->


    <owl:Class rdf:about="http://web-development-ontology.netlify.app/wdo#ThreeDimensionalModelFile">
        <rdfs:subClassOf rdf:resource="http://web-development-ontology.netlify.app/wdo#AssetFile"/>
        <dc:identifier>WDO:0000041</dc:identifier>
        <rdfs:label xml:lang="en">Three-Dimensional Model File</rdfs:label>
        <skos:definition xml:lang="en">A Three-Dimensional Model File is an Asset File that bears a Three-Dimensional Model Description.</skos:definition>
        <skos:example xml:lang="en">A file named &apos;product_model.glb&apos; or &apos;character.fbx&apos;.</skos:example>
    </owl:Class>
    


    <!-- http://web-development-ontology.netlify.app/wdo#TraitDefinition -->


    <owl:Class rdf:about="http://web-development-ontology.netlify.app/wdo#TraitDefinition">
        <rdfs:subClassOf rdf:resource="http://web-development-ontology.netlify.app/wdo#ComplexType"/>
        <dc:identifier>WDO:0000116</dc:identifier>
        <rdfs:label xml:lang="en">Trait Definition</rdfs:label>
        <skos:definition xml:lang="en">A Trait Definition is a Complex Type that defines a collection of methods that can be implemented by other types, used for sharing functionality between classes.</skos:definition>
        <skos:example xml:lang="en">The definition `trait Loggable { fn log(&amp;self); }` in Rust.</skos:example>
    </owl:Class>
    


    <!-- http://web-development-ontology.netlify.app/wdo#Tutorial -->


    <owl:Class rdf:about="http://web-development-ontology.netlify.app/wdo#Tutorial">
        <rdfs:subClassOf rdf:resource="http://web-development-ontology.netlify.app/wdo#Guide"/>
        <rdfs:subClassOf rdf:resource="https://schema.org/HowTo"/>
        <dc:identifier>WDO:0000099</dc:identifier>
        <rdfs:label xml:lang="en">Tutorial</rdfs:label>
        <skos:definition xml:lang="en">A Tutorial is a type of Guide that provides step-by-step instructions to complete a specific task.</skos:definition>
    </owl:Class>
    


    <!-- http://web-development-ontology.netlify.app/wdo#TypeDeclaration -->


    <owl:Class rdf:about="http://web-development-ontology.netlify.app/wdo#TypeDeclaration">
        <rdfs:subClassOf rdf:resource="http://web-development-ontology.netlify.app/wdo#CodeConstruct"/>
        <dc:identifier>WDO:0000004</dc:identifier>
        <rdfs:label xml:lang="en">Type Declaration</rdfs:label>
        <skos:definition xml:lang="en">A Type is a Code Construct which represents the specification of a data type in a programming language. This is an abstract class.</skos:definition>
    </owl:Class>
    


    <!-- http://web-development-ontology.netlify.app/wdo#TypeScriptCode -->


    <owl:Class rdf:about="http://web-development-ontology.netlify.app/wdo#TypeScriptCode">
        <rdfs:subClassOf rdf:resource="http://web-development-ontology.netlify.app/wdo#StaticallyTypedLanguageCode"/>
        <dc:identifier>WDO:0000075</dc:identifier>
        <rdfs:label xml:lang="en">TypeScript Code</rdfs:label>
        <skos:definition xml:lang="en">A TypeScript Code is a Statically Typed Language Code written in the TypeScript programming language.</skos:definition>
    </owl:Class>
    


    <!-- http://web-development-ontology.netlify.app/wdo#UserGuide -->


    <owl:Class rdf:about="http://web-development-ontology.netlify.app/wdo#UserGuide">
        <rdfs:subClassOf rdf:resource="http://web-development-ontology.netlify.app/wdo#Guide"/>
        <rdfs:subClassOf rdf:resource="https://schema.org/HowTo"/>
        <dc:identifier>WDO:0000103</dc:identifier>
        <rdfs:label xml:lang="en">User Guide</rdfs:label>
        <skos:definition xml:lang="en">A User Guide is a type of Guide that explains how to use a software product from an end-user perspective.</skos:definition>
    </owl:Class>
    


    <!-- http://web-development-ontology.netlify.app/wdo#UserInterfaceDesignDescription -->


    <owl:Class rdf:about="http://web-development-ontology.netlify.app/wdo#UserInterfaceDesignDescription">
        <rdfs:subClassOf rdf:resource="http://web-development-ontology.netlify.app/wdo#DigitalAssetDescription"/>
        <dc:identifier>WDO:0000029</dc:identifier>
        <rdfs:label xml:lang="en">User Interface Design Description</rdfs:label>
        <skos:definition xml:lang="en">A User Interface Design Description is a Digital Asset Description that defines the visual layout and interactive elements of a user interface, such as a wireframe or mockup.</skos:definition>
    </owl:Class>
    


    <!-- http://web-development-ontology.netlify.app/wdo#UserInterfaceDesignFile -->


    <owl:Class rdf:about="http://web-development-ontology.netlify.app/wdo#UserInterfaceDesignFile">
        <rdfs:subClassOf rdf:resource="http://web-development-ontology.netlify.app/wdo#AssetFile"/>
        <dc:identifier>WDO:0000042</dc:identifier>
        <rdfs:label xml:lang="en">User Interface Design File</rdfs:label>
        <skos:definition xml:lang="en">A User Interface Design File is an Asset File that bears a User Interface Design Description.</skos:definition>
        <skos:example xml:lang="en">A file named &apos;homepage_mockup.fig&apos; or &apos;app_prototype.sketch&apos;.</skos:example>
    </owl:Class>
    


    <!-- http://web-development-ontology.netlify.app/wdo#VariableDeclaration -->


    <owl:Class rdf:about="http://web-development-ontology.netlify.app/wdo#VariableDeclaration">
        <rdfs:subClassOf rdf:resource="http://web-development-ontology.netlify.app/wdo#CodeConstruct"/>
        <rdfs:subClassOf rdf:resource="https://schema.org/PropertyValue"/>
        <dc:identifier>WDO:0000067</dc:identifier>
        <rdfs:label xml:lang="en">Variable Declaration</rdfs:label>
        <skos:definition xml:lang="en">A Variable Declaration is a Code Construct which is the declaration of a variable within a local scope, such as a function body.</skos:definition>
        <skos:example xml:lang="en">The declaration `let counter = 0;` inside a JavaScript function.</skos:example>
    </owl:Class>
    


    <!-- http://web-development-ontology.netlify.app/wdo#VideoDescription -->


    <owl:Class rdf:about="http://web-development-ontology.netlify.app/wdo#VideoDescription">
        <rdfs:subClassOf rdf:resource="http://web-development-ontology.netlify.app/wdo#DigitalAssetDescription"/>
        <dc:identifier>WDO:0000025</dc:identifier>
        <rdfs:label xml:lang="en">Video Description</rdfs:label>
        <skos:definition xml:lang="en">A Video Description is a Digital Asset Description that defines the characteristics of a video, such as its duration, frame rate, and encoding.</skos:definition>
    </owl:Class>
    


    <!-- http://web-development-ontology.netlify.app/wdo#VideoFile -->


    <owl:Class rdf:about="http://web-development-ontology.netlify.app/wdo#VideoFile">
        <rdfs:subClassOf rdf:resource="http://web-development-ontology.netlify.app/wdo#AssetFile"/>
        <rdfs:subClassOf rdf:resource="https://schema.org/VideoObject"/>
        <dc:identifier>WDO:0000038</dc:identifier>
        <rdfs:label xml:lang="en">Video File</rdfs:label>
        <skos:definition xml:lang="en">A Video File is an Asset File that bears a Video Description.</skos:definition>
        <skos:example xml:lang="en">A file named &apos;tutorial.mp4&apos; or &apos;promo.webm&apos;.</skos:example>
    </owl:Class>
    


    <!-- http://web-development-ontology.netlify.app/wdo#WebDevelopmentProject -->


    <owl:Class rdf:about="http://web-development-ontology.netlify.app/wdo#WebDevelopmentProject">
        <rdfs:subClassOf rdf:resource="http://purl.obolibrary.org/obo/BFO_0000015"/>
        <dc:identifier>WDO:0000001</dc:identifier>
        <rdfs:label xml:lang="en">Web Development Project</rdfs:label>
        <skos:definition xml:lang="en">A Web Development Project is a process that encompasses all activities involved in creating, deploying, or maintaining a web-based software system.</skos:definition>
        <skos:example xml:lang="en">The &apos;Apollo E-commerce Platform Upgrade&apos; project aiming to refactor the checkout module over three months.</skos:example>
    </owl:Class>
    


    <!-- http://web-development-ontology.netlify.app/wdo#WebPresentationCode -->


    <owl:Class rdf:about="http://web-development-ontology.netlify.app/wdo#WebPresentationCode">
        <rdfs:subClassOf rdf:resource="http://web-development-ontology.netlify.app/wdo#SoftwareCode"/>
        <dc:identifier>WDO:0000118</dc:identifier>
        <rdfs:label xml:lang="en">Web Presentation Code</rdfs:label>
        <skos:definition xml:lang="en">A Web Presentation Code is a type of Software Code that defines the structure, layout, and styling of a user interface for the web. This is an abstract class.</skos:definition>
    </owl:Class>
    


    <!-- http://web-development-ontology.netlify.app/wdo#XML -->


    <owl:Class rdf:about="http://web-development-ontology.netlify.app/wdo#XML">
        <rdfs:subClassOf rdf:resource="http://web-development-ontology.netlify.app/wdo#DataFormat"/>
        <dc:identifier>WDO:0000097</dc:identifier>
        <rdfs:label xml:lang="en">XML</rdfs:label>
        <skos:definition xml:lang="en">An XML is a Data Format that structures data according to the Extensible Markup Language syntax.</skos:definition>
    </owl:Class>
    


    <!-- http://web-development-ontology.netlify.app/wdo#YAML -->


    <owl:Class rdf:about="http://web-development-ontology.netlify.app/wdo#YAML">
        <rdfs:subClassOf rdf:resource="http://web-development-ontology.netlify.app/wdo#DataFormat"/>
        <dc:identifier>WDO:0000098</dc:identifier>
        <rdfs:label xml:lang="en">YAML</rdfs:label>
        <skos:definition xml:lang="en">A YAML is a Data Format that structures data according to the YAML Ain&apos;t Markup Language syntax.</skos:definition>
    </owl:Class>
    


    <!-- http://xmlns.com/foaf/0.1/Organization -->


    <owl:Class rdf:about="http://xmlns.com/foaf/0.1/Organization"/>
    


    <!-- http://xmlns.com/foaf/0.1/Person -->


    <owl:Class rdf:about="http://xmlns.com/foaf/0.1/Person"/>
    


    <!-- https://schema.org/APIReference -->


    <owl:Class rdf:about="https://schema.org/APIReference"/>
    


    <!-- https://schema.org/ArchiveComponent -->


    <owl:Class rdf:about="https://schema.org/ArchiveComponent"/>
    


    <!-- https://schema.org/AudioObject -->


    <owl:Class rdf:about="https://schema.org/AudioObject"/>
    


    <!-- https://schema.org/Comment -->


    <owl:Class rdf:about="https://schema.org/Comment"/>
    


    <!-- https://schema.org/CreativeWork -->


    <owl:Class rdf:about="https://schema.org/CreativeWork"/>
    


    <!-- https://schema.org/DigitalDocument -->


    <owl:Class rdf:about="https://schema.org/DigitalDocument"/>
    


    <!-- https://schema.org/Enumeration -->


    <owl:Class rdf:about="https://schema.org/Enumeration"/>
    


    <!-- https://schema.org/Function -->


    <owl:Class rdf:about="https://schema.org/Function"/>
    


    <!-- https://schema.org/HowTo -->


    <owl:Class rdf:about="https://schema.org/HowTo"/>
    


    <!-- https://schema.org/ImageObject -->


    <owl:Class rdf:about="https://schema.org/ImageObject"/>
    


    <!-- https://schema.org/ItemList -->


    <owl:Class rdf:about="https://schema.org/ItemList"/>
    


    <!-- https://schema.org/MediaObject -->


    <owl:Class rdf:about="https://schema.org/MediaObject"/>
    


    <!-- https://schema.org/Message -->


    <owl:Class rdf:about="https://schema.org/Message"/>
    


    <!-- https://schema.org/PropertyValue -->


    <owl:Class rdf:about="https://schema.org/PropertyValue"/>
    


    <!-- https://schema.org/SoftwareApplication -->


    <owl:Class rdf:about="https://schema.org/SoftwareApplication"/>
    


    <!-- https://schema.org/SoftwareSourceCode -->


    <owl:Class rdf:about="https://schema.org/SoftwareSourceCode"/>
    


    <!-- https://schema.org/Table -->


    <owl:Class rdf:about="https://schema.org/Table"/>
    


    <!-- https://schema.org/TechArticle -->


    <owl:Class rdf:about="https://schema.org/TechArticle"/>
    


    <!-- https://schema.org/UpdateAction -->


    <owl:Class rdf:about="https://schema.org/UpdateAction"/>
    


    <!-- https://schema.org/VideoObject -->


    <owl:Class rdf:about="https://schema.org/VideoObject"/>
    


    <!-- https://schema.org/3DModel -->


    <owl:Class rdf:about="https://schema.org/3DModel"/>
    


    <!-- 
    ///////////////////////////////////////////////////////////////////////////////////////
    //
    // General axioms
    //
    ///////////////////////////////////////////////////////////////////////////////////////
     -->


    <rdf:Description>
        <rdf:type rdf:resource="http://www.w3.org/2002/07/owl#AllDisjointClasses"/>
        <owl:members rdf:parseType="Collection">
            <rdf:Description rdf:about="http://purl.obolibrary.org/obo/BFO_0000004"/>
            <rdf:Description rdf:about="http://purl.obolibrary.org/obo/BFO_0000020"/>
            <rdf:Description rdf:about="http://purl.obolibrary.org/obo/BFO_0000031"/>
        </owl:members>
    </rdf:Description>
    <rdf:Description>
        <rdf:type rdf:resource="http://www.w3.org/2002/07/owl#AllDisjointClasses"/>
        <owl:members rdf:parseType="Collection">
            <rdf:Description rdf:about="http://purl.obolibrary.org/obo/BFO_0000006"/>
            <rdf:Description rdf:about="http://purl.obolibrary.org/obo/BFO_0000029"/>
            <rdf:Description rdf:about="http://purl.obolibrary.org/obo/BFO_0000140"/>
        </owl:members>
    </rdf:Description>
    <rdf:Description>
        <rdf:type rdf:resource="http://www.w3.org/2002/07/owl#AllDisjointClasses"/>
        <owl:members rdf:parseType="Collection">
            <rdf:Description rdf:about="http://purl.obolibrary.org/obo/BFO_0000008"/>
            <rdf:Description rdf:about="http://purl.obolibrary.org/obo/BFO_0000011"/>
            <rdf:Description rdf:about="http://purl.obolibrary.org/obo/BFO_0000015"/>
            <rdf:Description rdf:about="http://purl.obolibrary.org/obo/BFO_0000035"/>
        </owl:members>
    </rdf:Description>
    <rdf:Description>
        <rdf:type rdf:resource="http://www.w3.org/2002/07/owl#AllDisjointClasses"/>
        <owl:members rdf:parseType="Collection">
            <rdf:Description rdf:about="http://purl.obolibrary.org/obo/BFO_0000009"/>
            <rdf:Description rdf:about="http://purl.obolibrary.org/obo/BFO_0000018"/>
            <rdf:Description rdf:about="http://purl.obolibrary.org/obo/BFO_0000026"/>
            <rdf:Description rdf:about="http://purl.obolibrary.org/obo/BFO_0000028"/>
        </owl:members>
    </rdf:Description>
    <rdf:Description>
        <rdf:type rdf:resource="http://www.w3.org/2002/07/owl#AllDisjointClasses"/>
        <owl:members rdf:parseType="Collection">
            <rdf:Description rdf:about="http://purl.obolibrary.org/obo/BFO_0000142"/>
            <rdf:Description rdf:about="http://purl.obolibrary.org/obo/BFO_0000146"/>
            <rdf:Description rdf:about="http://purl.obolibrary.org/obo/BFO_0000147"/>
        </owl:members>
    </rdf:Description>
</rdf:RDF>



<!-- Generated by the OWL API (version 5.1.18) https://github.com/owlcs/owlapi/ -->


